@prefix rdf: <http://www.w3.org/1999/02/22-rdf-syntax-ns#>.
@prefix rdfs: <http://www.w3.org/2000/01/rdf-schema#>.
@prefix schema: <http://schema.org/>.
@prefix xml: <http://www.w3.org/XML/1998/namespace>.
@prefix xsd: <http://www.w3.org/2001/XMLSchema#>.

schema:Abortion a rdfs:Class ;
    rdfs:label "Abortion" ;
    rdfs:comment "Abortion is the ending of pregnancy by the removal or expulsion from the uterus of a fetus or embryo before viability." ;
    rdfs:subClassOf schema:CreatedInExtension,
        schema:GynObsHistory .

schema:Acupuncture a rdfs:Class ;
    rdfs:label "Acupuncture" ;
    rdfs:comment "A system of complementary medicine in which fine needles are inserted in the skin at specific points along what are considered to be lines of energy (meridians), used in the treatment of various physical and mental conditions." ;
    rdfs:subClassOf schema:AlternativeTherapy,
        schema:CreatedInExtension .

schema:AdministrativeProcedure a rdfs:Class ;
    rdfs:label "AdministrativeProcedure" ;
    rdfs:comment "Procedure related to the administrative aspects of health care, including, business, legal, financial, quality review, peer review, data reporting, notification, and so forth" ;
    rdfs:subClassOf schema:CreatedInExtension,
        schema:MedicalProcedure .

schema:AdulthoodHistory a rdfs:Class ;
    rdfs:label "AdulthoodHistory" ;
    rdfs:comment "Any medical history happening in adulthood, the period of time in your life after your physical growth has stopped and you are fully developed" ;
    rdfs:subClassOf schema:CreatedInExtension,
        schema:SocialHistory .

schema:AdverseDrugReaction a rdfs:Class ;
    rdfs:label "AdverseDrugReaction" ;
    rdfs:comment "An adverse drug reaction is an expression that describes harm associated with the use of given medications at a normal dosage during normal use. " ;
    rdfs:subClassOf schema:AdverseEvent,
        schema:CreatedInExtension .

schema:AdverseEvent a rdfs:Class ;
    rdfs:label "AdverseEvent" ;
    rdfs:comment "In medicine, an adverse effect is an undesired harmful effect associated with the use of a medical product or other intervention such as surgery in a patient ." ;
    rdfs:subClassOf schema:CreatedInExtension,
        schema:MedicalCondition .

schema:AlcoholIntake a rdfs:Class ;
    rdfs:label "AlcoholIntake" ;
    rdfs:comment "The quantification or description of alcohol intake for the person" ;
    rdfs:subClassOf schema:CreatedInExtension,
        schema:LifestyleOrHabits .

schema:Allergen a rdfs:Class ;
    rdfs:label "Allergen" ;
    rdfs:comment "Any substance, often a protein, that induces an allergy: common allergens include pollen, grasses, dust, and some medications." ;
    rdfs:subClassOf schema:CreatedInExtension,
        schema:Substance .

schema:Allergy a rdfs:Class ;
    rdfs:label "Allergy" ;
    rdfs:comment "An abnormal reaction of the body to a previously encountered allergen." ;
    rdfs:subClassOf schema:CreatedInExtension,
        schema:MedicalCondition .

schema:AlternativeTherapy a rdfs:Class ;
    rdfs:label "AlternativeTherapy" ;
    rdfs:comment "Any practice that is put forward as having the healing effects of medicine but is not based on evidence gathered using the scientific method. It may however consists of a wide range of health care practices, products and therapies known in conventional medicine. Source: Wikipedia" ;
    rdfs:subClassOf schema:CreatedInExtension,
        schema:TherapeuticProcedure .

schema:AnamnesisProcedure a rdfs:Class ;
    rdfs:label "AnamnesisProcedure" ;
    rdfs:comment "Interview aiming collecting of the medical history of a patient." ;
    rdfs:subClassOf schema:CreatedInExtension,
        schema:MedicalProcedure .

schema:AnatomicalEntity a rdfs:Class ;
    rdfs:label "AnatomicalEntity" ;
    rdfs:comment "Defining an anatomical resource of the human body." ;
    rdfs:subClassOf schema:CreatedInExtension,
        schema:MedicalEntity .

schema:AnatomicalOrgan a rdfs:Class ;
    rdfs:label "AnatomicalOrgan" ;
    rdfs:comment "In biology or anatomy, an organ (or viscus) is a collection of tissues joined in a structural unit to serve a common function." ;
    rdfs:subClassOf schema:AnatomicalEntity,
        schema:CreatedInExtension .

schema:AnatomicalRegion a rdfs:Class ;
    rdfs:label "AnatomicalRegion" ;
    rdfs:comment "Anatomy based region of the human body which describe areas of the body that have a special function or are supplied by specific blood vessels or nerves." ;
    rdfs:subClassOf schema:AnatomicalEntity,
        schema:CreatedInExtension .

schema:AnatomicalStructure a rdfs:Class ;
    rdfs:label "AnatomicalStructure" ;
    rdfs:comment "Any part of the human body, typically a component of an anatomical system. Organs, tissues, and cells are all anatomical structures." ;
    rdfs:subClassOf schema:AnatomicalEntity,
        schema:MovedFromCore .

schema:AnatomicalSystem a rdfs:Class ;
    rdfs:label "AnatomicalSystem" ;
    rdfs:comment "An anatomical system is a group of anatomical structures that work together to perform a certain task. Anatomical systems, such as organ systems, are one organizing principle of anatomy, and can includes circulatory, digestive, endocrine, integumentary, immune, lymphatic, muscular, nervous, reproductive, respiratory, skeletal, urinary, vestibular, and other systems." ;
    rdfs:subClassOf schema:AnatomicalEntity,
        schema:MovedFromCore .

schema:Angiography a rdfs:Class ;
    rdfs:label "Angiography" ;
    rdfs:comment "Radiography of blood or lymph vessels, carried out after introduction of a radiopaque substance." ;
    rdfs:subClassOf schema:CreatedInExtension,
        schema:MedicalImaging .

schema:ApgarScore a rdfs:Class ;
    rdfs:label "ApgarScore" ;
    rdfs:comment "A scoring method to quickly and summarily assess the health of newborn children immediately after birth." ;
    rdfs:subClassOf schema:CreatedInExtension,
        schema:MedicalScore .

schema:ApprovedIndication a rdfs:Class ;
    rdfs:label "ApprovedIndication" ;
    rdfs:comment "An indication for a medical therapy that has been formally specified or approved by a regulatory body that regulates use of the therapy; for example, the US FDA approves indications for most drugs in the US." ;
    rdfs:subClassOf schema:MedicalIndication,
        schema:MovedFromCore .

schema:Artery a rdfs:Class ;
    rdfs:label "Artery" ;
    rdfs:comment "A type of blood vessel that specifically carries blood away from the heart." ;
    rdfs:subClassOf schema:MovedFromCore,
        schema:Vessel .

schema:AxillaryTemperature a rdfs:Class ;
    rdfs:label "AxillaryTemperature" ;
    rdfs:comment "Temperature of human body taken in axillary region" ;
    rdfs:subClassOf schema:BodyTemperature,
        schema:CreatedInExtension .

schema:BiologicalSubstance a rdfs:Class ;
    rdfs:label "BiologicalSubstance" ;
    rdfs:comment "Material produced by living organisms; it can be a necessary constituent of, or product of an organismal process" ;
    rdfs:subClassOf schema:CreatedInExtension,
        schema:Substance .

schema:Birth a rdfs:Class ;
    rdfs:label "Birth" ;
    rdfs:comment "The event, act or process of bearing or bringing forth offspring" ;
    rdfs:subClassOf schema:CreatedInExtension,
        schema:LifeEvent .

schema:BloodPressure a rdfs:Class ;
    rdfs:label "BloodPressure" ;
    rdfs:comment "Blood pressure (BP), sometimes referred to as arterial blood pressure, is the pressure exerted by circulating blood upon the walls of blood vessels, and is one of the principal vital signs. " ;
    rdfs:subClassOf schema:CreatedInExtension,
        schema:VitalSign .

schema:BloodTest a rdfs:Class ;
    rdfs:label "BloodTest" ;
    rdfs:comment "A medical test performed on a sample of a patient's blood." ;
    rdfs:subClassOf schema:MedicalTest,
        schema:MovedFromCore .

schema:BodyMassIndex a rdfs:Class ;
    rdfs:label "BodyMassIndex" ;
    rdfs:comment "Also known as BMI, is measure of relative weight based on an individual's mass and height." ;
    rdfs:subClassOf schema:BodyMeasure,
        schema:CreatedInExtension .

schema:BodyMeasure a rdfs:Class ;
    rdfs:label "BodyMeasure" ;
    rdfs:comment "Common method of specifying body sizes parameters" ;
    rdfs:subClassOf schema:CreatedInExtension,
        schema:PhysicalExam .

schema:BodySubstance a rdfs:Class ;
    rdfs:label "BodySubstance" ;
    rdfs:comment "The substance of the human body." ;
    rdfs:subClassOf schema:CreatedInExtension,
        schema:Substance .

schema:BodyTemperature a rdfs:Class ;
    rdfs:label "BodyTemperature" ;
    rdfs:comment "Human body temperature is the temperature of person's body. " ;
    rdfs:subClassOf schema:CreatedInExtension,
        schema:VitalSign .

schema:BodyVolumeIndex a rdfs:Class ;
    rdfs:label "BodyVolumeIndex" ;
    rdfs:comment "Measurement for obesity,  based at the relationship between mass and volume distribution" ;
    rdfs:subClassOf schema:BodyMeasure,
        schema:CreatedInExtension .

schema:Bone a rdfs:Class ;
    rdfs:label "Bone" ;
    rdfs:comment "Rigid connective tissue that comprises up the skeletal structure of the human body." ;
    rdfs:subClassOf schema:AnatomicalStructure,
        schema:MovedFromCore .

schema:BrainStructure a rdfs:Class ;
    rdfs:label "BrainStructure" ;
    rdfs:comment "Any anatomical structure which pertains to the soft nervous tissue functioning as the coordinating center of sensation and intellectual and nervous activity." ;
    rdfs:subClassOf schema:AnatomicalStructure,
        schema:MovedFromCore .

schema:CardiovascularSystem a rdfs:Class ;
    rdfs:label "CardiovascularSystem" ;
    rdfs:comment "A circulatory system which distributes blood through the body" ;
    rdfs:subClassOf schema:CirculatorySystem,
        schema:CreatedInExtension .

schema:CarePlan a rdfs:Class ;
    rdfs:label "CarePlan" ;
    rdfs:comment "Describes the intention of how one or more practitioners intend to deliver care for a particular patient for a period of time, possibly limited to care for a specific condition or set of conditions.." ;
    rdfs:subClassOf schema:CreatedInExtension,
        schema:LifeEvent .

schema:CaringEvent a rdfs:Class ;
    rdfs:label "CaringEvent" ;
    rdfs:comment "Commonly regarded as 'episode of care, the caring event refers to any event of the prevention, treatment, and management of illness and the preservation of mental and physical well-being through the services offered by the medical and allied health professions." ;
    rdfs:subClassOf schema:CreatedInExtension,
        schema:LifeEvent .

schema:ChemicalSubstance a rdfs:Class ;
    rdfs:label "ChemicalSubstance" ;
    rdfs:comment "Substance produced by or used in a reaction involving changes in atoms or molecules" ;
    rdfs:subClassOf schema:CreatedInExtension,
        schema:Substance .

schema:Chemotherapy a rdfs:Class ;
    rdfs:label "Chemotherapy" ;
    rdfs:comment "The word chemotherapy means the use of any drug (such as aspirin or penicillin) to treat any disease, but to most people chemotherapy refers to drugs used for cancer treatment." ;
    rdfs:subClassOf schema:CreatedInExtension,
        schema:Pharmacotherapy .

schema:ChiefComplaint a rdfs:Class ;
    rdfs:label "ChiefComplaint" ;
    rdfs:comment "Also  termed Presenting Complaint, Reason for Encounter, Presenting Problem, Problem on admission or Reason for Presenting, refers the primary symptom that a patient states as the reason for seeking medical care." ;
    rdfs:subClassOf schema:CreatedInExtension,
        schema:MedicalSymptom .

schema:ChildhoodHistory a rdfs:Class ;
    rdfs:label "ChildhoodHistory" ;
    rdfs:comment "Any medical history happening in childhood" ;
    rdfs:subClassOf schema:CreatedInExtension,
        schema:SocialHistory .

schema:CirculatorySystem a rdfs:Class ;
    rdfs:label "CirculatorySystem" ;
    rdfs:comment "The circulatory system is an organ system that permits blood and lymph circulation to transport nutrients, oxygen, carbon dioxide, hormones, blood cells, etc. to and from cells in the body " ;
    rdfs:subClassOf schema:AnatomicalSystem,
        schema:CreatedInExtension .

schema:ClinicalDocument a rdfs:Class ;
    rdfs:label "ClinicalDocument" ;
    rdfs:comment "Any document used throughout healthcare to describe care provided to a patient, communicate essential information between healthcare providers and to maintain a patient medical record. " ;
    rdfs:subClassOf schema:CreatedInExtension,
        schema:MedicalEntity .

schema:ClinicalFinding a rdfs:Class ;
    rdfs:label "ClinicalFinding" ;
    rdfs:comment "The result of a clinical observation, assessment or judgement, and include both normal and abnormal clinical states." ;
    rdfs:subClassOf schema:CreatedInExtension,
        schema:MedicalEntity .

schema:ComputedTomography a rdfs:Class ;
    rdfs:label "ComputedTomography" ;
    rdfs:comment "A method of examining body organs by scanning them with X rays and using a computer to construct a series of cross-sectional scans along a single axis" ;
    rdfs:subClassOf schema:CreatedInExtension,
        schema:MedicalImaging .

schema:CosmeticProcedure a rdfs:Class ;
    rdfs:label "CosmeticProcedure" ;
    rdfs:comment "Procedures which improve the appearance, but are not medically necessary." ;
    rdfs:subClassOf schema:CreatedInExtension,
        schema:ElectiveProcedure .

schema:CreatedInCore a rdfs:Class ;
    rdfs:label "CreatedInCore" ;
    rdfs:comment "A class of all items, related to the extension but created in the schema core" ;
    rdfs:subClassOf schema:Enumeration .

schema:CreatedInExtension a rdfs:Class ;
    rdfs:label "CreatedInExtension" ;
    rdfs:comment "A class of all items created the extension" ;
    rdfs:subClassOf schema:Thing .

schema:DDxElement a rdfs:Class ;
    rdfs:label "DDxElement" ;
    rdfs:comment "An alternative, closely-related condition typically considered later in the differential diagnosis process along with the signs that are used to distinguish it." ;
    rdfs:subClassOf schema:MedicalIntangible,
        schema:MovedFromCore .

schema:DataReporter a rdfs:Class ;
    rdfs:label "DataReporter" ;
    rdfs:comment "Somebody who makes a report of any kind, e.g. a person who is authorized to gather and give a formal or official account or description of findings, events, issues and other information regarding clinical study, drug adverse effect, pre-clinical research results, data and safety monitoring, etc. to appropriate agency or institution. Source NCIt" ;
    rdfs:subClassOf schema:CreatedInExtension,
        schema:HealthcareProfessional .

schema:Death a rdfs:Class ;
    rdfs:label "Death" ;
    rdfs:comment "Death is the cessation of all biological functions that sustain a living organism. " ;
    rdfs:subClassOf schema:CreatedInExtension,
        schema:LifeEvent .

schema:Dentist a rdfs:Class ;
    rdfs:label "Dentist" ;
    rdfs:comment "A dentist." ;
    rdfs:subClassOf schema:MedicalOrganization,
        schema:MovedFromCore,
        schema:ProfessionalService .

schema:Dermis a rdfs:Class ;
    rdfs:label "Dermis" ;
    rdfs:comment "The dermis is the middle layer of skin, composed of dense irregular connective tissue and areolar connective tissue such as collagen with elastin arranged in a diffusely bundled and woven pattern." ;
    rdfs:subClassOf schema:CreatedInExtension,
        schema:IntegumentarySystem .

schema:Diagnosis a rdfs:Class ;
    rdfs:label "Diagnosis" ;
    rdfs:comment "The diagnosis my refer as well to the process of determining by examination the nature and circumstances of a diseased condition or to the decision reached from such an examination. " ;
    rdfs:subClassOf schema:CreatedInExtension,
        schema:MedicalCondition .

schema:DiagnosticLab a rdfs:Class ;
    rdfs:label "DiagnosticLab" ;
    rdfs:comment "A medical laboratory that offers on-site or off-site diagnostic services." ;
    rdfs:subClassOf schema:MedicalOrganization,
        schema:MovedFromCore .

schema:DiagnosticProcedure a rdfs:Class ;
    rdfs:label "DiagnosticProcedure" ;
    rdfs:comment "A medical procedure intended primarily for diagnostic, as opposed to therapeutic, purposes." ;
    rdfs:subClassOf schema:MedicalProcedure,
        schema:MedicalTest,
        schema:MovedFromCore .

schema:Diet a rdfs:Class ;
    rdfs:label "Diet" ;
    rdfs:comment "A strategy of regulating the intake of food to achieve or maintain a specific health-related goal." ;
    rdfs:subClassOf schema:CreativeWork,
        schema:LifestyleModification,
        schema:MovedFromCore .

schema:DietarySupplement a rdfs:Class ;
    rdfs:label "DietarySupplement" ;
    rdfs:comment "A product taken by mouth that contains a dietary ingredient intended to supplement the diet. Dietary ingredients may include vitamins, minerals, herbs or other botanicals, amino acids, and substances such as enzymes, organ tissues, glandulars and metabolites." ;
    rdfs:subClassOf schema:MedicalTherapy,
        schema:MovedFromCore .

schema:DigestiveSystem a rdfs:Class ;
    rdfs:label "DigestiveSystem" ;
    rdfs:comment "The human digestive system is a complex series of organs and glands that processes food. Digestion involves the breakdown of food into smaller and smaller components which can be absorbed and assimilated into the body." ;
    rdfs:subClassOf schema:AnatomicalSystem,
        schema:CreatedInExtension .

schema:Disability a rdfs:Class ;
    rdfs:label "Disability" ;
    rdfs:comment "Any disability history in patient anamnesis" ;
    rdfs:subClassOf schema:CreatedInExtension,
        schema:SocialHistory .

schema:Disease a rdfs:Class ;
    rdfs:label "Disease" ;
    rdfs:comment "The term disease broadly refers to any condition that impairs normal function, and is therefore associated with dysfunction of normal homeostasis. In other side, in medicine, a disorder is a functional abnormality or disturbance. Source: Wikipedia." ;
    rdfs:subClassOf schema:CreatedInExtension,
        schema:MedicalCondition .

schema:DoseSchedule a rdfs:Class ;
    rdfs:label "DoseSchedule" ;
    rdfs:comment "A specific dosing schedule for a drug or supplement." ;
    rdfs:subClassOf schema:MedicalIntangible,
        schema:MovedFromCore .

schema:Drug a rdfs:Class ;
    rdfs:label "Drug" ;
    rdfs:comment "A chemical or biologic substance, used as a medical therapy, that has a physiological effect on an organism. Here the term drug is used interchangeably with the term medicine although clinical knowledge make a clear difference between them." ;
    rdfs:subClassOf schema:MovedFromCore,
        schema:PharmaceuticalSubstance .

schema:DrugClass a rdfs:Class ;
    rdfs:label "DrugClass" ;
    rdfs:comment "A class of medical drugs, e.g., statins. Classes can represent general pharmacological class, common mechanisms of action, common physiological effects, etc." ;
    rdfs:subClassOf schema:MedicalEnumeration,
        schema:MovedFromCore .

schema:DrugCost a rdfs:Class ;
    rdfs:label "DrugCost" ;
    rdfs:comment "The cost per unit of a medical drug. Note that this type is not meant to represent the price in an offer of a drug for sale; see the Offer type for that. This type will typically be used to tag wholesale or average retail cost of a drug, or maximum reimbursable cost. Costs of medical drugs vary widely depending on how and where they are paid for, so while this type captures some of the variables, costs should be used with caution by consumers of this schema's markup." ;
    rdfs:subClassOf schema:MedicalEnumeration,
        schema:MovedFromCore .

schema:DrugCostCategory a rdfs:Class ;
    rdfs:label "DrugCostCategory" ;
    rdfs:comment "Enumerated categories of medical drug costs." ;
    rdfs:subClassOf schema:Enumeration,
        schema:MedicalEnumeration,
        schema:MovedFromCore .

schema:DrugLegalStatus a rdfs:Class ;
    rdfs:label "DrugLegalStatus" ;
    rdfs:comment "The legal availability status of a medical drug." ;
    rdfs:subClassOf schema:MedicalIntangible,
        schema:MovedFromCore .

schema:DrugPackage a rdfs:Class ;
    rdfs:label "DrugPackage" ;
    rdfs:comment "The drug or medicine package" ;
    rdfs:subClassOf schema:CreatedInExtension,
        schema:MedicalEnumeration .

schema:DrugPregnancyCategory a rdfs:Class ;
    rdfs:label "DrugPregnancyCategory" ;
    rdfs:comment "Categories that represent an assessment of the risk of fetal injury due to a drug or pharmaceutical used as directed by the mother during pregnancy." ;
    rdfs:subClassOf schema:Enumeration,
        schema:MedicalEnumeration,
        schema:MovedFromCore .

schema:DrugPrescriptionStatus a rdfs:Class ;
    rdfs:label "DrugPrescriptionStatus" ;
    rdfs:comment "Indicates whether this drug is available by prescription or over-the-counter." ;
    rdfs:subClassOf schema:Enumeration,
        schema:MedicalEnumeration,
        schema:MovedFromCore .

schema:DrugStrength a rdfs:Class ;
    rdfs:label "DrugStrength" ;
    rdfs:comment "A specific strength in which a medical drug is available in a specific country." ;
    rdfs:subClassOf schema:MedicalIntangible,
        schema:MovedFromCore .

schema:EHR a rdfs:Class ;
    rdfs:label "EHR" ;
    rdfs:comment "The Electronic Health Record (EHR) is an electronic record of health-related information on an individual that conforms to nationally recognized interoperability standards and that can be created, managed, and consulted by authorized clinicians and staff across more than one health care organization.US NAHIT" ;
    rdfs:subClassOf schema:CreatedInExtension,
        schema:MedicalRecord .

schema:EMR a rdfs:Class ;
    rdfs:label "EMR" ;
    rdfs:comment "An Electronic Medical Record (EMR) is an electronic record of health-related information on an individual that can be created, gathered, managed, and consulted by authorized clinicians and staff within one health care organization. Source: US NAHIT" ;
    rdfs:subClassOf schema:CreatedInExtension,
        schema:MedicalRecord .

schema:EducationLevel a rdfs:Class ;
    rdfs:label "EducationLevel" ;
    rdfs:comment "The level of formal education" ;
    rdfs:subClassOf schema:CreatedInExtension,
        schema:SocialHistory .

schema:Elderhood a rdfs:Class ;
    rdfs:label "Elderhood" ;
    rdfs:comment "Any medical history happening in elderhood" ;
    rdfs:subClassOf schema:CreatedInExtension,
        schema:SocialHistory .

schema:ElectiveProcedure a rdfs:Class ;
    rdfs:label "ElectiveProcedure" ;
    rdfs:comment " An elective procedure is one that is chosen (elected) by the patient or physician that is advantageous to the patient but is not urgent." ;
    rdfs:subClassOf schema:CreatedInExtension,
        schema:MedicalProcedure .

schema:EndocrineSystem a rdfs:Class ;
    rdfs:label "EndocrineSystem" ;
    rdfs:comment "The endocrine system refers to the collection of glands of an organism that secrete hormones directly into the circulatory system to be carried toward a distant target organ." ;
    rdfs:subClassOf schema:AnatomicalSystem,
        schema:CreatedInExtension .

schema:Endoscopy a rdfs:Class ;
    rdfs:label "Endoscopy" ;
    rdfs:comment "Visual examination of the interior of a hollow body organ by use of an endoscope" ;
    rdfs:subClassOf schema:CreatedInExtension,
        schema:MedicalImaging .

schema:Enumeration a rdfs:Class ;
    rdfs:label "Enumeration" ;
    rdfs:comment "Lists or enumerations—for example, a list of cuisines or music genres, etc." ;
    rdfs:subClassOf schema:Intangible,
        schema:MaintainedInCore .

schema:Epidermis a rdfs:Class ;
    rdfs:label "Epidermis" ;
    rdfs:comment "This is the top layer of skin made up of epithelial cells." ;
    rdfs:subClassOf schema:CreatedInExtension,
        schema:IntegumentarySystem .

schema:Episodicity a rdfs:Class ;
    rdfs:label "Episodicity" ;
    rdfs:comment "A quantification of a medical condition occurrences." ;
    rdfs:subClassOf schema:CreatedInExtension,
        schema:MedicalEnumeration .

schema:Ethnicity a rdfs:Class ;
    rdfs:label "Ethnicity" ;
    rdfs:comment "A social group characterized by a distinctive social and cultural tradition that is maintained from generation to generation. " ;
    rdfs:subClassOf schema:CreatedInExtension,
        schema:SocialHistory .

schema:ExercisePlan a rdfs:Class ;
    rdfs:label "ExercisePlan" ;
    rdfs:comment "Fitness-related activity designed for a specific health-related purpose, including defined exercise routines as well as activity prescribed by a clinician." ;
    rdfs:subClassOf schema:CreativeWork,
        schema:MovedFromCore,
        schema:PhysicalActivity .

schema:FamilyMedicalHistory a rdfs:Class ;
    rdfs:label "FamilyMedicalHistory" ;
    rdfs:comment "In medicine, as a part of medical history, the family history consists of information about disorders from which the direct blood relatives of the patient have suffered." ;
    rdfs:subClassOf schema:CreatedInExtension,
        schema:MedicalHistory .

schema:FamilyRelation a rdfs:Class ;
    rdfs:label "FamilyRelation" ;
    rdfs:comment "Relationship relatedness or connection by blood, marriage or adoption ." ;
    rdfs:subClassOf schema:CreatedInExtension,
        schema:MedicalEnumeration .

schema:FoodIntolerance a rdfs:Class ;
    rdfs:label "FoodIntolerance" ;
    rdfs:comment "Food intolerance or non-allergic food hypersensitivity is a term used widely for varied physiological responses associated with a particular food, or compound found in a range of foods." ;
    rdfs:subClassOf schema:CreatedInExtension,
        schema:MedicalCondition .

schema:GeneTherapy a rdfs:Class ;
    rdfs:label "GeneTherapy" ;
    rdfs:comment "The introduction of normal genes into cells in place of missing or defective ones in order to correct genetic disorders." ;
    rdfs:subClassOf schema:CreatedInExtension,
        schema:MedicalTherapy .

schema:Gland a rdfs:Class ;
    rdfs:label "Gland" ;
    rdfs:comment "A gland is an organ in an animal's body that synthesizes a substance such as hormones for release into the bloodstream (endocrine gland) or into cavities inside the body or its outer surface (exocrine gland)." ;
    rdfs:subClassOf schema:CreatedInExtension,
        schema:EndocrineSystem .

schema:Gravidity a rdfs:Class ;
    rdfs:label "Gravidity" ;
    rdfs:comment "Gravidity is defined as the number of times that a woman has been pregnant." ;
    rdfs:subClassOf schema:CreatedInExtension,
        schema:GynObsHistory .

schema:GynObsHistory a rdfs:Class ;
    rdfs:label "GynObsHistory" ;
    rdfs:comment "As a part of personal medical history, the gynecology and obstetric history consist of information about reproductive life of the patient" ;
    rdfs:subClassOf schema:CreatedInExtension,
        schema:PersonalHistory .

schema:HealthFacility a rdfs:Class ;
    rdfs:label "HealthFacility" ;
    rdfs:comment "A medical facility is, in general, any location where healthcare is provided or medicine is practised regularly. " ;
    rdfs:subClassOf schema:CreatedInExtension,
        schema:MedicalEntity .

schema:HealthcareProfessional a rdfs:Class ;
    rdfs:label "HealthcareProfessional" ;
    rdfs:comment "Any person working in healthcare settings. This includes healthcare providers but also data reporters, and others" ;
    rdfs:subClassOf schema:CreatedInExtension,
        schema:MedicalEntity .

schema:HealthcareProvider a rdfs:Class ;
    rdfs:label "HealthcareProvider" ;
    rdfs:comment "A health care provider is an individual or an institution that provides preventive, curative, promotional or rehabilitative health care services in a systematic way to individuals, families or communities." ;
    rdfs:subClassOf schema:CreatedInExtension,
        schema:HealthcareProfessional .

schema:HeartRate a rdfs:Class ;
    rdfs:label "HeartRate" ;
    rdfs:comment "In medicine, heart rate represents the heat beat frequency normally evaluated per minute. " ;
    rdfs:subClassOf schema:CreatedInExtension,
        schema:VitalSign .

schema:HipCircumference a rdfs:Class ;
    rdfs:label "HipCircumference" ;
    rdfs:comment "A measurement of the hips, including the widest portion of the buttocks, used in conjunction with the waist circumference, body weight and percent body fat to calculate the body composition score." ;
    rdfs:subClassOf schema:BodyMeasure,
        schema:CreatedInExtension .

schema:HistoryOfPresentIllness a rdfs:Class ;
    rdfs:label "HistoryOfPresentIllness" ;
    rdfs:comment "As a part of personal medical history, the history of the present illness consist of information about the patient present problem history." ;
    rdfs:subClassOf schema:CreatedInExtension,
        schema:PersonalHistory .

schema:Homeostasis a rdfs:Class ;
    rdfs:label "Homeostasis" ;
    rdfs:comment "The ability or tendency of an organism or cell to maintain internal equilibrium by adjusting its physiological processes." ;
    rdfs:subClassOf schema:CreatedInExtension,
        schema:PhysiologicalEntity .

schema:HormoneTherapy a rdfs:Class ;
    rdfs:label "HormoneTherapy" ;
    rdfs:comment "Hormone therapy or hormonal therapy is the use of hormones in medical treatment. " ;
    rdfs:subClassOf schema:CreatedInExtension,
        schema:MedicalTherapy .

schema:Hospital a rdfs:Class ;
    rdfs:label "Hospital" ;
    rdfs:comment "A hospital." ;
    rdfs:subClassOf schema:CivicStructure,
        schema:EmergencyService,
        schema:MedicalOrganization,
        schema:MovedFromCore .

schema:Hydrotherapy a rdfs:Class ;
    rdfs:label "Hydrotherapy" ;
    rdfs:comment "Hydrotherapy, or water therapy, is the use of water (hot, cold, steam, or ice) to relieve discomfort and promote physical well-being." ;
    rdfs:subClassOf schema:AlternativeTherapy,
        schema:CreatedInExtension .

schema:Hypodermis a rdfs:Class ;
    rdfs:label "Hypodermis" ;
    rdfs:comment "The innermost and thickest layer of the skin." ;
    rdfs:subClassOf schema:CreatedInExtension,
        schema:IntegumentarySystem .

schema:ImagingTest a rdfs:Class ;
    rdfs:label "ImagingTest" ;
    rdfs:comment "Any medical imaging modality typically used for diagnostic purposes." ;
    rdfs:subClassOf schema:MedicalTest,
        schema:MovedFromCore .

schema:ImmuneSystem a rdfs:Class ;
    rdfs:label "ImmuneSystem" ;
    rdfs:comment "The immune system is a system of biological structures and processes within an organism that protects against disease." ;
    rdfs:subClassOf schema:AnatomicalSystem,
        schema:CreatedInExtension .

schema:Immunotherapy a rdfs:Class ;
    rdfs:label "Immunotherapy" ;
    rdfs:comment "The treatment of disease by inducing, enhancing, or suppressing an immune response." ;
    rdfs:subClassOf schema:CreatedInExtension,
        schema:Pharmacotherapy .

schema:InfectiousAgentClass a rdfs:Class ;
    rdfs:label "InfectiousAgentClass" ;
    rdfs:comment "Classes of agents or pathogens that transmit infectious diseases. Enumerated type." ;
    rdfs:subClassOf schema:Enumeration,
        schema:MedicalEnumeration,
        schema:MovedFromCore .

schema:InfectiousDisease a rdfs:Class ;
    rdfs:label "InfectiousDisease" ;
    rdfs:comment "An infectious disease is a clinically evident human disease resulting from the presence of pathogenic microbial agents, like pathogenic viruses, pathogenic bacteria, fungi, protozoa, multicellular parasites, and prions. To be considered an infectious disease, such pathogens are known to be able to cause this disease." ;
    rdfs:subClassOf schema:MedicalCondition,
        schema:MovedFromCore .

schema:Intangible a rdfs:Class ;
    rdfs:label "Intangible" ;
    rdfs:comment "A utility class that serves as the umbrella for a number of 'intangible' things such as quantities, structured values, etc." ;
    rdfs:subClassOf schema:MaintainedInCore,
        schema:Thing .

schema:IntegumentarySystem a rdfs:Class ;
    rdfs:label "IntegumentarySystem" ;
    rdfs:comment "The organ system that protects the body from various kinds of damage, such as loss of water or abrasion from outside, including the skin and its appendages (hair, scales, feathers, hooves, and nails)." ;
    rdfs:subClassOf schema:AnatomicalSystem,
        schema:CreatedInExtension .

schema:InvasivenessType a rdfs:Class ;
    rdfs:label "InvasivenessType" ;
    rdfs:comment "A categorization of invasiveness type of medical procedures." ;
    rdfs:subClassOf schema:CreatedInExtension,
        schema:MedicalEnumeration .

schema:Joint a rdfs:Class ;
    rdfs:label "Joint" ;
    rdfs:comment "The anatomical location at which two or more bones make contact." ;
    rdfs:subClassOf schema:AnatomicalStructure,
        schema:MovedFromCore .

schema:Kinesiotherapy a rdfs:Class ;
    rdfs:label "Kinesiotherapy" ;
    rdfs:comment "Also known as physical therapy or physiotherapy is a health care profession primarily concerned with the remediation of impairments and disabilities and the promotion of mobility, functional ability, quality of life and movement potential through examination, evaluation, diagnosis and physical intervention." ;
    rdfs:subClassOf schema:CreatedInExtension,
        schema:MedicalTherapy .

schema:LaboratoryResult a rdfs:Class ;
    rdfs:label "LaboratoryResult" ;
    rdfs:comment "Medical laboratory results resource" ;
    rdfs:subClassOf schema:ClinicalFinding,
        schema:CreatedInExtension .

schema:LaboratoryTest a rdfs:Class ;
    rdfs:label "LaboratoryTest" ;
    rdfs:comment "A quantitative or qualitative test of a substance to determine its components" ;
    rdfs:subClassOf schema:CreatedInExtension,
        schema:DiagnosticProcedure .

schema:LegalIssueHistory a rdfs:Class ;
    rdfs:label "LegalIssueHistory" ;
    rdfs:comment "All legal issue in history of a person" ;
    rdfs:subClassOf schema:CreatedInExtension,
        schema:SocialHistory .

schema:LifeEvent a rdfs:Class ;
    rdfs:label "LifeEvent" ;
    rdfs:comment "Any event happening in person's life." ;
    rdfs:subClassOf schema:CreatedInExtension,
        schema:MedicalEntity .

schema:LifestyleModification a rdfs:Class ;
    rdfs:label "LifestyleModification" ;
    rdfs:comment "A process of care involving exercise, changes to diet, fitness routines, and other lifestyle changes aimed at improving a health condition." ;
    rdfs:subClassOf schema:MedicalTherapy,
        schema:MovedFromCore .

schema:LifestyleOrHabits a rdfs:Class ;
    rdfs:label "LifestyleOrHabits" ;
    rdfs:comment "As a part of personal medical history, the lifestyle or habits data  consist of information behavior, lifestyles and habits features or risk factors in the living of the patient" ;
    rdfs:subClassOf schema:CreatedInExtension,
        schema:PersonalHistory .

schema:Ligament a rdfs:Class ;
    rdfs:label "Ligament" ;
    rdfs:comment "A short band of tough, flexible, fibrous connective tissue that functions to connect multiple bones, cartilages, and structurally support joints." ;
    rdfs:subClassOf schema:AnatomicalStructure,
        schema:MovedFromCore .

schema:LymphaticSystem a rdfs:Class ;
    rdfs:label "LymphaticSystem" ;
    rdfs:comment "The lymphatic system is part of the circulatory system, comprising a network of conduits called lymphatic vessels that carry a clear fluid called lymph directionally towards the heart." ;
    rdfs:subClassOf schema:CirculatorySystem,
        schema:CreatedInExtension .

schema:LymphaticVessel a rdfs:Class ;
    rdfs:label "LymphaticVessel" ;
    rdfs:comment "A type of blood vessel that specifically carries lymph fluid unidirectionally toward the heart." ;
    rdfs:subClassOf schema:MovedFromCore,
        schema:Vessel .

schema:MagneticResonanceImaging a rdfs:Class ;
    rdfs:label "MagneticResonanceImaging" ;
    rdfs:comment "Also known as MRI, is a technique for producing images of bodily organs by measuring the response of the atomic nuclei of body tissues to high-frequency radio waves when placed in a strong magnetic field." ;
    rdfs:subClassOf schema:CreatedInExtension,
        schema:MedicalImaging .

schema:MaintainedInCore a rdfs:Class ;
    rdfs:label "MaintainedInCore" ;
    rdfs:comment "A class of all items -although medical/health related, maintained in the schema core" ;
    rdfs:subClassOf schema:Thing .

schema:MaritalStatus a rdfs:Class ;
    rdfs:label "MaritalStatus" ;
    rdfs:comment "One's situation with regard to whether one is single, married, separated, divorced, or widowed." ;
    rdfs:subClassOf schema:CreatedInExtension,
        schema:SocialHistory .

schema:MaximumDoseSchedule a rdfs:Class ;
    rdfs:label "MaximumDoseSchedule" ;
    rdfs:comment "The maximum dosing schedule considered safe for a drug or supplement as recommended by an authority or by the drug/supplement's manufacturer. Capture the recommending authority in the recognizingAuthority property of MedicalEntity." ;
    rdfs:subClassOf schema:DoseSchedule,
        schema:MovedFromCore .

schema:MedicalAdmission a rdfs:Class ;
    rdfs:label "MedicalAdmission" ;
    rdfs:comment "Procedure consisting in taking a patient into a health care environment" ;
    rdfs:subClassOf schema:CreatedInExtension,
        schema:MedicalEncounter .

schema:MedicalAudience a rdfs:Class ;
    rdfs:label "MedicalAudience" ;
    rdfs:comment "Target audiences for medical web pages. Enumerated type." ;
    rdfs:subClassOf schema:Audience,
        schema:Enumeration,
        schema:MedicalEnumeration,
        schema:MovedFromCore,
        schema:PeopleAudience .

schema:MedicalAuscultation a rdfs:Class ;
    rdfs:label "MedicalAuscultation" ;
    rdfs:comment "The action of listening to sounds from the heart, lungs, or other organs, typically with a stethoscope, as a part of medical diagnosis." ;
    rdfs:subClassOf schema:CreatedInExtension,
        schema:PhysicalExam .

schema:MedicalBed a rdfs:Class ;
    rdfs:label "MedicalBed" ;
    rdfs:comment "A bed (as a physical thing) in a healthcare facility environment" ;
    rdfs:subClassOf schema:CreatedInExtension,
        schema:HealthFacility .

schema:MedicalCase a rdfs:Class ;
    rdfs:label "MedicalCase" ;
    rdfs:comment "A summary of all relevant and actionable information and instructions for a given patient in given time period." ;
    rdfs:subClassOf schema:CreatedInExtension,
        schema:MedicalRecord .

schema:MedicalCause a rdfs:Class ;
    rdfs:label "MedicalCause" ;
    rdfs:comment "The causative agent(s) that are responsible for the pathophysiologic process that eventually results in a medical condition, symptom or sign. In this schema, unless otherwise specified this is meant to be the proximate cause of the medical condition, symptom or sign. The proximate cause is defined as the causative agent that most directly results in the medical condition, symptom or sign. For example, the HIV virus could be considered a cause of AIDS. Or in a diagnostic context, if a patient fell and sustained a hip fracture and two days later sustained a pulmonary embolism which eventuated in a cardiac arrest, the cause of the cardiac arrest (the proximate cause) would be the pulmonary embolism and not the fall. Medical causes can include cardiovascular, chemical, dermatologic, endocrine, environmental, gastroenterologic, genetic, hematologic, gynecologic, iatrogenic, infectious, musculoskeletal, neurologic, nutritional, obstetric, oncologic, otolaryngologic, pharmacologic, psychiatric, pulmonary, renal, rheumatologic, toxic, traumatic, or urologic causes; medical conditions can be causes as well." ;
    rdfs:subClassOf schema:MedicalEntity,
        schema:MovedFromCore .

schema:MedicalCertificate a rdfs:Class ;
    rdfs:label "MedicalCertificate" ;
    rdfs:comment "Any certificate given to a person for healthcare purposes" ;
    rdfs:subClassOf schema:ClinicalDocument,
        schema:CreatedInExtension .

schema:MedicalClinic a rdfs:Class ;
    rdfs:label "MedicalClinic" ;
    rdfs:comment "A facility, often associated with a hospital or medical school, that is devoted to the specific diagnosis and/or healthcare. Previously limited to outpatients but with evolution it may be open to inpatients as well." ;
    rdfs:subClassOf schema:CreatedInExtension,
        schema:HealthFacility,
        schema:MedicalOrganization .

schema:MedicalCode a rdfs:Class ;
    rdfs:label "MedicalCode" ;
    rdfs:comment "A code for a medical entity." ;
    rdfs:subClassOf schema:MedicalIntangible,
        schema:MovedFromCore .

schema:MedicalCondition a rdfs:Class ;
    rdfs:label "MedicalCondition" ;
    rdfs:comment "Any condition of the human body that affects the normal functioning of a person, whether physically or mentally. Includes diseases, injuries, disabilities, disorders, syndromes, etc." ;
    rdfs:subClassOf schema:ClinicalFinding,
        schema:MovedFromCore .

schema:MedicalConditionStage a rdfs:Class ;
    rdfs:label "MedicalConditionStage" ;
    rdfs:comment "A stage of a medical condition, such as 'Stage IIIa'." ;
    rdfs:subClassOf schema:MedicalIntangible,
        schema:MovedFromCore .

schema:MedicalContraindication a rdfs:Class ;
    rdfs:label "MedicalContraindication" ;
    rdfs:comment "A condition or factor that serves as a reason to withhold a certain medical therapy. Contraindications can be absolute (there are no reasonable circumstances for undertaking a course of action) or relative (the patient is at higher risk of complications, but that these risks may be outweighed by other considerations or mitigated by other measures)." ;
    rdfs:subClassOf schema:MedicalEntity,
        schema:MovedFromCore .

schema:MedicalDepartment a rdfs:Class ;
    rdfs:label "MedicalDepartment" ;
    rdfs:comment "A health facility department. Typically named according the medical specialties. Eg. Internal medicine, Surgery, etc." ;
    rdfs:subClassOf schema:CreatedInExtension,
        schema:HealthFacility .

schema:MedicalDevice a rdfs:Class ;
    rdfs:label "MedicalDevice" ;
    rdfs:comment "Any object used in a medical capacity, such as to diagnose or treat a patient." ;
    rdfs:subClassOf schema:MedicalEntity,
        schema:MovedFromCore .

schema:MedicalDevicePurpose a rdfs:Class ;
    rdfs:label "MedicalDevicePurpose" ;
    rdfs:comment "Categories of medical devices, organized by the purpose or intended use of the device." ;
    rdfs:subClassOf schema:Enumeration,
        schema:MedicalEnumeration,
        schema:MovedFromCore .

schema:MedicalDischarge a rdfs:Class ;
    rdfs:label "MedicalDischarge" ;
    rdfs:comment "Procedure consisting in taking a patient out of a health care environment" ;
    rdfs:subClassOf schema:CreatedInExtension,
        schema:MedicalEncounter .

schema:MedicalEncounter a rdfs:Class ;
    rdfs:label "MedicalEncounter" ;
    rdfs:comment "An interaction between a patient and healthcare participant(s) for the purpose of providing patient service(s) or assessing the health status of a patient." ;
    rdfs:subClassOf schema:AdministrativeProcedure,
        schema:CreatedInExtension .

schema:MedicalEntity a rdfs:Class ;
    rdfs:label "MedicalEntity" ;
    rdfs:comment "The most generic type of entity related to health and the practice of medicine." ;
    rdfs:subClassOf schema:MovedFromCore,
        schema:Thing .

schema:MedicalEnumeration a rdfs:Class ;
    rdfs:label "MedicalEnumeration" ;
    rdfs:comment "Enumerations related to health and the practice of medicine: A concept that is used to attribute a quality to another concept, as a qualifier, a collection of items or a listing of all of the elements of a set in medicine practice." ;
    rdfs:subClassOf schema:Enumeration,
        schema:MedicalIntangible,
        schema:MovedFromCore .

schema:MedicalEvidenceLevel a rdfs:Class ;
    rdfs:label "MedicalEvidenceLevel" ;
    rdfs:comment "Level of evidence for a medical guideline. Enumerated type." ;
    rdfs:subClassOf schema:Enumeration,
        schema:MedicalEnumeration,
        schema:MovedFromCore .

schema:MedicalGuideline a rdfs:Class ;
    rdfs:label "MedicalGuideline" ;
    rdfs:comment "Any recommendation made by a standard society (e.g. ACC/AHA) or consensus statement that denotes how to diagnose and treat a particular condition. Note: this type should be used to tag the actual guideline recommendation; if the guideline recommendation occurs in a larger scholarly article, use MedicalScholarlyArticle to tag the overall article, not this type. Note also: the organization making the recommendation should be captured in the recognizingAuthority base property of MedicalEntity." ;
    rdfs:subClassOf schema:MedicalEntity,
        schema:MovedFromCore .

schema:MedicalGuidelineContraindication a rdfs:Class ;
    rdfs:label "MedicalGuidelineContraindication" ;
    rdfs:comment "A guideline contraindication that designates a process as harmful and where quality of the data supporting the contraindication is sound." ;
    rdfs:subClassOf schema:MedicalGuideline,
        schema:MovedFromCore .

schema:MedicalGuidelineRecommendation a rdfs:Class ;
    rdfs:label "MedicalGuidelineRecommendation" ;
    rdfs:comment "A guideline recommendation that is regarded as efficacious and where quality of the data supporting the recommendation is sound." ;
    rdfs:subClassOf schema:MedicalGuideline,
        schema:MovedFromCore .

schema:MedicalHistory a rdfs:Class ;
    rdfs:label "MedicalHistory" ;
    rdfs:comment "The medical history of a patient is information gained by a physician by asking specific questions through anamnesis procedure, either of the patient or of other people who know the person and can give suitable information, with the aim of obtaining information useful in formulating a diagnosis and providing medical care to the patient. " ;
    rdfs:subClassOf schema:CreatedInExtension,
        schema:MedicalEntity .

schema:MedicalImaging a rdfs:Class ;
    rdfs:label "MedicalImaging" ;
    rdfs:comment "A process of capturing, storing, manipulating, and displaying of images for a medical use" ;
    rdfs:subClassOf schema:CreatedInExtension,
        schema:DiagnosticProcedure .

schema:MedicalImagingTechnique a rdfs:Class ;
    rdfs:label "MedicalImagingTechnique" ;
    rdfs:comment "Any medical imaging modality typically used for diagnostic purposes. Enumerated type." ;
    rdfs:subClassOf schema:Enumeration,
        schema:MedicalEnumeration,
        schema:MovedFromCore .

schema:MedicalIndication a rdfs:Class ;
    rdfs:label "MedicalIndication" ;
    rdfs:comment "A condition or factor that indicates use of a medical therapy, including signs, symptoms, risk factors, anatomical states, etc." ;
    rdfs:subClassOf schema:MedicalEntity,
        schema:MovedFromCore .

schema:MedicalInspection a rdfs:Class ;
    rdfs:label "MedicalInspection" ;
    rdfs:comment "The thorough and unhurried visualization of the patient that requires the use of the naked eye." ;
    rdfs:subClassOf schema:CreatedInExtension,
        schema:PhysicalExam .

schema:MedicalIntangible a rdfs:Class ;
    rdfs:label "MedicalIntangible" ;
    rdfs:comment "A utility class that serves as the umbrella for a number of 'intangible' things in the medical space." ;
    rdfs:subClassOf schema:MedicalEntity,
        schema:MovedFromCore .

schema:MedicalIntervention a rdfs:Class ;
    rdfs:label "MedicalIntervention" ;
    rdfs:comment "Any examination, treatment, or other act having preventive, diagnostic, therapeutic or rehabilitative aims and which is carried out by a physician or other health care provider (Declaration on the Promotion of Rights of Patients in Europe, WHO, Amsterdam 1994). Typically-but not limited to, the intervention is set of different procedures for a common care purpose." ;
    rdfs:subClassOf schema:CreatedInExtension,
        schema:MedicalEntity .

schema:MedicalObservationalStudy a rdfs:Class ;
    rdfs:label "MedicalObservationalStudy" ;
    rdfs:comment "An observational study is a type of medical study that attempts to infer the possible effect of a treatment through observation of a cohort of subjects over a period of time. In an observational study, the assignment of subjects into treatment groups versus control groups is outside the control of the investigator. This is in contrast with controlled studies, such as the randomized controlled trials represented by MedicalTrial, where each subject is randomly assigned to a treatment group or a control group before the start of the treatment." ;
    rdfs:subClassOf schema:MedicalStudy,
        schema:MovedFromCore .

schema:MedicalObservationalStudyDesign a rdfs:Class ;
    rdfs:label "MedicalObservationalStudyDesign" ;
    rdfs:comment "Design models for observational medical studies. Enumerated type." ;
    rdfs:subClassOf schema:Enumeration,
        schema:MedicalEnumeration,
        schema:MovedFromCore .

schema:MedicalOrder a rdfs:Class ;
    rdfs:label "MedicalOrder" ;
    rdfs:comment "Written orders by medical providers to other members of the health care team or to the patient." ;
    rdfs:subClassOf schema:ClinicalDocument,
        schema:CreatedInExtension .

schema:MedicalOrganization a rdfs:Class ;
    rdfs:label "MedicalOrganization" ;
    rdfs:comment "A medical organization, such as a doctor's office or clinic." ;
    rdfs:subClassOf schema:LocalBusiness,
        schema:MovedFromCore .

schema:MedicalPalpation a rdfs:Class ;
    rdfs:label "MedicalPalpation" ;
    rdfs:comment "The process of using your hands to examine the body, especially while perceiving/diagnosing a disease or illness." ;
    rdfs:subClassOf schema:CreatedInExtension,
        schema:PhysicalExam .

schema:MedicalPercussion a rdfs:Class ;
    rdfs:label "MedicalPercussion" ;
    rdfs:comment "A method of tapping on a surface to determine the underlying structure, and is used in clinical examinations to assess the condition of the thorax or abdomen" ;
    rdfs:subClassOf schema:CreatedInExtension,
        schema:PhysicalExam .

schema:MedicalPrescription a rdfs:Class ;
    rdfs:label "MedicalPrescription" ;
    rdfs:comment "Also known as a medical order, the prescription is a written document from a healthcare provider to the patient bearing the information about the medicine or therapy to be used as a treatment." ;
    rdfs:subClassOf schema:ClinicalDocument,
        schema:CreatedInExtension .

schema:MedicalProcedure a rdfs:Class ;
    rdfs:label "MedicalProcedure" ;
    rdfs:comment "A process of care used in either a diagnostic, therapeutic, preventive or palliative capacity that relies on invasive (surgical), non-invasive, or other techniques." ;
    rdfs:subClassOf schema:MedicalEntity,
        schema:MovedFromCore .

schema:MedicalProcedureActivity a rdfs:Class ;
    rdfs:label "MedicalProcedureActivity" ;
    rdfs:comment "A medical procedure activity" ;
    rdfs:subClassOf schema:CreatedInCore,
        schema:MedicalProcedure .

schema:MedicalProcedurePhase a rdfs:Class ;
    rdfs:label "MedicalProcedurePhase" ;
    rdfs:comment "A medical procedure phase" ;
    rdfs:subClassOf schema:CreatedInCore,
        schema:MedicalProcedure .

schema:MedicalProcedureType a rdfs:Class ;
    rdfs:label "MedicalProcedureType" ;
    rdfs:comment "An enumeration that describes different types of medical procedures." ;
    rdfs:subClassOf schema:Enumeration,
        schema:MedicalEnumeration,
        schema:MovedFromCore .

schema:MedicalRecord a rdfs:Class ;
    rdfs:label "MedicalRecord" ;
    rdfs:comment "Any kind of patient related information record. This can be paper or digital" ;
    rdfs:subClassOf schema:CreatedInExtension,
        schema:MedicalEntity .

schema:MedicalReport a rdfs:Class ;
    rdfs:label "MedicalReport" ;
    rdfs:comment "Any kind of report with patient information" ;
    rdfs:subClassOf schema:ClinicalDocument,
        schema:CreatedInExtension .

schema:MedicalRequest a rdfs:Class ;
    rdfs:label "MedicalRequest" ;
    rdfs:comment "A medical request for medical information of a patient, or an exam/procedure to be done, or something else. Specifically a procedure request is a record of a request for a procedure to be performed. It can be used to represent a procedure that is planned, that is proposed, or that is ordered." ;
    rdfs:subClassOf schema:ClinicalDocument,
        schema:CreatedInExtension .

schema:MedicalRiskCalculator a rdfs:Class ;
    rdfs:label "MedicalRiskCalculator" ;
    rdfs:comment "A complex mathematical calculation requiring an online calculator, used to assess prognosis. Note: use the url property of Thing to record any URLs for online calculators." ;
    rdfs:subClassOf schema:MedicalRiskEstimator,
        schema:MovedFromCore .

schema:MedicalRiskEstimator a rdfs:Class ;
    rdfs:label "MedicalRiskEstimator" ;
    rdfs:comment "Any rule set or interactive tool for estimating the risk of developing a complication or condition." ;
    rdfs:subClassOf schema:MedicalEntity,
        schema:MovedFromCore .

schema:MedicalRiskFactor a rdfs:Class ;
    rdfs:label "MedicalRiskFactor" ;
    rdfs:comment "A risk factor is anything that increases a person's likelihood of developing or contracting a disease, medical condition, or complication." ;
    rdfs:subClassOf schema:MedicalEntity,
        schema:MovedFromCore .

schema:MedicalRiskScore a rdfs:Class ;
    rdfs:label "MedicalRiskScore" ;
    rdfs:comment "A simple system that adds up the number of risk factors to yield a score that is associated with prognosis, e.g. CHAD score, TIMI risk score." ;
    rdfs:subClassOf schema:MedicalRiskEstimator,
        schema:MovedFromCore .

schema:MedicalRoom a rdfs:Class ;
    rdfs:label "MedicalRoom" ;
    rdfs:comment "A room (as a physical space) in a healthcare facility environment" ;
    rdfs:subClassOf schema:CreatedInExtension,
        schema:HealthFacility .

schema:MedicalScholarlyArticle a rdfs:Class ;
    rdfs:label "MedicalScholarlyArticle" ;
    rdfs:comment "A scholarly article in the medical domain." ;
    rdfs:subClassOf schema:MovedFromCore,
        schema:ScholarlyArticle .

schema:MedicalScore a rdfs:Class ;
    rdfs:label "MedicalScore" ;
    rdfs:comment "The number of points achieved by a individual through a systematic evaluation." ;
    rdfs:subClassOf schema:CreatedInExtension,
        schema:MedicalEntity .

schema:MedicalSign a rdfs:Class ;
    rdfs:label "MedicalSign" ;
    rdfs:comment "Any physical manifestation of a person's medical condition discoverable by objective diagnostic tests or physical examination." ;
    rdfs:subClassOf schema:MedicalSignOrSymptom,
        schema:MovedFromCore .

schema:MedicalSignOrSymptom a rdfs:Class ;
    rdfs:label "MedicalSignOrSymptom" ;
    rdfs:comment "Any feature associated or not with a medical condition. In medicine a symptom is generally subjective while a sign is objective." ;
    rdfs:subClassOf schema:MedicalCondition,
        schema:MovedFromCore .

schema:MedicalSpecialty a rdfs:Class ;
    rdfs:label "MedicalSpecialty" ;
    rdfs:comment "Any specific branch of medical science or practice. Medical specialities include clinical specialties that pertain to particular organ systems and their respective disease states, as well as allied health specialties. Enumerated type." ;
    rdfs:subClassOf schema:Enumeration,
        schema:MedicalEnumeration,
        schema:MovedFromCore,
        schema:Specialty .

schema:MedicalSpecimen a rdfs:Class ;
    rdfs:label "MedicalSpecimen" ;
    rdfs:comment "Material (structure, substance, device) removed from a source (patient, donor, physical location, product)" ;
    rdfs:subClassOf schema:CreatedInExtension,
        schema:MedicalEntity .

schema:MedicalSpecimenDonor a rdfs:Class ;
    rdfs:label "MedicalSpecimenDonor" ;
    rdfs:comment "Medical Specimen Donor" ;
    rdfs:subClassOf <http://schema.org#MedicalSpecimen>,
        schema:CreatedInExtension .

schema:MedicalSpecimenReceiver a rdfs:Class ;
    rdfs:label "MedicalSpecimenReceiver" ;
    rdfs:comment "Medical Specimen Receiver" ;
    rdfs:subClassOf <http://schema.org#MedicalSpecimen>,
        schema:CreatedInExtension .

schema:MedicalStay a rdfs:Class ;
    rdfs:label "MedicalStay" ;
    rdfs:comment "Procedure consisting in taking a patient into a healthcare environment as inpatient (hospitalization)" ;
    rdfs:subClassOf schema:CreatedInExtension,
        schema:MedicalEncounter .

schema:MedicalStudy a rdfs:Class ;
    rdfs:label "MedicalStudy" ;
    rdfs:comment "A medical study is an umbrella type covering all kinds of research studies relating to human medicine or health, including observational studies and interventional trials and registries, randomized, controlled or not. When the specific type of study is known, use one of the extensions of this type, such as MedicalTrial or MedicalObservationalStudy. Also, note that this type should be used to mark up data that describes the study itself; to tag an article that publishes the results of a study, use MedicalScholarlyArticle. Note: use the code property of MedicalEntity to store study IDs, e.g. clinicaltrials.gov ID." ;
    rdfs:subClassOf schema:MedicalEntity,
        schema:MovedFromCore .

schema:MedicalStudyStatus a rdfs:Class ;
    rdfs:label "MedicalStudyStatus" ;
    rdfs:comment "The status of a medical study. Enumerated type." ;
    rdfs:subClassOf schema:Enumeration,
        schema:MedicalEnumeration,
        schema:MovedFromCore .

schema:MedicalSubSpeciality a rdfs:Class ;
    rdfs:label "MedicalSubSpeciality" ;
    rdfs:comment "A subspecialty (or sub-specialty) in medicine is a branch of medical specialty." ;
    rdfs:subClassOf schema:CreatedInExtension,
        schema:MedicalSpecialty .

schema:MedicalSymptom a rdfs:Class ;
    rdfs:label "MedicalSymptom" ;
    rdfs:comment "Any complain sensed and expressed by the patient (therefore defined as subjective)  like stomachache, lower-back pain, or fatigue." ;
    rdfs:subClassOf schema:MedicalSignOrSymptom,
        schema:MovedFromCore .

schema:MedicalTest a rdfs:Class ;
    rdfs:label "MedicalTest" ;
    rdfs:comment "Any medical test, typically performed for diagnostic purposes." ;
    rdfs:subClassOf schema:MedicalEntity,
        schema:MovedFromCore .

schema:MedicalTestPanel a rdfs:Class ;
    rdfs:label "MedicalTestPanel" ;
    rdfs:comment "Any collection of tests commonly ordered together." ;
    rdfs:subClassOf schema:MedicalTest,
        schema:MovedFromCore .

schema:MedicalTherapy a rdfs:Class ;
    rdfs:label "MedicalTherapy" ;
    rdfs:comment "Any medical intervention designed to prevent, treat, and cure human diseases and medical conditions, including both curative and palliative therapies. Medical therapies are typically processes of care relying upon pharmacotherapy, behavioral therapy, supportive therapy (with fluid or nutrition for example), or detoxification (e.g. hemodialysis) aimed at improving or preventing a health condition." ;
    rdfs:subClassOf schema:MovedFromCore,
        schema:TherapeuticProcedure .

schema:MedicalTransfer a rdfs:Class ;
    rdfs:label "MedicalTransfer" ;
    rdfs:comment "Procedure consisting in transferring a patient from a health care environment to another" ;
    rdfs:subClassOf schema:CreatedInExtension,
        schema:MedicalEncounter .

schema:MedicalTriage a rdfs:Class ;
    rdfs:label "MedicalTriage" ;
    rdfs:comment "Procedure which consist in selecting patients by priority of care need, typically at hospital emergency unit" ;
    rdfs:subClassOf schema:AdministrativeProcedure,
        schema:CreatedInExtension .

schema:MedicalTrial a rdfs:Class ;
    rdfs:label "MedicalTrial" ;
    rdfs:comment "A medical trial is a type of medical study that uses scientific process used to compare the safety and efficacy of medical therapies or medical procedures. In general, medical trials are controlled and subjects are allocated at random to the different treatment and/or control groups." ;
    rdfs:subClassOf schema:MedicalStudy,
        schema:MovedFromCore .

schema:MedicalTrialDesign a rdfs:Class ;
    rdfs:label "MedicalTrialDesign" ;
    rdfs:comment "Design models for medical trials. Enumerated type." ;
    rdfs:subClassOf schema:Enumeration,
        schema:MedicalEnumeration,
        schema:MovedFromCore .

schema:MedicalUnit a rdfs:Class ;
    rdfs:label "MedicalUnit" ;
    rdfs:comment "A health facility Unit. eg Nephrology unit, Dialysis unit etc." ;
    rdfs:subClassOf schema:CreatedInExtension,
        schema:HealthFacility .

schema:MedicalVisit a rdfs:Class ;
    rdfs:label "MedicalVisit" ;
    rdfs:comment "Procedure consisting in having a patient visiting a health care environment as outpatient" ;
    rdfs:subClassOf schema:CreatedInExtension,
        schema:MedicalEncounter .

schema:MedicalWard a rdfs:Class ;
    rdfs:label "MedicalWard" ;
    rdfs:comment "A block forming a division of a hospital (or a suite of rooms) shared by patients who need a similar kind of care" ;
    rdfs:subClassOf schema:CreatedInExtension,
        schema:HealthFacility .

schema:MedicalWebPage a rdfs:Class ;
    rdfs:label "MedicalWebPage" ;
    rdfs:comment "A web page that provides medical information." ;
    rdfs:subClassOf schema:MovedFromCore,
        schema:WebPage .

schema:MedicationUseHistory a rdfs:Class ;
    rdfs:label "MedicationUseHistory" ;
    rdfs:comment "The description of medications use for a person" ;
    rdfs:subClassOf schema:CreatedInExtension,
        schema:PersonalHistory .

schema:MedicineSystem a rdfs:Class ;
    rdfs:label "MedicineSystem" ;
    rdfs:comment "Systems of medical practice." ;
    rdfs:subClassOf schema:Enumeration,
        schema:MedicalEnumeration,
        schema:MovedFromCore .

schema:Menopause a rdfs:Class ;
    rdfs:label "Menopause" ;
    rdfs:comment "The period in a woman's life when menstruation ceases." ;
    rdfs:subClassOf schema:CreatedInExtension,
        schema:GynObsHistory .

schema:Menstruation a rdfs:Class ;
    rdfs:label "Menstruation" ;
    rdfs:comment "The periodic discharge of blood and mucosal tissue (the endometrium) from the uterus and vagina." ;
    rdfs:subClassOf schema:CreatedInExtension,
        schema:GynObsHistory .

schema:MentalHealthHistory a rdfs:Class ;
    rdfs:label "MentalHealthHistory" ;
    rdfs:comment "The description of mental health disorder or conditions for a person" ;
    rdfs:subClassOf schema:CreatedInExtension,
        schema:PersonalHistory .

schema:MorbidityEvent a rdfs:Class ;
    rdfs:label "MorbidityEvent" ;
    rdfs:comment "The state of being  diseased or unhealthy for a person or within a population" ;
    rdfs:subClassOf schema:CreatedInExtension,
        schema:LifeEvent .

schema:MovedFromCore a rdfs:Class ;
    rdfs:label "MovedFromCore" ;
    rdfs:comment "A class of all items moved from the schema core to the extension" ;
    rdfs:subClassOf schema:Thing .

schema:Muscle a rdfs:Class ;
    rdfs:label "Muscle" ;
    rdfs:comment "A muscle is an anatomical structure consisting of a contractile form of tissue that animals use to effect movement." ;
    rdfs:subClassOf schema:AnatomicalStructure,
        schema:MovedFromCore .

schema:MuscularSystem a rdfs:Class ;
    rdfs:label "MuscularSystem" ;
    rdfs:comment " An organ system consisting of skeletal, smooth and cardiac muscles." ;
    rdfs:subClassOf schema:CreatedInExtension,
        schema:MusculoskeletalSystem .

schema:MusculoskeletalSystem a rdfs:Class ;
    rdfs:label "MusculoskeletalSystem" ;
    rdfs:comment "The human musculoskeletal system (also known as the locomotor system, and previously the activity system) is an organ system that gives humans (and many animal species) the ability to move using the muscular and skeletal systems." ;
    rdfs:subClassOf schema:AnatomicalSystem,
        schema:CreatedInExtension .

schema:Nerve a rdfs:Class ;
    rdfs:label "Nerve" ;
    rdfs:comment "A common pathway for the electrochemical nerve impulses that are transmitted along each of the axons." ;
    rdfs:subClassOf schema:AnatomicalStructure,
        schema:MovedFromCore .

schema:NervousSystem a rdfs:Class ;
    rdfs:label "NervousSystem" ;
    rdfs:comment "The part of an animal's body that coordinates its voluntary and involuntary actions and transmits signals between different parts of its body. In most animal species it consists of two main parts, the central nervous system (CNS) and the peripheral nervous system (PNS)." ;
    rdfs:subClassOf schema:AnatomicalSystem,
        schema:CreatedInExtension .

schema:NuclearMedicineImaging a rdfs:Class ;
    rdfs:label "NuclearMedicineImaging" ;
    rdfs:comment "The branch of medicine that deals with the use of radioactive substances in research, diagnosis, and treatment." ;
    rdfs:subClassOf schema:CreatedInExtension,
        schema:MedicalImaging .

schema:NutritionInformation a rdfs:Class ;
    rdfs:label "NutritionInformation" ;
    rdfs:comment "Nutritional information about the recipe." ;
    rdfs:subClassOf schema:MovedFromCore,
        schema:StructuredValue .

schema:ObstetricSurgery a rdfs:Class ;
    rdfs:label "ObstetricSurgery" ;
    rdfs:comment "A surgical procedure related to the care of women during or after pregnancy." ;
    rdfs:subClassOf schema:CreatedInExtension,
        schema:SurgicalProcedure .

schema:OccupationalHistory a rdfs:Class ;
    rdfs:label "OccupationalHistory" ;
    rdfs:comment "A part of the health history in which questions are asked about the person's occupation, source of income, effects of the work on the worker's health or the worker's health on the job, the duration of the job, and to what degree the occupation satisfies the person." ;
    rdfs:subClassOf schema:CreatedInExtension,
        schema:SocialHistory .

schema:OnsetMode a rdfs:Class ;
    rdfs:label "OnsetMode" ;
    rdfs:comment "Description of how the medical condition started." ;
    rdfs:subClassOf schema:CreatedInExtension,
        schema:MedicalEnumeration .

schema:Optician a rdfs:Class ;
    rdfs:label "Optician" ;
    rdfs:comment "A store that sells reading glasses and similar devices for improving vision." ;
    rdfs:subClassOf schema:HealthFacility,
        schema:MedicalOrganization,
        schema:MovedFromCore .

schema:OralTemperature a rdfs:Class ;
    rdfs:label "OralTemperature" ;
    rdfs:comment "Human body temperature taken from oral region (mouth)" ;
    rdfs:subClassOf schema:BodyTemperature,
        schema:CreatedInExtension .

schema:Oxygenotherapy a rdfs:Class ;
    rdfs:label "Oxygenotherapy" ;
    rdfs:comment "Oxygen therapy is the administration of oxygen as a medical intervention, which can be for a variety of purposes in both chronic and acute patient care" ;
    rdfs:subClassOf schema:CreatedInExtension,
        schema:MedicalTherapy .

schema:PHR a rdfs:Class ;
    rdfs:label "PHR" ;
    rdfs:comment "The Personal Health Record (PHR) is an electronic record of health-related information on an individual that conforms to nationally recognized interoperability standards and that can be drawn from multiple sources while being managed, shared, and controlled by the individual.Source: US NAHIT" ;
    rdfs:subClassOf schema:CreatedInExtension,
        schema:MedicalRecord .

schema:PalliativeProcedure a rdfs:Class ;
    rdfs:label "PalliativeProcedure" ;
    rdfs:comment "A medical procedure intended primarily for palliative purposes, aimed at relieving the symptoms of an underlying health condition." ;
    rdfs:subClassOf schema:MedicalProcedure,
        schema:MedicalTherapy,
        schema:MovedFromCore .

schema:PastMedicalHistory a rdfs:Class ;
    rdfs:label "PastMedicalHistory" ;
    rdfs:comment "The total sum of a patient's health status and morbidity events prior to the presenting problem" ;
    rdfs:subClassOf schema:CreatedInExtension,
        schema:PersonalHistory .

schema:PathologyTest a rdfs:Class ;
    rdfs:label "PathologyTest" ;
    rdfs:comment "A medical test performed by a laboratory that typically involves examination of a tissue sample by a pathologist." ;
    rdfs:subClassOf schema:MedicalTest,
        schema:MovedFromCore .

schema:Patient a rdfs:Class ;
    rdfs:label "Patient" ;
    rdfs:comment "A patient is any person recipient of health care services." ;
    rdfs:subClassOf schema:MedicalAudience,
        schema:MovedFromCore,
        schema:Person .

schema:PersonalHistory a rdfs:Class ;
    rdfs:label "PersonalHistory" ;
    rdfs:comment "In medicine, as a part of medical history, the personal history consist of information about disorders the patient have suffered, but also all other information about health determinants for the patient." ;
    rdfs:subClassOf schema:CreatedInExtension,
        schema:MedicalHistory .

schema:PharmaceuticalSubstance a rdfs:Class ;
    rdfs:label "PharmaceuticalSubstance" ;
    rdfs:comment "Any chemical substance formulated or compounded as single active ingredient or in combination of other pharmacologically active substance, intended for internal, or external or for use in the medical diagnosis, cure, treatment, or prevention of disease" ;
    rdfs:subClassOf schema:ChemicalSubstance,
        schema:CreatedInExtension .

schema:Pharmacotherapy a rdfs:Class ;
    rdfs:label "Pharmacotherapy" ;
    rdfs:comment "Pharmacotherapy or drug therapy or medication is the treatment of disease through the administration of drugs." ;
    rdfs:subClassOf schema:CreatedInExtension,
        schema:MedicalTherapy .

schema:Pharmacy a rdfs:Class ;
    rdfs:label "Pharmacy" ;
    rdfs:comment "A pharmacy or drugstore." ;
    rdfs:subClassOf schema:MedicalOrganization,
        schema:MovedFromCore .

schema:Phototherapy a rdfs:Class ;
    rdfs:label "Phototherapy" ;
    rdfs:comment "Also known as light therapy or classically referred to as heliotherapy, consists of exposure to daylight or to specific wavelengths of light using polychromatic polarised light, lasers, light-emitting diodes, fluorescent lamps, dichroic lamps or very bright, full-spectrum light, usually controlled with various devices." ;
    rdfs:subClassOf schema:CreatedInExtension,
        schema:MedicalTherapy .

schema:PhysicalActivity a rdfs:Class ;
    rdfs:label "PhysicalActivity" ;
    rdfs:comment "Any bodily activity that enhances or maintains physical fitness and overall health and wellness. Includes activity that is part of daily living and routine, structured exercise, and exercise prescribed as part of a medical treatment or recovery plan." ;
    rdfs:subClassOf schema:LifestyleModification,
        schema:MovedFromCore .

schema:PhysicalActivityCategory a rdfs:Class ;
    rdfs:label "PhysicalActivityCategory" ;
    rdfs:comment "Categories of physical activity, organized by physiologic classification." ;
    rdfs:subClassOf schema:Enumeration,
        schema:MedicalEnumeration,
        schema:MovedFromCore .

schema:PhysicalExam a rdfs:Class ;
    rdfs:label "PhysicalExam" ;
    rdfs:comment "A type of physical examination of a patient performed by a physician. " ;
    rdfs:subClassOf schema:MedicalProcedure,
        schema:MovedFromCore .

schema:PhysicalTherapy a rdfs:Class ;
    rdfs:label "PhysicalTherapy" ;
    rdfs:comment "A process of progressive physical care and rehabilitation aimed at improving a health condition." ;
    rdfs:subClassOf schema:MedicalTherapy,
        schema:MovedFromCore .

schema:Physician a rdfs:Class ;
    rdfs:label "Physician" ;
    rdfs:comment "A doctor's office." ;
    rdfs:subClassOf schema:MedicalOrganization,
        schema:MovedFromCore .

schema:PhysiologicalEntity a rdfs:Class ;
    rdfs:label "PhysiologicalEntity" ;
    rdfs:comment "Any entity describing how organisms, organ systems, organs, cells, and bio-molecules carry out the chemical or physical functions that exist in a living system." ;
    rdfs:subClassOf schema:CreatedInExtension,
        schema:MedicalEntity .

schema:PlasticSurgeryProcedure a rdfs:Class ;
    rdfs:label "PlasticSurgeryProcedure" ;
    rdfs:comment "The process of reconstructing or repairing parts of the body by the transfer of tissue, either in the treatment of injury or for cosmetic reasons." ;
    rdfs:subClassOf schema:CreatedInExtension,
        schema:SurgicalProcedure .

schema:Pregnancy a rdfs:Class ;
    rdfs:label "Pregnancy" ;
    rdfs:comment "The period from conception to birth. Can also refer to the condition of a woman or female animal that is going to have a baby or babies. This is regardless to the outcome" ;
    rdfs:subClassOf schema:ClinicalFinding,
        schema:CreatedInExtension .

schema:PrescribingProcedure a rdfs:Class ;
    rdfs:label "PrescribingProcedure" ;
    rdfs:comment "Any procedure which consist in prescribing a medicine or other treatment designed to prevent disease or ill health." ;
    rdfs:subClassOf schema:CreatedInExtension,
        schema:TherapeuticProcedure .

schema:PreventionIndication a rdfs:Class ;
    rdfs:label "PreventionIndication" ;
    rdfs:comment "An indication for preventing an underlying condition, symptom, etc." ;
    rdfs:subClassOf schema:MedicalIndication,
        schema:MovedFromCore .

schema:PreventiveProcedure a rdfs:Class ;
    rdfs:label "PreventiveProcedure" ;
    rdfs:comment "Any procedure or any medicine or other treatment designed to prevent disease or ill health." ;
    rdfs:subClassOf schema:CreatedInExtension,
        schema:TherapeuticProcedure .

schema:PsychologicalTreatment a rdfs:Class ;
    rdfs:label "PsychologicalTreatment" ;
    rdfs:comment "A process of care relying upon counseling, dialogue and communication  aimed at improving a mental health condition without use of drugs." ;
    rdfs:subClassOf schema:MovedFromCore,
        schema:TherapeuticProcedure .

schema:Psychotherapy a rdfs:Class ;
    rdfs:label "Psychotherapy" ;
    rdfs:comment " A general term for treatment of mental health problems by a mental health services provider: a psychiatrist (who only can also prescribe drugs), psychologist, social counselor, etc." ;
    rdfs:subClassOf schema:CreatedInExtension,
        schema:MedicalTherapy .

schema:Pulse a rdfs:Class ;
    rdfs:label "Pulse" ;
    rdfs:comment "In medicine, one's pulse represents the tactile arterial palpation of the heartbeat by trained fingertips. " ;
    rdfs:subClassOf schema:CreatedInExtension,
        schema:MedicalSign .

schema:Race a rdfs:Class ;
    rdfs:label "Race" ;
    rdfs:comment "An arbitrary classification of a taxonomic group that is a division of a species." ;
    rdfs:subClassOf schema:CreatedInExtension,
        schema:SocialHistory .

schema:RadiationTherapy a rdfs:Class ;
    rdfs:label "RadiationTherapy" ;
    rdfs:comment "A process of care using radiation aimed at improving a health condition." ;
    rdfs:subClassOf schema:MedicalTherapy,
        schema:MovedFromCore .

schema:Radiography a rdfs:Class ;
    rdfs:label "Radiography" ;
    rdfs:comment "Radiography is an imaging technique that uses electromagnetic radiation other than visible light, especially X-rays, to view the internal structure of a non-uniformly composed and opaque object such as the human body. " ;
    rdfs:subClassOf schema:CreatedInExtension,
        schema:MedicalImaging .

schema:Radiotherapy a rdfs:Class ;
    rdfs:label "Radiotherapy" ;
    rdfs:comment "The treatment of disease, especially cancer, using X-rays or similar forms of radiation." ;
    rdfs:subClassOf schema:CreatedInExtension,
        schema:MedicalTherapy .

schema:Recipe a rdfs:Class ;
    rdfs:label "Recipe" ;
    rdfs:comment "A recipe." ;
    rdfs:subClassOf schema:CreativeWork,
        schema:MovedFromCore .

schema:RecommendedDoseSchedule a rdfs:Class ;
    rdfs:label "RecommendedDoseSchedule" ;
    rdfs:comment "A recommended dosing schedule for a drug or supplement as prescribed or recommended by an authority or by the drug/supplement's manufacturer. Capture the recommending authority in the recognizingAuthority property of MedicalEntity." ;
    rdfs:subClassOf schema:DoseSchedule,
        schema:MovedFromCore .

schema:RecreationalHistory a rdfs:Class ;
    rdfs:label "RecreationalHistory" ;
    rdfs:comment "Description of activity history of a person during his leisure or recreation time. This is a part of medical history describing the physical activity of a person." ;
    rdfs:subClassOf schema:CreatedInExtension,
        schema:SocialHistory .

schema:RectalTemperature a rdfs:Class ;
    rdfs:label "RectalTemperature" ;
    rdfs:comment "Human body temperature taken at rectal region (anal)" ;
    rdfs:subClassOf schema:BodyTemperature,
        schema:CreatedInExtension .

schema:Refill a rdfs:Class ;
    rdfs:label "Refill" ;
    rdfs:comment "A prescription section, that shows many times you can get more of your medicine without going back to see your doctor." ;
    rdfs:subClassOf schema:CreatedInExtension,
        schema:MedicalPrescription .

schema:ReligionGroup a rdfs:Class ;
    rdfs:label "ReligionGroup" ;
    rdfs:comment "A group of people characterized by the practice of a common religion." ;
    rdfs:subClassOf schema:CreatedInExtension,
        schema:SocialHistory .

schema:ReligiousBelief a rdfs:Class ;
    rdfs:label "ReligiousBelief" ;
    rdfs:comment "A strong belief in a supernatural power or powers that control human destiny." ;
    rdfs:subClassOf schema:CreatedInExtension,
        schema:ReligionGroup .

schema:ReportedDoseSchedule a rdfs:Class ;
    rdfs:label "ReportedDoseSchedule" ;
    rdfs:comment "A patient-reported or observed dosing schedule for a drug or supplement." ;
    rdfs:subClassOf schema:DoseSchedule,
        schema:MovedFromCore .

schema:ReproductiveSystem a rdfs:Class ;
    rdfs:label "ReproductiveSystem" ;
    rdfs:comment "A system of sex organs within an organism which work together for the purpose of sexual reproduction. It comprises the sex organs, such as ovaries, fallopian tubes, uterus, vagina, mammary glands, testes, vas deferens, seminal vesicles and prostate" ;
    rdfs:subClassOf schema:AnatomicalSystem,
        schema:CreatedInExtension .

schema:ResearchPersonnel a rdfs:Class ;
    rdfs:label "ResearchPersonnel" ;
    rdfs:comment "People engaged in research in healthcare environment." ;
    rdfs:subClassOf schema:CreatedInExtension,
        schema:HealthcareProfessional .

schema:ResidenceHistory a rdfs:Class ;
    rdfs:label "ResidenceHistory" ;
    rdfs:comment "History of residence addresses change for a person" ;
    rdfs:subClassOf schema:CreatedInExtension,
        schema:SocialHistory .

schema:RespirationRate a rdfs:Class ;
    rdfs:label "RespirationRate" ;
    rdfs:comment "The respiratory rate (RR), also known as the respiration rate, ventilation rate, ventilatory rate, ventilation frequency (Vf), respiration frequency (Rf), pulmonary ventilation rate, or breathing frequency, is the rate (frequency) of ventilation, that is, the number of breaths (inhalation-exhalation cycles) taken within a set amount of time (typically 60 seconds). " ;
    rdfs:subClassOf schema:CreatedInExtension,
        schema:VitalSign .

schema:RespiratorySystem a rdfs:Class ;
    rdfs:label "RespiratorySystem" ;
    rdfs:comment "A biological system consisting of specific organs and structures used for the process of respiration in an organism. The respiratory system is involved in the intake and exchange of oxygen and carbon dioxide between an organism and the environment." ;
    rdfs:subClassOf schema:AnatomicalSystem,
        schema:CreatedInExtension .

schema:ScholarlyArticle a rdfs:Class ;
    rdfs:label "ScholarlyArticle" ;
    rdfs:comment "A scholarly article." ;
    rdfs:subClassOf schema:Article,
        schema:MaintainedInCore .

schema:Severity a rdfs:Class ;
    rdfs:label "Severity" ;
    rdfs:comment "Intensity quantification or scoring of illness or a medical condition" ;
    rdfs:subClassOf schema:CreatedInExtension,
        schema:MedicalEnumeration .

schema:SexualBehaviour a rdfs:Class ;
    rdfs:label "SexualBehaviour" ;
    rdfs:comment "The history describing the capacity to have erotic experiences and responses. Human sexuality may also involve a person's sexual attraction to another person" ;
    rdfs:subClassOf schema:CreatedInExtension,
        schema:SocialHistory .

schema:SkeletalSystem a rdfs:Class ;
    rdfs:label "SkeletalSystem" ;
    rdfs:comment "The internal framework of the body composed of bones" ;
    rdfs:subClassOf schema:CreatedInExtension,
        schema:MusculoskeletalSystem .

schema:Smoking a rdfs:Class ;
    rdfs:label "Smoking" ;
    rdfs:comment "The quantification or description of smoking habit for the person" ;
    rdfs:subClassOf schema:CreatedInExtension,
        schema:LifestyleOrHabits .

schema:SocialHistory a rdfs:Class ;
    rdfs:label "SocialHistory" ;
    rdfs:comment "A portion of the medical history addressing familial, occupational, and recreational aspects of the patient's personal life that have the potential to be clinically significant." ;
    rdfs:subClassOf schema:CreatedInExtension,
        schema:PersonalHistory .

schema:Specialty a rdfs:Class ;
    rdfs:label "Specialty" ;
    rdfs:comment "Any branch of a field in which people typically develop specific expertise, usually after significant study, time, and effort." ;
    rdfs:subClassOf schema:Enumeration,
        schema:MaintainedInCore .

schema:Substance a rdfs:Class ;
    rdfs:label "Substance" ;
    rdfs:comment "Any matter of defined composition that has discrete existence, whose origin may be biological, mineral or chemical." ;
    rdfs:subClassOf schema:CreatedInExtension,
        schema:MedicalEntity .

schema:SubstanceUseOrAbuse a rdfs:Class ;
    rdfs:label "SubstanceUseOrAbuse" ;
    rdfs:comment "The quantification or description of substance use (i.e illicit substances or psychoactive drugs) or abuse for a person" ;
    rdfs:subClassOf schema:CreatedInExtension,
        schema:LifestyleOrHabits .

schema:SuperficialAnatomy a rdfs:Class ;
    rdfs:label "SuperficialAnatomy" ;
    rdfs:comment "Anatomical features that can be observed by sight (without dissection), including the form and proportions of the human body as well as surface landmarks that correspond to deeper subcutaneous structures. Superficial anatomy plays an important role in sports medicine, phlebotomy, and other medical specialties as underlying anatomical structures can be identified through surface palpation. For example, during back surgery, superficial anatomy can be used to palpate and count vertebrae to find the site of incision. Or in phlebotomy, superficial anatomy can be used to locate an underlying vein; for example, the median cubital vein can be located by palpating the borders of the cubital fossa (such as the epicondyles of the humerus) and then looking for the superficial signs of the vein, such as size, prominence, ability to refill after depression, and feel of surrounding tissue support. As another example, in a subluxation (dislocation) of the glenohumeral joint, the bony structure becomes pronounced with the deltoid muscle failing to cover the glenohumeral joint allowing the edges of the scapula to be superficially visible. Here, the superficial anatomy is the visible edges of the scapula, implying the underlying dislocation of the joint (the related anatomical structure)." ;
    rdfs:subClassOf schema:MedicalEntity,
        schema:MovedFromCore .

schema:SurgicalProcedure a rdfs:Class ;
    rdfs:label "SurgicalProcedure" ;
    rdfs:comment "A medical procedure involving an incision with instruments; performed for diagnose, or therapeutic purposes" ;
    rdfs:subClassOf schema:MedicalProcedure,
        schema:MovedFromCore .

schema:Syndrome a rdfs:Class ;
    rdfs:label "Syndrome" ;
    rdfs:comment "A syndrome is the association of several medical signs, symptoms, and or other characteristics that often occur together." ;
    rdfs:subClassOf schema:CreatedInExtension,
        schema:MedicalCondition .

schema:SystemicReview a rdfs:Class ;
    rdfs:label "SystemicReview" ;
    rdfs:comment "The part of anamnesis where the physician makes a screening interview of all body systems and organs for relevant disorders in history of the patient." ;
    rdfs:subClassOf schema:CreatedInExtension,
        schema:MedicalEnumeration .

schema:TherapeuticProcedure a rdfs:Class ;
    rdfs:label "TherapeuticProcedure" ;
    rdfs:comment "A medical procedure intended primarily for therapeutic purposes, aimed at improving a health condition." ;
    rdfs:subClassOf schema:MedicalProcedure,
        schema:MovedFromCore .

schema:TreatmentIndication a rdfs:Class ;
    rdfs:label "TreatmentIndication" ;
    rdfs:comment "An indication for treating an underlying condition, symptom, etc." ;
    rdfs:subClassOf schema:MedicalIndication,
        schema:MovedFromCore .

schema:TriageComplaint a rdfs:Class ;
    rdfs:label "TriageComplaint" ;
    rdfs:comment "A complaint on which patient triage is based" ;
    rdfs:subClassOf schema:CreatedInExtension,
        schema:MedicalSignOrSymptom .

schema:TriageScore a rdfs:Class ;
    rdfs:label "TriageScore" ;
    rdfs:comment "The score used sorting of patients (as in an emergency room) according to the urgency of their need for care normally evaluated on scale or coding system" ;
    rdfs:subClassOf schema:CreatedInExtension,
        schema:MedicalScore .

schema:Ultrasound a rdfs:Class ;
    rdfs:label "Ultrasound" ;
    rdfs:comment "Diagnostic ultrasound, also called sonography or diagnostic medical sonography, is an imaging method that uses high-frequency sound waves to produce relatively precise images of structures within your body." ;
    rdfs:subClassOf schema:CreatedInExtension,
        schema:MedicalImaging .

schema:UrinarySystem a rdfs:Class ;
    rdfs:label "UrinarySystem" ;
    rdfs:comment "Also known as the renal system, is an organ system which contribute to eliminate wastes from the body, regulate blood volume and pressure, control levels of electrolytes and metabolites, and regulate blood pH. Normally it consists of the two kidneys, ureters, the bladder, and the urethra." ;
    rdfs:subClassOf schema:AnatomicalSystem,
        schema:CreatedInExtension .

schema:Vaccination a rdfs:Class ;
    rdfs:label "Vaccination" ;
    rdfs:comment "Commonly known as immunization, vaccination is the administration of antigenic material (a vaccine) to stimulate an individual's immune system to develop adaptive immunity to a pathogen." ;
    rdfs:subClassOf schema:CreatedInExtension,
        schema:Immunotherapy .

schema:Vein a rdfs:Class ;
    rdfs:label "Vein" ;
    rdfs:comment "A type of blood vessel that specifically carries blood to the heart." ;
    rdfs:subClassOf schema:MovedFromCore,
        schema:Vessel .

schema:Vessel a rdfs:Class ;
    rdfs:label "Vessel" ;
    rdfs:comment "A component of the human body circulatory system comprised of an intricate network of hollow tubes that transport blood throughout the entire body." ;
    rdfs:subClassOf schema:AnatomicalStructure,
        schema:MovedFromCore .

schema:VesselsFunction a rdfs:Class ;
    rdfs:label "VesselsFunction" ;
    rdfs:comment "The function of vessels in human body" ;
    rdfs:subClassOf schema:CreatedInExtension,
        schema:PhysiologicalEntity .

schema:VeterinaryCare a rdfs:Class ;
    rdfs:label "VeterinaryCare" ;
    rdfs:comment "A vet's office." ;
    rdfs:subClassOf schema:MedicalOrganization,
        schema:MovedFromCore .

schema:VitalSign a rdfs:Class ;
    rdfs:label "VitalSign" ;
    rdfs:comment "Vital signs are measures of various physiological functions in order to assess the most basic body functions" ;
    rdfs:subClassOf schema:MedicalSign,
        schema:MovedFromCore .

schema:WaistCircumference a rdfs:Class ;
    rdfs:label "WaistCircumference" ;
    rdfs:comment "A measure of the circumference of the narrowest part of a person's waist, typically measured between belly button and the center of rib cage. This measurement can be used to indicate abdominal obesity and to track changes in waist size during weight loss efforts." ;
    rdfs:subClassOf schema:BodyMeasure,
        schema:CreatedInExtension .

schema:WaistHipRatio a rdfs:Class ;
    rdfs:label "WaistHipRatio" ;
    rdfs:comment "Waist–hip ratio or waist-to-hip ratio is the ratio of the circumference of the waist to that of the hips." ;
    rdfs:subClassOf schema:BodyMeasure,
        schema:CreatedInExtension .

<http://schema.org#drugPackage> a rdf:Property ;
    rdfs:label "drugPackage" ;
    schema:domainIncludes schema:Drug ;
    schema:rangeIncludes <http://schema.org#DrugPackage> ;
    rdfs:comment "Specifying the drug package resource" .

<http://schema.org#familyRelationshipName> a rdf:Property ;
    rdfs:label "familyRelationshipName" ;
    schema:domainIncludes schema:FamilyRelation ;
    schema:rangeIncludes schema:Text ;
    rdfs:comment "Specifying the label of any relationship between persons. " .

<http://schema.org#medicalScore> a rdf:Property ;
    rdfs:label "medicalScore" ;
    schema:domainIncludes schema:MedicalEntity ;
    schema:rangeIncludes schema:MedicalScore ;
    rdfs:comment "Specifying a medical score resource" .

<http://schema.org#medicalSpecimen> a rdf:Property ;
    rdfs:label "medicalSpecimen" ;
    schema:domainIncludes schema:MedicalProcedure,
        schema:Person ;
    schema:rangeIncludes <http://schema.org#MedicalSpecimen> ;
    rdfs:comment "Specifying a medical specimen resource for a person" .

<http://schema.org#medicalSpecimenDonor> a rdf:Property ;
    rdfs:label "medicalSpecimenDonor" ;
    schema:domainIncludes <http://schema.org#MedicalSpecimen> ;
    schema:rangeIncludes schema:Person ;
    rdfs:comment "The specimen donor" .

<http://schema.org#medicalSpecimenReceiver> a rdf:Property ;
    rdfs:label "medicalSpecimenReceiver" ;
    schema:domainIncludes <http://schema.org#MedicalSpecimen> ;
    schema:rangeIncludes schema:Person ;
    rdfs:comment "The specimen receiver" .

<http://schema.org#receiptDate> a rdf:Property ;
    rdfs:label "receiptDate" ;
    schema:domainIncludes <http://schema.org#MedicalSpecimen> ;
    schema:rangeIncludes schema:DateTime ;
    rdfs:comment "The date when the medical specimen was received" ;
    rdfs:subPropertyOf schema:dateTime .

<http://schema.org#specimenCollectionDate> a rdf:Property ;
    rdfs:label "specimenCollectionDate" ;
    schema:domainIncludes <http://schema.org#MedicalSpecimen> ;
    schema:rangeIncludes schema:DateTime ;
    rdfs:comment "The date when the medical specimen was collected" ;
    rdfs:subPropertyOf schema:dateTime .

schema:abortions a rdf:Property ;
    rdfs:label "abortions" ;
    schema:domainIncludes <http://purl.bioontology.org/ontology/SNOMEDCT/224526002> ;
    schema:rangeIncludes schema:Number ;
    rdfs:comment "Specifying the number of abortion for a given woman" .

schema:aboutRelative a rdf:Property ;
    rdfs:label "aboutRelative" ;
    schema:domainIncludes schema:Person ;
    schema:rangeIncludes <http://purl.bioontology.org/ontology/SNOMEDCT/303071001> ;
    rdfs:comment "Specifying a relative who is concerned by something. i.e medical history about XY relative." .

schema:action a rdf:Property ;
    rdfs:label "action" ;
    schema:domainIncludes schema:Muscle ;
    schema:rangeIncludes schema:Text ;
    rdfs:comment "The movement the muscle generates." .

schema:activeIngredient a rdf:Property ;
    rdfs:label "activeIngredient" ;
    schema:domainIncludes schema:DietarySupplement,
        schema:Drug,
        schema:DrugStrength,
        schema:PharmaceuticalSubstance ;
    schema:rangeIncludes schema:Text ;
    rdfs:comment "An active ingredient, typically chemical compounds and/or biologic substances." .

schema:administrationRoute a rdf:Property ;
    rdfs:label "administrationRoute" ;
    schema:domainIncludes schema:Drug ;
    schema:rangeIncludes schema:Text ;
    rdfs:comment "A route by which this drug may be administered, e.g. 'oral'." .

schema:admissionDate a rdf:Property ;
    rdfs:label "admissionDate" ;
    schema:domainIncludes <http://purl.bioontology.org/ontology/SNOMEDCT/305056002>,
        schema:MedicalAdmission,
        schema:Patient ;
    schema:rangeIncludes schema:DateTime ;
    rdfs:comment "Specifying a medical admission date" ;
    rdfs:subPropertyOf schema:dateTime .

schema:adulthoodHistory a rdf:Property ;
    rdfs:label "adulthoodHistory" ;
    schema:domainIncludes schema:Person ;
    schema:rangeIncludes <http://purl.bioontology.org/ontology/SNOMEDCT/41847000>,
        schema:AdulthoodHistory ;
    rdfs:comment "Specifying an adulthood description of someone" ;
    rdfs:subPropertyOf schema:socialHistory .

schema:adverseDrugEvent a rdf:Property ;
    rdfs:label "adverseDrugEvent" ;
    schema:domainIncludes <http://purl.bioontology.org/ontology/SNOMEDCT/277132007>,
        <http://purl.bioontology.org/ontology/SNOMEDCT/410942007>,
        schema:Drug,
        schema:DrugClass,
        schema:Patient ;
    schema:rangeIncludes <http://purl.bioontology.org/ontology/SNOMEDCT/62014003>,
        schema:AdverseDrugReaction ;
    rdfs:comment "Adverse drug events (ADEs) are defined as any injuries resulting from medication use, including physical harm, mental harm, or loss of function. ADEs, compared to medication errors, are a more direct measure of patient harm." ;
    rdfs:subPropertyOf schema:adverseEvent .

schema:affectedBy a rdf:Property ;
    rdfs:label "affectedBy" ;
    schema:domainIncludes schema:MedicalTest ;
    schema:rangeIncludes schema:Drug ;
    rdfs:comment "Drugs that affect the test's results." .

schema:ageAtEvent a rdf:Property ;
    rdfs:label "ageAtEvent" ;
    schema:domainIncludes schema:Person ;
    schema:rangeIncludes schema:Number ;
    rdfs:comment "Specifying the age of the entity when an event occurred" .

schema:alcoholIntake a rdf:Property ;
    rdfs:label "alcoholIntake" ;
    schema:domainIncludes schema:Person ;
    schema:rangeIncludes schema:AlcoholIntake ;
    rdfs:comment "Specifying a alcohol intake behaviour description of a person. " ;
    rdfs:subPropertyOf schema:lifestyleOrHabit .

schema:alcoholWarning a rdf:Property ;
    rdfs:label "alcoholWarning" ;
    schema:domainIncludes schema:Drug ;
    schema:rangeIncludes schema:Text ;
    rdfs:comment "Any precaution, guidance, contraindication, etc. related to consumption of alcohol while taking this drug." .

schema:algorithm a rdf:Property ;
    rdfs:label "algorithm" ;
    schema:domainIncludes schema:MedicalRiskScore ;
    schema:rangeIncludes schema:Text ;
    rdfs:comment "The algorithm or rules to follow to compute the score." .

schema:allergen a rdf:Property ;
    rdfs:label "allergen" ;
    schema:domainIncludes <http://purl.bioontology.org/ontology/SNOMEDCT/421961002>,
        <http://purl.bioontology.org/ontology/SNOMEDCT/473011001>,
        schema:Allergy,
        schema:Person ;
    schema:rangeIncludes <http://purl.bioontology.org/ontology/SNOMEDCT/90260006> ;
    rdfs:comment "Specifying something that can cause an allergic reaction." .

schema:allergy a rdf:Property ;
    rdfs:label "allergy" ;
    schema:domainIncludes schema:Patient ;
    schema:rangeIncludes <http://purl.bioontology.org/ontology/SNOMEDCT/421961002>,
        <http://purl.bioontology.org/ontology/SNOMEDCT/473011001>,
        schema:Allergy ;
    rdfs:comment "Specifying an allergic reaction, an hypersensitivity or disorder." .

schema:anamnesisProcedure a rdf:Property ;
    rdfs:label "anamnesisProcedure" ;
    schema:domainIncludes schema:Person ;
    schema:rangeIncludes schema:AnamnesisProcedure ;
    rdfs:comment "Specifying the anamnesis procedure resource for a patient or a person." ;
    rdfs:subPropertyOf schema:medicalProcedure .

schema:anatomicalOrgan a rdf:Property ;
    rdfs:label "anatomicalOrgan" ;
    schema:domainIncludes <http://purl.bioontology.org/ontology/SNOMEDCT/404684003>,
        schema:ClinicalFinding,
        schema:MedicalProcedure,
        schema:Person ;
    schema:rangeIncludes schema:AnatomicalOrgan ;
    rdfs:comment "Specifying the anatomical organ for a resource" .

schema:anatomicalRegion a rdf:Property ;
    rdfs:label "anatomicalRegion" ;
    schema:domainIncludes <http://purl.bioontology.org/ontology/SNOMEDCT/404684003>,
        schema:ClinicalFinding,
        schema:MedicalProcedure,
        schema:Person ;
    schema:rangeIncludes schema:AnatomicalRegion ;
    rdfs:comment "Specifying the anatomical region for a resource" .

schema:anatomicalStructure a rdf:Property ;
    rdfs:label "anatomicalStructure" ;
    schema:domainIncludes <http://purl.bioontology.org/ontology/SNOMEDCT/404684003>,
        schema:ClinicalFinding,
        schema:MedicalProcedure,
        schema:Person ;
    schema:rangeIncludes schema:AnatomicalStructure ;
    rdfs:comment "Specifying the anatomical structure for a resource" .

schema:anatomicalSystem a rdf:Property ;
    rdfs:label "anatomicalSystem" ;
    schema:domainIncludes <http://purl.bioontology.org/ontology/SNOMEDCT/404684003>,
        schema:ClinicalFinding,
        schema:MedicalProcedure,
        schema:Person ;
    schema:rangeIncludes schema:AnatomicalSystem ;
    rdfs:comment "Specifying the anatomical system for a resource" .

schema:antagonist a rdf:Property ;
    rdfs:label "antagonist" ;
    schema:domainIncludes schema:Muscle ;
    schema:rangeIncludes schema:Muscle ;
    rdfs:comment "The muscle whose action counteracts the specified muscle." .

schema:apgarScore a rdf:Property ;
    rdfs:label "apgarScore" ;
    schema:domainIncludes <http://purl.bioontology.org/ontology/SNOMEDCT/133933007> ;
    schema:rangeIncludes schema:Number ;
    rdfs:comment "Specifying the value of APGAR Score. " .

schema:applicableLocation a rdf:Property ;
    rdfs:label "applicableLocation" ;
    schema:domainIncludes schema:DrugCost,
        schema:DrugLegalStatus ;
    schema:rangeIncludes schema:AdministrativeArea ;
    rdfs:comment "The location in which the status applies." .

schema:arterialBranch a rdf:Property ;
    rdfs:label "arterialBranch" ;
    schema:domainIncludes schema:Artery ;
    schema:rangeIncludes schema:AnatomicalStructure ;
    rdfs:comment "The branches that comprise the arterial structure." .

schema:arterialPulse a rdf:Property ;
    rdfs:label "arterialPulse" ;
    schema:domainIncludes schema:Person ;
    schema:rangeIncludes schema:Pulse ;
    rdfs:comment "Specifying the regularly recurrent wave of distension in arteries that results from the progress through an artery of blood injected into the arterial system at each contraction of the ventricles of the heart" ;
    rdfs:subPropertyOf schema:medicalSign .

schema:aspect a rdf:Property ;
    rdfs:label "aspect" ;
    schema:domainIncludes schema:MedicalWebPage ;
    schema:rangeIncludes schema:Text ;
    rdfs:comment "An aspect of medical practice that is considered on the page, such as 'diagnosis', 'treatment', 'causes', 'prognosis', 'etiology', 'epidemiology', etc." .

schema:associatedAnatomy a rdf:Property ;
    rdfs:label "associatedAnatomy" ;
    schema:domainIncludes schema:MedicalCondition,
        schema:PhysicalActivity ;
    schema:rangeIncludes schema:AnatomicalStructure,
        schema:AnatomicalSystem,
        schema:SuperficialAnatomy ;
    rdfs:comment "The anatomy of the underlying organ system or structures associated with this entity." .

schema:associatedPathophysiology a rdf:Property ;
    rdfs:label "associatedPathophysiology" ;
    schema:domainIncludes schema:AnatomicalStructure,
        schema:AnatomicalSystem,
        schema:SuperficialAnatomy ;
    schema:rangeIncludes schema:Text ;
    rdfs:comment "If applicable, a description of the pathophysiology associated with the anatomical system, including potential abnormal changes in the mechanical, physical, and biochemical functions of the system." .

schema:atWeeksAmenorrhea a rdf:Property ;
    rdfs:label "atWeeksAmenorrhea" ;
    schema:domainIncludes schema:MedicalCondition ;
    schema:rangeIncludes schema:Number ;
    rdfs:comment "Specifying the weeks of amenorrhoea when an event occurs. " .

schema:availableIn a rdf:Property ;
    rdfs:label "availableIn" ;
    schema:domainIncludes schema:DrugStrength ;
    schema:rangeIncludes schema:AdministrativeArea ;
    rdfs:comment "The location in which the strength is available." .

schema:availableService a rdf:Property ;
    rdfs:label "availableService" ;
    schema:domainIncludes schema:Hospital,
        schema:MedicalClinic,
        schema:Physician ;
    schema:rangeIncludes schema:MedicalProcedure,
        schema:MedicalTest,
        schema:MedicalTherapy ;
    rdfs:comment "A medical service available from this provider." .

schema:availableStrength a rdf:Property ;
    rdfs:label "availableStrength" ;
    schema:domainIncludes schema:Drug ;
    schema:rangeIncludes schema:DrugStrength ;
    rdfs:comment "An available dosage strength for the drug." .

schema:availableTest a rdf:Property ;
    rdfs:label "availableTest" ;
    schema:domainIncludes schema:DiagnosticLab ;
    schema:rangeIncludes schema:MedicalTest ;
    rdfs:comment "A diagnostic test or procedure offered by this lab." .

schema:belongsTo a rdf:Property ;
    rdfs:label "belongsTo" ;
    schema:domainIncludes schema:MedicalEntity ;
    schema:rangeIncludes schema:MedicalEntity ;
    rdfs:comment "Specifying a resource to which another resource belongs. Typically here it's used to link a medicalRecord to the Patient where isPartOf can't be used'. e.g :MedicalRecord schema:belongsTo :Patient" .

schema:birthHeight a rdf:Property ;
    rdfs:label "birthHeight" ;
    schema:domainIncludes <http://purl.bioontology.org/ontology/SNOMEDCT/133933007> ;
    schema:rangeIncludes schema:Number ;
    rdfs:comment "Specifying a birth weight" .

schema:birthPercentile a rdf:Property ;
    rdfs:label "birthPercentile" ;
    schema:domainIncludes <http://purl.bioontology.org/ontology/SNOMEDCT/133933007> ;
    schema:rangeIncludes schema:Number ;
    rdfs:comment "Specifying the birth percentile of a newborn" .

schema:birthPlace a rdf:Property ;
    rdfs:label "birthPlace" ;
    schema:domainIncludes schema:Birth,
        schema:Person ;
    schema:rangeIncludes <http://purl.bioontology.org/ontology/SNOMEDCT/169812000>,
        schema:Place ;
    rdfs:comment "The place where the person was born." .

schema:birthWeight a rdf:Property ;
    rdfs:label "birthWeight" ;
    schema:domainIncludes <http://purl.bioontology.org/ontology/SNOMEDCT/133933007> ;
    schema:rangeIncludes schema:Number ;
    rdfs:comment "Specifying birth weight of a newborn" .

schema:bloodGroup a rdf:Property ;
    rdfs:label "bloodGroup" ;
    schema:domainIncludes schema:Person ;
    schema:rangeIncludes <http://purl.bioontology.org/ontology/SNOMEDCT/365636006> ;
    rdfs:comment "Specifying the blood group for a person, i.e type of human blood based on presence or absence of inherited antigenic substances on the surface of red blood cells." .

schema:bloodSupply a rdf:Property ;
    rdfs:label "bloodSupply" ;
    schema:domainIncludes schema:Muscle ;
    schema:rangeIncludes schema:Vessel ;
    rdfs:comment "The blood vessel that carries blood from the heart to the muscle." .

schema:bodyLocation a rdf:Property ;
    rdfs:label "bodyLocation" ;
    schema:domainIncludes schema:AnatomicalStructure ;
    schema:rangeIncludes schema:Text ;
    rdfs:comment "Location in the body of the anatomical structure." .

schema:bodyMassIndex a rdf:Property ;
    rdfs:label "bodyMassIndex" ;
    schema:domainIncludes schema:Person ;
    schema:rangeIncludes schema:Number ;
    rdfs:comment "Specifying the body mass index of  a person" .

schema:bodyPosition a rdf:Property ;
    rdfs:label "bodyPosition" ;
    schema:domainIncludes schema:MedicalEntity ;
    schema:rangeIncludes <http://purl.bioontology.org/ontology/SNOMEDCT/364830008> ;
    rdfs:comment "Specifying a position of human body or anatomical entity in given space e.g. Supine body position, standing position, sitting position etc." .

schema:bodySide a rdf:Property ;
    rdfs:label "bodySide" ;
    schema:domainIncludes <http://purl.bioontology.org/ontology/SNOMEDCT/404684003>,
        schema:ClinicalFinding ;
    schema:rangeIncludes schema:Text ;
    rdfs:comment "Specifying the laterality of the body structure, body organ, or body region." .

schema:bodyVolumeIndex a rdf:Property ;
    rdfs:label "bodyVolumeIndex" ;
    schema:domainIncludes schema:Person ;
    schema:rangeIncludes schema:Number ;
    rdfs:comment "Specifying the body volume index of  a person" .

schema:branch a rdf:Property ;
    rdfs:label "branch" ;
    schema:domainIncludes schema:Nerve ;
    schema:rangeIncludes schema:AnatomicalStructure ;
    rdfs:comment "The branches that delineate from the nerve bundle." .

schema:breastfeedingWarning a rdf:Property ;
    rdfs:label "breastfeedingWarning" ;
    schema:domainIncludes schema:Drug ;
    schema:rangeIncludes schema:Text ;
    rdfs:comment "Any precaution, guidance, contraindication, etc. related to this drug's use by breastfeeding mothers." .

schema:careLocation a rdf:Property ;
    rdfs:label "careLocation" ;
    schema:domainIncludes <http://purl.bioontology.org/ontology/SNOMEDCT/305056002>,
        schema:Event,
        schema:MedicalProcedure,
        schema:Patient ;
    schema:rangeIncludes schema:HealthFacility,
        schema:MedicalDepartment,
        schema:MedicalUnit,
        schema:Place ;
    rdfs:comment "Specifying a location or a place where the care event is taking place" ;
    rdfs:subPropertyOf schema:location .

schema:carePlan a rdf:Property ;
    rdfs:label "carePlan" ;
    schema:domainIncludes schema:Drug ;
    schema:rangeIncludes schema:Text ;
    rdfs:comment "Any precaution, guidance, contraindication, etc. related to consumption of specific foods while taking this drug." .

schema:careReason a rdf:Property ;
    rdfs:label "careReason" ;
    schema:domainIncludes schema:CaringEvent,
        schema:MedicalProcedure,
        schema:Patient ;
    schema:rangeIncludes schema:MedicalIndication ;
    rdfs:comment "Specifying a reason for a caring event(typically a medical condition or other medical encounter reasons)" ;
    rdfs:subPropertyOf schema:indication .

schema:caredPerson a rdf:Property ;
    rdfs:label "caredPerson" ;
    schema:domainIncludes <http://purl.bioontology.org/ontology/SNOMEDCT/223366009>,
        schema:CaringEvent,
        schema:HealthcareProfessional ;
    schema:rangeIncludes schema:Patient ;
    rdfs:comment "Specifying a person (typically a patient) receiving services from the health care professional during a caring event." .

schema:caringEvent a rdf:Property ;
    rdfs:label "caringEvent" ;
    schema:domainIncludes schema:MedicalCondition,
        schema:Patient ;
    schema:rangeIncludes schema:CaringEvent ;
    rdfs:comment "Specifying an event wherein services are rendered by members of the health profession (or under their supervision) for the benefit of the patient." ;
    rdfs:subPropertyOf schema:lifeEvent .

schema:causalityStatus a rdf:Property ;
    rdfs:label "causalityStatus" ;
    schema:domainIncludes schema:MedicalEntity ;
    schema:rangeIncludes schema:MedicalEntity ;
    rdfs:comment "Causality score or ranking following a codified system (like HL7 causalityExpectation) or not." ;
    rdfs:subPropertyOf schema:status .

schema:causeOf a rdf:Property ;
    rdfs:label "causeOf" ;
    schema:domainIncludes schema:MedicalCause ;
    schema:rangeIncludes schema:MedicalEntity ;
    rdfs:comment "The condition, complication, symptom, sign, etc. caused." .

schema:chiefComplaint a rdf:Property ;
    rdfs:label "chiefComplaint" ;
    schema:domainIncludes schema:Patient ;
    schema:rangeIncludes schema:ChiefComplaint ;
    rdfs:comment "Specifying a chief complaint resource" ;
    rdfs:subPropertyOf schema:medicalSymptom .

schema:childhoodHistory a rdf:Property ;
    rdfs:label "childhoodHistory" ;
    schema:domainIncludes schema:Person ;
    schema:rangeIncludes schema:ChildhoodHistory ;
    rdfs:comment "Specifying a resource describing the childhood history of a patient or a person" ;
    rdfs:subPropertyOf schema:socialHistory .

schema:clincalPharmacology a rdf:Property ;
    rdfs:label "clincalPharmacology" ;
    schema:domainIncludes schema:Drug ;
    schema:rangeIncludes schema:Text ;
    rdfs:comment "Description of the absorption and elimination of drugs, including their concentration (pharmacokinetics, pK) and biological effects (pharmacodynamics, pD)." .

schema:clinicalFinding a rdf:Property ;
    rdfs:label "clinicalFinding" ;
    schema:domainIncludes schema:Patient ;
    schema:rangeIncludes <http://purl.bioontology.org/ontology/SNOMEDCT/118246004>,
        <http://purl.bioontology.org/ontology/SNOMEDCT/404684003>,
        schema:ClinicalFinding ;
    rdfs:comment "Specifying a clinical finding of a patient through a formal clinical examination. example: Body temperature, etc" .

schema:code a rdf:Property ;
    rdfs:label "code" ;
    schema:domainIncludes schema:MedicalEntity ;
    schema:rangeIncludes schema:MedicalCode ;
    rdfs:comment "A medical code for the entity, taken from a controlled vocabulary or ontology such as ICD-9, DiseasesDB, MeSH, SNOMED-CT, RxNorm, etc." .

schema:codeValue a rdf:Property ;
    rdfs:label "codeValue" ;
    schema:domainIncludes schema:MedicalCode ;
    schema:rangeIncludes schema:Text ;
    rdfs:comment "The actual code." .

schema:codingSystem a rdf:Property ;
    rdfs:label "codingSystem" ;
    schema:domainIncludes schema:MedicalCode ;
    schema:rangeIncludes schema:Text ;
    rdfs:comment "The coding system, e.g. 'ICD-10'." .

schema:codingSystemVersion a rdf:Property ;
    rdfs:label "codingSystemVersion" ;
    schema:domainIncludes schema:MedicalCode ;
    schema:rangeIncludes schema:Text ;
    rdfs:comment "The coding system version, e.g. 'Version 2015-01-31'." .

schema:comorbidity a rdf:Property ;
    rdfs:label "comorbidity" ;
    schema:domainIncludes schema:MedicalCondition,
        schema:Patient ;
    schema:rangeIncludes schema:MedicalCondition ;
    rdfs:comment "Specifying a health disorder simultaneously but independently existing with another health disorder in a human." .

schema:comprisedOf a rdf:Property ;
    rdfs:label "comprisedOf" ;
    schema:domainIncludes schema:AnatomicalSystem ;
    schema:rangeIncludes schema:AnatomicalStructure,
        schema:AnatomicalSystem ;
    rdfs:comment "Specifying something physically contained by something else. Typically used here for the underlying anatomical structures, such as organs, that comprise the anatomical system." .

schema:confirmationStatus a rdf:Property ;
    rdfs:label "confirmationStatus" ;
    schema:domainIncludes schema:Text ;
    schema:rangeIncludes schema:MedicalEntity ;
    rdfs:comment "Specifying the confirmation status of something. eg: confirmed, suspected etc., as outcome of evaluation process" ;
    rdfs:subPropertyOf schema:status .

schema:connectedTo a rdf:Property ;
    rdfs:label "connectedTo" ;
    schema:domainIncludes schema:AnatomicalStructure ;
    schema:rangeIncludes schema:AnatomicalStructure ;
    rdfs:comment "Other anatomical structures to which this structure is connected." .

schema:contraindication a rdf:Property ;
    rdfs:label "contraindication" ;
    schema:domainIncludes schema:MedicalDevice,
        schema:MedicalTherapy ;
    schema:rangeIncludes schema:MedicalContraindication ;
    rdfs:comment "A contraindication for this therapy." .

schema:cookTime a rdf:Property ;
    rdfs:label "cookTime" ;
    schema:domainIncludes schema:Recipe ;
    schema:rangeIncludes schema:Duration ;
    rdfs:comment "The time it takes to actually cook the dish, in ISO 8601 duration format." .

schema:cookingMethod a rdf:Property ;
    rdfs:label "cookingMethod" ;
    schema:domainIncludes schema:Recipe ;
    schema:rangeIncludes schema:Text ;
    rdfs:comment "The method of cooking, such as Frying, Steaming, ..." .

schema:cosmeticProcedure a rdf:Property ;
    rdfs:label "cosmeticProcedure" ;
    schema:domainIncludes schema:Person ;
    schema:rangeIncludes schema:MedicalProcedure ;
    rdfs:comment "Specifying a cosmetic procedure resource for a patient or a person" ;
    rdfs:subPropertyOf schema:electiveProcedure .

schema:cost a rdf:Property ;
    rdfs:label "cost" ;
    schema:domainIncludes schema:Drug ;
    schema:rangeIncludes schema:DrugCost ;
    rdfs:comment "Cost per unit of the drug, as reported by the source being tagged." .

schema:costCategory a rdf:Property ;
    rdfs:label "costCategory" ;
    schema:domainIncludes schema:DrugCost ;
    schema:rangeIncludes schema:DrugCostCategory ;
    rdfs:comment "The category of cost, such as wholesale, retail, reimbursement cap, etc." .

schema:costCurrency a rdf:Property ;
    rdfs:label "costCurrency" ;
    schema:domainIncludes schema:DrugCost ;
    schema:rangeIncludes schema:Text ;
    rdfs:comment "The currency (in 3-letter of the drug cost. See: http://en.wikipedia.org/wiki/ISO_4217 " .

schema:costOrigin a rdf:Property ;
    rdfs:label "costOrigin" ;
    schema:domainIncludes schema:DrugCost ;
    schema:rangeIncludes schema:Text ;
    rdfs:comment "Additional details to capture the origin of the cost data. For example, 'Medicare Part B'." .

schema:costPerUnit a rdf:Property ;
    rdfs:label "costPerUnit" ;
    schema:domainIncludes schema:DrugCost ;
    schema:rangeIncludes schema:Number,
        schema:Text ;
    rdfs:comment "The cost per unit of the drug." .

schema:deathPlace a rdf:Property ;
    rdfs:label "deathPlace" ;
    schema:domainIncludes schema:Death,
        schema:Person ;
    schema:rangeIncludes <http://purl.bioontology.org/ontology/SNOMEDCT/169812000>,
        schema:Place ;
    rdfs:comment "The place where the person died." ;
    rdfs:subClassOf schema:MovedFromCore .

schema:diagnosis a rdf:Property ;
    rdfs:label "diagnosis" ;
    schema:domainIncludes schema:DDxElement,
        schema:Patient ;
    schema:rangeIncludes <http://purl.bioontology.org/ontology/SNOMEDCT/439401001>,
        schema:MedicalCondition ;
    rdfs:comment "One or more alternative conditions considered in the differential diagnosis process as output of a diagnosis process." .

schema:diagnosticDate a rdf:Property ;
    rdfs:label "diagnosticDate" ;
    schema:domainIncludes <http://purl.bioontology.org/ontology/SNOMEDCT/439401001>,
        schema:Person ;
    schema:rangeIncludes schema:DateTime ;
    rdfs:comment "Specifying the diagnostic date for  a person" ;
    rdfs:subPropertyOf schema:dateTime .

schema:diagnosticMean a rdf:Property ;
    rdfs:label "diagnosticMean" ;
    schema:domainIncludes <http://purl.bioontology.org/ontology/SNOMEDCT/439401001>,
        schema:Diagnosis ;
    schema:rangeIncludes <http://purl.bioontology.org/ontology/SNOMEDCT/260686004>,
        schema:MedicalDevice,
        schema:MedicalTest ;
    rdfs:comment "Specifying the mean for diagnosis procedure." .

schema:diagnosticPlace a rdf:Property ;
    rdfs:label "diagnosticPlace" ;
    schema:domainIncludes <http://purl.bioontology.org/ontology/SNOMEDCT/439401001>,
        schema:Diagnosis ;
    schema:rangeIncludes schema:HealthFacility,
        schema:MedicalDepartment,
        schema:MedicalUnit ;
    rdfs:comment "Specifying the location or place where the diagnosis was made. Typically the department or health facility unit." .

schema:diagnosticType a rdf:Property ;
    rdfs:label "diagnosticType" ;
    schema:domainIncludes <http://purl.bioontology.org/ontology/SNOMEDCT/439401001>,
        schema:Diagnosis ;
    schema:rangeIncludes <http://purl.bioontology.org/ontology/SNOMEDCT/106229004> ;
    rdfs:comment "Specifying the type of diagnosis i.e medical discharge diagnosis, admission diagnosis, etc." .

schema:diagram a rdf:Property ;
    rdfs:label "diagram" ;
    schema:domainIncludes schema:AnatomicalStructure ;
    schema:rangeIncludes schema:ImageObject ;
    rdfs:comment "An image containing a diagram that illustrates the structure and/or its component substructures and/or connections with other structures." .

schema:diastolicBloodPressure a rdf:Property ;
    rdfs:label "diastolicBloodPressure" ;
    schema:domainIncludes schema:Person ;
    schema:rangeIncludes <http://purl.bioontology.org/ontology/SNOMEDCT/271650006> ;
    rdfs:comment "Specifying a diastolic arterial blood pressure of a patient." ;
    rdfs:subPropertyOf schema:bloodPressure .

schema:diet a rdf:Property ;
    rdfs:label "diet" ;
    schema:domainIncludes schema:ExerciseAction ;
    schema:rangeIncludes schema:Diet ;
    rdfs:comment "A sub property of instrument. The diet used in this action." ;
    rdfs:subPropertyOf schema:instrument .

schema:dietFeatures a rdf:Property ;
    rdfs:label "dietFeatures" ;
    schema:domainIncludes schema:Diet ;
    schema:rangeIncludes schema:Text ;
    rdfs:comment "Nutritional information specific to the dietary plan. May include dietary recommendations on what foods to avoid, what foods to consume, and specific alterations/deviations from the USDA or other regulatory body's approved dietary guidelines." .

schema:differentialDiagnosis a rdf:Property ;
    rdfs:label "differentialDiagnosis" ;
    schema:domainIncludes schema:MedicalCondition ;
    schema:rangeIncludes schema:DDxElement ;
    rdfs:comment "One of a set of differential diagnoses for the condition. Specifically, a closely-related or competing diagnosis typically considered later in the cognitive process whereby this medical condition is distinguished from others most likely responsible for a similar collection of signs and symptoms to reach the most parsimonious diagnosis or diagnoses in a patient." .

schema:dischargeDate a rdf:Property ;
    rdfs:label "dischargeDate" ;
    schema:domainIncludes schema:MedicalDischarge,
        schema:Patient ;
    schema:rangeIncludes schema:DateTime ;
    rdfs:comment "Specifying a medical discharge date for a patient" ;
    rdfs:subPropertyOf schema:dateTime .

schema:dispensationCode a rdf:Property ;
    rdfs:label "dispensationCode" ;
    schema:domainIncludes schema:Drug,
        schema:MedicationDispensation ;
    schema:rangeIncludes schema:Text ;
    rdfs:comment "specifying the code of the medication dispensation activity" .

schema:distinguishingSign a rdf:Property ;
    rdfs:label "distinguishingSign" ;
    schema:domainIncludes schema:DDxElement ;
    schema:rangeIncludes schema:MedicalSignOrSymptom ;
    rdfs:comment "One of a set of signs and symptoms that can be used to distinguish this diagnosis from others in the differential diagnosis." .

schema:dosageForm a rdf:Property ;
    rdfs:label "dosageForm" ;
    schema:domainIncludes schema:DietarySupplement,
        schema:Drug ;
    schema:rangeIncludes schema:Text ;
    rdfs:comment "A dosage form in which this drug/supplement is available, e.g. 'tablet', 'suspension', 'injection'." .

schema:doseSchedule a rdf:Property ;
    rdfs:label "doseSchedule" ;
    schema:domainIncludes schema:Drug,
        schema:TherapeuticProcedure ;
    schema:rangeIncludes schema:DoseSchedule ;
    rdfs:comment "A dosing schedule for the drug for a given population, either observed, recommended, or maximum dose based on the type used." .

schema:doseUnit a rdf:Property ;
    rdfs:label "doseUnit" ;
    schema:domainIncludes schema:DoseSchedule ;
    schema:rangeIncludes schema:Text ;
    rdfs:comment "The unit of the dose, e.g. 'mg'." .

schema:doseValue a rdf:Property ;
    rdfs:label "doseValue" ;
    schema:domainIncludes schema:DoseSchedule ;
    schema:rangeIncludes schema:Number ;
    rdfs:comment "The value of the dose, e.g. 500." .

schema:drainsTo a rdf:Property ;
    rdfs:label "drainsTo" ;
    schema:domainIncludes schema:Vein ;
    schema:rangeIncludes schema:Vessel ;
    rdfs:comment "The vasculature that the vein drains into." .

schema:drug a rdf:Property ;
    rdfs:label "drug" ;
    schema:domainIncludes schema:DrugClass,
        schema:MedicalCondition,
        schema:Patient,
        schema:TherapeuticProcedure ;
    schema:rangeIncludes <http://purl.bioontology.org/ontology/SNOMEDCT/410942007>,
        schema:Drug ;
    rdfs:comment "Specifying a drug or medicine used in a medication procedure" .

schema:drugAdministrated a rdf:Property ;
    rdfs:label "drugAdministrated" ;
    schema:domainIncludes schema:Drug,
        schema:Patient,
        schema:TherapeuticProcedure ;
    schema:rangeIncludes <http://purl.bioontology.org/ontology/SNOMEDCT/129019007> ;
    rdfs:comment "Medication administrated not taking into account the quantity really taken by the patient f.eg. when some quantity may be vomitted" .

schema:drugAdministration a rdf:Property ;
    rdfs:label "drugAdministration" ;
    schema:domainIncludes schema:MedicalCondition,
        schema:Patient,
        schema:TherapeuticProcedure ;
    schema:rangeIncludes <http://purl.bioontology.org/ontology/SNOMEDCT/182832007> ;
    rdfs:comment "specifying the event of administering the drug to the patient. Typically associated with the route of administration i.e.oral, injection etc." .

schema:drugClass a rdf:Property ;
    rdfs:label "drugClass" ;
    schema:domainIncludes schema:Drug ;
    schema:rangeIncludes schema:DrugClass ;
    rdfs:comment "The class of drug this belongs to (e.g., statins)." .

schema:drugDispensation a rdf:Property ;
    rdfs:label "drugDispensation" ;
    schema:domainIncludes <http://purl.bioontology.org/ontology/SNOMEDCT/223366009>,
        schema:HealthcareProfessional,
        schema:MedicalCondition,
        schema:MedicationDispensation,
        schema:TherapeuticProcedure ;
    schema:rangeIncludes <http://purl.bioontology.org/ontology/SNOMEDCT/440298008> ;
    rdfs:comment "Specifying an drug dispensation event i.e the event of delivering the drug to the patient at pharmacy. This is different to the drug administration" .

schema:drugDispensator a rdf:Property ;
    rdfs:label "drugDispensator" ;
    schema:domainIncludes schema:Drug,
        schema:Patient ;
    schema:rangeIncludes schema:HealthcareProfessional ;
    rdfs:comment "Health care professional entitled to deliver drugs on prescription to the end-consumer (pharmacist). " ;
    rdfs:subPropertyOf schema:provider .

schema:drugPreparation a rdf:Property ;
    rdfs:label "drugPreparation" ;
    schema:domainIncludes <http://purl.bioontology.org/ontology/SNOMEDCT/223366009>,
        schema:Drug,
        schema:HealthcareProfessional,
        schema:Person,
        schema:TherapeuticProcedure ;
    schema:rangeIncludes <http://purl.bioontology.org/ontology/SNOMEDCT/105904009> ;
    rdfs:comment "Specifying a drug preparation used in a procedure, typically prepared for a patient from one or multiple drug packages" .

schema:drugTaken a rdf:Property ;
    rdfs:label "drugTaken" ;
    schema:domainIncludes schema:Drug,
        schema:Patient,
        schema:TherapeuticProcedure ;
    schema:rangeIncludes <http://purl.bioontology.org/ontology/SNOMEDCT/129019007> ;
    rdfs:comment "Medication actually taken which may be different from drug administrated sometimes when some quantity is lost" .

schema:drugUnit a rdf:Property ;
    rdfs:label "drugUnit" ;
    schema:domainIncludes schema:DrugCost ;
    schema:rangeIncludes schema:Text ;
    rdfs:comment "The unit in which the drug is measured, e.g. '5 mg tablet'." .

schema:duplicateTherapy a rdf:Property ;
    rdfs:label "duplicateTherapy" ;
    schema:domainIncludes schema:MedicalTherapy ;
    schema:rangeIncludes schema:MedicalTherapy ;
    rdfs:comment "A therapy that duplicates or overlaps this one." .

schema:educationLevel a rdf:Property ;
    rdfs:label "educationLevel" ;
    schema:domainIncludes schema:Person ;
    schema:rangeIncludes schema:EducationLevel ;
    rdfs:comment "Specifying the education level of the person" .

schema:elderhoodHistory a rdf:Property ;
    rdfs:label "elderhoodHistory" ;
    schema:domainIncludes schema:Person ;
    schema:rangeIncludes schema:Elderhood ;
    rdfs:comment "specifying the elderhood history of someone" ;
    rdfs:subPropertyOf schema:socialHistory .

schema:encounterPlace a rdf:Property ;
    rdfs:label "encounterPlace" ;
    schema:domainIncludes schema:MedicalEncounter ;
    schema:rangeIncludes schema:HealthFacility ;
    rdfs:comment "specifying the location or a place where the medical encounter took place" ;
    rdfs:subPropertyOf schema:location .

schema:encounterProvider a rdf:Property ;
    rdfs:label "encounterProvider" ;
    schema:domainIncludes schema:MedicalEncounter ;
    schema:rangeIncludes <http://purl.bioontology.org/ontology/SNOMEDCT/223366009>,
        schema:HealthcareProfessional,
        schema:Person ;
    rdfs:comment "specifying the provider of the medical encounter" ;
    rdfs:subPropertyOf schema:provider .

schema:encounterReason a rdf:Property ;
    rdfs:label "encounterReason" ;
    schema:domainIncludes schema:MedicalEncounter,
        schema:Patient ;
    schema:rangeIncludes schema:MedicalCondition,
        schema:MedicalIndication ;
    rdfs:comment "specifying the reason or indication for a patient medical encounter" ;
    rdfs:subPropertyOf schema:indication .

schema:encounterStatus a rdf:Property ;
    rdfs:label "encounterStatus" ;
    schema:domainIncludes schema:MedicalEncounter,
        schema:Patient,
        schema:Person ;
    schema:rangeIncludes schema:Text ;
    rdfs:comment "specifying the status of medical encounter procedure." ;
    rdfs:subPropertyOf schema:status .

schema:enzyme a rdf:Property ;
    rdfs:label "enzyme" ;
    schema:domainIncludes schema:PhysiologicalEntity ;
    schema:rangeIncludes schema:Enzyme ;
    rdfs:comment "Specifyning the enzyme involved in physiological role" .

schema:epidemiology a rdf:Property ;
    rdfs:label "epidemiology" ;
    schema:domainIncludes schema:MedicalCondition,
        schema:PhysicalActivity ;
    schema:rangeIncludes schema:Text ;
    rdfs:comment "The characteristics of associated patients, such as age, gender, race etc." .

schema:estimatesRiskOf a rdf:Property ;
    rdfs:label "estimatesRiskOf" ;
    schema:domainIncludes schema:MedicalRiskEstimator ;
    schema:rangeIncludes schema:MedicalEntity ;
    rdfs:comment "The condition, complication, or symptom whose risk is being estimated." .

schema:ethnicity a rdf:Property ;
    rdfs:label "ethnicity" ;
    schema:domainIncludes schema:Person ;
    schema:rangeIncludes schema:Ethnicity ;
    rdfs:comment "Specifying the ethnicity resource of someone. Ethnicity or ethnic group is a socially defined category of people. Race and Ethnicity as well as religious beliefs are in most cases not given in EHR, and collecting this info is often seen as illegal. Please check local regulations before using this property " .

schema:evidenceLevel a rdf:Property ;
    rdfs:label "evidenceLevel" ;
    schema:domainIncludes schema:MedicalGuideline ;
    schema:rangeIncludes schema:MedicalEvidenceLevel ;
    rdfs:comment "Strength of evidence of the data used to formulate the guideline (enumerated)." .

schema:evidenceOrigin a rdf:Property ;
    rdfs:label "evidenceOrigin" ;
    schema:domainIncludes schema:MedicalGuideline ;
    schema:rangeIncludes schema:Text ;
    rdfs:comment "Source of the data used to formulate the guidance, e.g. RCT, consensus opinion, etc." .

schema:examination a rdf:Property ;
    rdfs:label "examination" ;
    schema:domainIncludes schema:Patient ;
    schema:rangeIncludes schema:MedicalTest ;
    rdfs:comment "Specifying an examination procedure in general performed on  something or on a patient." .

schema:exerciseRelatedDiet a rdf:Property ;
    rdfs:label "exerciseRelatedDiet" ;
    schema:domainIncludes schema:ExerciseAction ;
    schema:rangeIncludes schema:Diet ;
    rdfs:comment "A sub property of instrument. The diet used in this action." ;
    rdfs:subPropertyOf schema:instrument .

schema:expectedPrognosis a rdf:Property ;
    rdfs:label "expectedPrognosis" ;
    schema:domainIncludes schema:MedicalCondition ;
    schema:rangeIncludes schema:Text ;
    rdfs:comment "The likely outcome in either the short term or long term of the medical condition." .

schema:expertConsiderations a rdf:Property ;
    rdfs:label "expertConsiderations" ;
    schema:domainIncludes schema:Diet ;
    schema:rangeIncludes schema:Text ;
    rdfs:comment "Medical expert advice related to the plan." .

schema:familyMedicalHistory a rdf:Property ;
    rdfs:label "familyMedicalHistory" ;
    schema:domainIncludes schema:Person ;
    schema:rangeIncludes <http://purl.bioontology.org/ontology/SNOMEDCT/57177007> ;
    rdfs:comment "Specifying a personal history as a part of a full medical history provided by the patient during an anamnesis procedure ." ;
    rdfs:subPropertyOf schema:medicalHistory .

schema:familyRelationship a rdf:Property ;
    rdfs:label "familyRelationship" ;
    schema:domainIncludes schema:Person ;
    schema:rangeIncludes schema:FamilyRelation ;
    rdfs:comment "Specifying a relationship between persons. Typically between persons uses the 'American Kinship terminology'." .

schema:fatContent a rdf:Property ;
    rdfs:label "fatContent" ;
    schema:domainIncludes schema:NutritionInformation ;
    schema:rangeIncludes schema:Mass ;
    rdfs:comment "The number of grams of fat." .

schema:father a rdf:Property ;
    rdfs:label "father" ;
    schema:domainIncludes schema:Person ;
    schema:rangeIncludes schema:Person ;
    rdfs:comment "Specifying a father (parent) of this person when no other specifications are given." ;
    rdfs:subPropertyOf schema:parent .

schema:followup a rdf:Property ;
    rdfs:label "followup" ;
    schema:domainIncludes schema:MedicalProcedure ;
    schema:rangeIncludes schema:Text ;
    rdfs:comment "Typical or recommended followup care after the procedure is performed." .

schema:foodEstablishment a rdf:Property ;
    rdfs:label "foodEstablishment" ;
    schema:domainIncludes schema:CookAction ;
    schema:rangeIncludes schema:FoodEstablishment,
        schema:Place ;
    rdfs:comment "A sub property of location. The specific food establishment where the action occurred." ;
    rdfs:subPropertyOf schema:location .

schema:foodEvent a rdf:Property ;
    rdfs:label "foodEvent" ;
    schema:domainIncludes schema:CookAction ;
    schema:rangeIncludes schema:FoodEvent ;
    rdfs:comment "A sub property of location. The specific food event where the action occurred." ;
    rdfs:subPropertyOf schema:location .

schema:foodIntolerance a rdf:Property ;
    rdfs:label "foodIntolerance" ;
    schema:domainIncludes schema:Patient ;
    schema:rangeIncludes <http://purl.bioontology.org/ontology/SNOMEDCT/235719002>,
        schema:MedicalCondition ;
    rdfs:comment "Food intolerance or non-allergic food hypersensitivity is a term used widely for varied physiological responses associated with a particular food, or compound found in a range of foods." ;
    rdfs:subPropertyOf schema:adverseOutcome .

schema:foodWarning a rdf:Property ;
    rdfs:label "foodWarning" ;
    schema:domainIncludes schema:Drug ;
    schema:rangeIncludes schema:Text ;
    rdfs:comment "Any precaution, guidance, contraindication, etc. related to consumption of specific foods while taking this drug." .

schema:function a rdf:Property ;
    rdfs:label "function" ;
    schema:domainIncludes schema:AnatomicalStructure ;
    schema:rangeIncludes schema:Text ;
    rdfs:comment "Function of the anatomical structure." .

schema:functionalClass a rdf:Property ;
    rdfs:label "functionalClass" ;
    schema:domainIncludes schema:Joint ;
    schema:rangeIncludes schema:Text ;
    rdfs:comment "The degree of mobility the joint allows." .

schema:gravidity a rdf:Property ;
    rdfs:label "gravidity" ;
    schema:domainIncludes <http://purl.bioontology.org/ontology/SNOMEDCT/224526002>,
        schema:Person ;
    schema:rangeIncludes schema:Number ;
    rdfs:comment "Specifying the number of times a woman has been pregnant, regardless of whether the pregnancies were interrupted or resulted in a live birth." .

schema:guarantor a rdf:Property ;
    rdfs:label "guarantor" ;
    schema:domainIncludes schema:Person ;
    schema:rangeIncludes schema:Organization,
        schema:Person ;
    rdfs:comment "Specifying a person or company , known as guarantor, offering insurance policies in return for premiums" .

schema:guideline a rdf:Property ;
    rdfs:label "guideline" ;
    schema:domainIncludes schema:MedicalEntity ;
    schema:rangeIncludes schema:MedicalGuideline ;
    rdfs:comment "A medical guideline related to this entity." .

schema:guidelineDate a rdf:Property ;
    rdfs:label "guidelineDate" ;
    schema:domainIncludes schema:MedicalGuideline ;
    schema:rangeIncludes schema:Date ;
    rdfs:comment "Date on which this guideline's recommendation was made." .

schema:guidelineSubject a rdf:Property ;
    rdfs:label "guidelineSubject" ;
    schema:domainIncludes schema:MedicalGuideline ;
    schema:rangeIncludes schema:MedicalEntity ;
    rdfs:comment "The medical conditions, treatments, etc. that are the subject of the guideline." .

schema:healthCondition a rdf:Property ;
    rdfs:label "healthCondition" ;
    schema:domainIncludes schema:PeopleAudience ;
    schema:rangeIncludes schema:MedicalCondition ;
    rdfs:comment "Expectations for health conditions of target audience." .

schema:hipCircumference a rdf:Property ;
    rdfs:label "hipCircumference" ;
    schema:domainIncludes schema:HipCircumference,
        schema:Person ;
    schema:rangeIncludes schema:Number ;
    rdfs:comment "The hip circumference measurement of someone" .

schema:historyOfPresentIllness a rdf:Property ;
    rdfs:label "historyOfPresentIllness" ;
    schema:domainIncludes schema:Patient ;
    schema:rangeIncludes schema:HistoryOfPresentIllness ;
    rdfs:comment "The history of the present illness." ;
    rdfs:subPropertyOf schema:personalHistory .

schema:howPerformed a rdf:Property ;
    rdfs:label "howPerformed" ;
    schema:domainIncludes schema:MedicalProcedure ;
    schema:rangeIncludes schema:Text ;
    rdfs:comment "How the procedure is performed." .

schema:identifyingExam a rdf:Property ;
    rdfs:label "identifyingExam" ;
    schema:domainIncludes schema:MedicalSign ;
    schema:rangeIncludes schema:PhysicalExam ;
    rdfs:comment "A physical examination that can identify this sign." .

schema:identifyingTest a rdf:Property ;
    rdfs:label "identifyingTest" ;
    schema:domainIncludes schema:MedicalSign ;
    schema:rangeIncludes schema:MedicalTest ;
    rdfs:comment "A diagnostic test that can identify this sign." .

schema:imagingTechnique a rdf:Property ;
    rdfs:label "imagingTechnique" ;
    schema:domainIncludes schema:ImagingTest ;
    schema:rangeIncludes schema:MedicalImagingTechnique ;
    rdfs:comment "Imaging technique used." .

schema:includedRiskFactor a rdf:Property ;
    rdfs:label "includedRiskFactor" ;
    schema:domainIncludes schema:MedicalRiskEstimator ;
    schema:rangeIncludes schema:MedicalRiskFactor ;
    rdfs:comment "A modifiable or non-modifiable risk factor included in the calculation, e.g. age, coexisting condition." .

schema:increasesRiskOf a rdf:Property ;
    rdfs:label "increasesRiskOf" ;
    schema:domainIncludes schema:MedicalRiskFactor ;
    schema:rangeIncludes schema:MedicalEntity ;
    rdfs:comment "The condition, complication, etc. influenced by this factor." .

schema:infectiousAgent a rdf:Property ;
    rdfs:label "infectiousAgent" ;
    schema:domainIncludes schema:InfectiousDisease ;
    schema:rangeIncludes schema:Text ;
    rdfs:comment "The actual infectious agent, such as a specific bacterium." .

schema:infectiousAgentClass a rdf:Property ;
    rdfs:label "infectiousAgentClass" ;
    schema:domainIncludes schema:InfectiousDisease ;
    schema:rangeIncludes schema:InfectiousAgentClass ;
    rdfs:comment "The class of infectious agent (bacteria, prion, etc.) that causes the disease." .

schema:ingredients a rdf:Property ;
    rdfs:label "ingredients" ;
    schema:domainIncludes schema:Recipe ;
    schema:rangeIncludes schema:Text ;
    rdfs:comment "A single ingredient used in the recipe, e.g. sugar, flour or garlic." .

schema:insertion a rdf:Property ;
    rdfs:label "insertion" ;
    schema:domainIncludes schema:Muscle ;
    schema:rangeIncludes schema:AnatomicalStructure ;
    rdfs:comment "The place of attachment of a muscle, or what the muscle moves." .

schema:insurance a rdf:Property ;
    rdfs:label "insurance" ;
    schema:domainIncludes schema:Patient ;
    schema:rangeIncludes schema:Offer ;
    rdfs:comment "Specifying an insurance scheme for a patient. " .

schema:interactingDrug a rdf:Property ;
    rdfs:label "interactingDrug" ;
    schema:domainIncludes schema:Drug ;
    schema:rangeIncludes schema:Drug ;
    rdfs:comment "Another drug that is known to interact with this drug in a way that impacts the effect of this drug or causes a risk to the patient. Note: disease interactions are typically captured as contraindications." .

schema:interpretation a rdf:Property ;
    rdfs:label "interpretation" ;
    schema:domainIncludes <http://purl.bioontology.org/ontology/SNOMEDCT/404684003>,
        schema:ClinicalFinding,
        schema:DiagnosticProcedure,
        schema:PhysicalExam ;
    schema:rangeIncludes <http://purl.bioontology.org/ontology/SNOMEDCT/243814003>,
        <http://purl.bioontology.org/ontology/SNOMEDCT/277034006> ;
    rdfs:comment "Specifying an interpretation of something or concise and clinically contextualized narrative interpretation of laboratory results or medical test." .

schema:isAvailableGenerically a rdf:Property ;
    rdfs:label "isAvailableGenerically" ;
    schema:domainIncludes schema:Drug ;
    schema:rangeIncludes schema:Boolean ;
    rdfs:comment "True if the drug is available in a generic form (regardless of name)." .

schema:isProprietary a rdf:Property ;
    rdfs:label "isProprietary" ;
    schema:domainIncludes schema:DietarySupplement,
        schema:Drug ;
    schema:rangeIncludes schema:Boolean ;
    rdfs:comment "True if this item's name is a proprietary/brand name (vs. generic name)." .

schema:labelDetails a rdf:Property ;
    rdfs:label "labelDetails" ;
    schema:domainIncludes schema:Drug ;
    schema:rangeIncludes schema:URL ;
    rdfs:comment "Link to the drug's label details." .

schema:laboratoryProcedure a rdf:Property ;
    rdfs:label "laboratoryProcedure" ;
    schema:domainIncludes schema:Patient ;
    schema:rangeIncludes schema:LaboratoryTest ;
    rdfs:comment "Specifying a laboratory procedure resource for a patient or a person." ;
    rdfs:subPropertyOf schema:diagnosticProcedure .

schema:laboratoryResult a rdf:Property ;
    rdfs:label "laboratoryResult" ;
    schema:domainIncludes schema:Patient ;
    schema:rangeIncludes schema:LaboratoryResult ;
    rdfs:comment "Specifying the laboratory test findings for a person" .

schema:lastMenstruationPeriod a rdf:Property ;
    rdfs:label "lastMenstruationPeriod" ;
    schema:domainIncludes <http://purl.bioontology.org/ontology/SNOMEDCT/224526002> ;
    schema:rangeIncludes schema:QuantitativeValue ;
    rdfs:comment "Specifying the last menstruation period of a woman" ;
    rdfs:subPropertyOf schema:interval .

schema:legalStatus a rdf:Property ;
    rdfs:label "legalStatus" ;
    schema:domainIncludes schema:DietarySupplement,
        schema:Drug ;
    schema:rangeIncludes schema:DrugLegalStatus ;
    rdfs:comment "The drug or supplement's legal status, including any controlled substance schedules that apply." .

schema:manufacturer a rdf:Property ;
    rdfs:label "manufacturer" ;
    schema:domainIncludes schema:DietarySupplement,
        schema:Drug,
        schema:Product ;
    schema:rangeIncludes schema:Organization ;
    rdfs:comment "The manufacturer of the product." .

schema:maritalStatus a rdf:Property ;
    rdfs:label "maritalStatus" ;
    schema:domainIncludes schema:Person ;
    schema:rangeIncludes <http://purl.bioontology.org/ontology/SNOMEDCT/365581002> ;
    rdfs:comment "Specifying an agent having the social and/or juridical status of being married or unmarried. " .

schema:maternalRelative a rdf:Property ;
    rdfs:label "maternalRelative" ;
    schema:domainIncludes schema:Person ;
    schema:rangeIncludes schema:Person ;
    rdfs:comment "Specifying the a maternal relative person of this person" ;
    rdfs:subPropertyOf schema:familyMember .

schema:mechanismOfAction a rdf:Property ;
    rdfs:label "mechanismOfAction" ;
    schema:domainIncludes schema:DietarySupplement,
        schema:Drug ;
    schema:rangeIncludes schema:Text ;
    rdfs:comment "The specific biochemical interaction through which this drug or supplement produces its pharmacological effect." .

schema:medicalAdmission a rdf:Property ;
    rdfs:label "medicalAdmission" ;
    schema:domainIncludes schema:MedicalEncounter,
        schema:Person ;
    schema:rangeIncludes <http://purl.bioontology.org/ontology/SNOMEDCT/305056002>,
        schema:AdmissionProcedure,
        schema:MedicalAdmission ;
    rdfs:comment "Specifying admission procedure related to a resource, activity, another procedure, or patient" ;
    rdfs:subPropertyOf schema:medicalEncounter .

schema:medicalBed a rdf:Property ;
    rdfs:label "medicalBed" ;
    schema:domainIncludes <http://purl.bioontology.org/ontology/SNOMEDCT/404684003>,
        schema:ClinicalFinding,
        schema:LifeEvent,
        schema:MedicalIntervention,
        schema:MedicalProcedure,
        schema:Patient ;
    schema:rangeIncludes schema:MedicalBed ;
    rdfs:comment "Specifying the medical bed attended by a patient." ;
    rdfs:subPropertyOf schema:healthFacility .

schema:medicalCase a rdf:Property ;
    rdfs:label "medicalCase" ;
    schema:domainIncludes schema:Patient ;
    schema:rangeIncludes schema:MedicalCase ;
    rdfs:comment "Specifying a medical case for a given medical entity or patient. A medical case is a part of a full medical record of a patient." ;
    rdfs:subPropertyOf schema:medicalRecord .

schema:medicalCertificate a rdf:Property ;
    rdfs:label "medicalCertificate" ;
    schema:domainIncludes schema:Patient ;
    schema:rangeIncludes schema:MedicalCertificate ;
    rdfs:comment "Specifying any medical certificate" ;
    rdfs:subPropertyOf schema:clinicalDocument .

schema:medicalClinic a rdf:Property ;
    rdfs:label "medicalClinic" ;
    schema:domainIncludes <http://purl.bioontology.org/ontology/SNOMEDCT/404684003>,
        schema:ClinicalFinding,
        schema:LifeEvent,
        schema:MedicalIntervention,
        schema:MedicalProcedure,
        schema:Patient ;
    schema:rangeIncludes schema:MedicalClinic ;
    rdfs:comment "Specifying the medical clinic where a procedure or a care event is taking place or attended by a patient." ;
    rdfs:subPropertyOf schema:healthFacility .

schema:medicalCondition a rdf:Property ;
    rdfs:label "medicalCondition" ;
    schema:domainIncludes schema:Patient ;
    schema:rangeIncludes schema:MedicalCondition,
        schema:MorbidityEvent ;
    rdfs:comment "Specifying a medical condition in general, diagnosed or not." .

schema:medicalDepartment a rdf:Property ;
    rdfs:label "medicalDepartment" ;
    schema:domainIncludes <http://purl.bioontology.org/ontology/SNOMEDCT/404684003>,
        schema:ClinicalFinding,
        schema:LifeEvent,
        schema:MedicalEntity,
        schema:MedicalIntervention,
        schema:MedicalProcedure,
        schema:Patient ;
    schema:rangeIncludes schema:MedicalDepartment ;
    rdfs:comment "Specifying the medical department where a procedure or a care event is taking place or attended by a patient." ;
    rdfs:subPropertyOf schema:healthFacility .

schema:medicalDischarge a rdf:Property ;
    rdfs:label "medicalDischarge" ;
    schema:domainIncludes schema:MedicalEncounter,
        schema:Patient ;
    schema:rangeIncludes schema:MedicalDischarge ;
    rdfs:comment "specifying a medical discharge procedure resource of a patient" ;
    rdfs:subPropertyOf schema:medicalEncounter .

schema:medicalIdentifier a rdf:Property ;
    rdfs:label "medicalIdentifier" ;
    schema:domainIncludes <http://purl.bioontology.org/ontology/SNOMEDCT/223366009>,
        schema:HealthcareProfessional,
        schema:Person ;
    schema:rangeIncludes schema:Number ;
    rdfs:comment "Specifying the identification number of a medical entity like care provider identifier number, patient identifier etc." .

schema:medicalIntervention a rdf:Property ;
    rdfs:label "medicalIntervention" ;
    schema:domainIncludes schema:Patient ;
    schema:rangeIncludes schema:MedicalIntervention ;
    rdfs:comment "Specifying the medical intervention resource for the patient or person. Medical intervention is a broad non specific term often used as a set of multiple procedures." .

schema:medicalLetter a rdf:Property ;
    rdfs:label "medicalLetter" ;
    schema:domainIncludes schema:Patient ;
    schema:rangeIncludes schema:ClinicalDocument ;
    rdfs:comment "Specifying any medical letter " ;
    rdfs:subPropertyOf schema:clinicalDocument .

schema:medicalOrder a rdf:Property ;
    rdfs:label "medicalOrder" ;
    schema:domainIncludes schema:Patient ;
    schema:rangeIncludes schema:MedicalOrder ;
    rdfs:comment "Specifying any medical order" ;
    rdfs:subPropertyOf schema:clinicalDocument .

schema:medicalOrderID a rdf:Property ;
    rdfs:label "medicalOrderID" ;
    schema:domainIncludes schema:MedicalOrder ;
    schema:rangeIncludes schema:Text ;
    rdfs:comment "Specifying any medical order" .

schema:medicalPrescription a rdf:Property ;
    rdfs:label "medicalPrescription" ;
    schema:domainIncludes schema:Patient ;
    schema:rangeIncludes <http://purl.bioontology.org/ontology/SNOMEDCT/440545006>,
        schema:MedicalPrescription ;
    rdfs:comment "Linking a patient with his medical order (=written prescription) for the patient Eg. hasPrescription or gotPrescribed. For the provider we use the property prescribingProcedure." ;
    rdfs:subPropertyOf schema:clinicalDocument .

schema:medicalPriority a rdf:Property ;
    rdfs:label "medicalPriority" ;
    schema:domainIncludes <http://purl.bioontology.org/ontology/SNOMEDCT/116154003>,
        schema:Person ;
    schema:rangeIncludes <http://purl.bioontology.org/ontology/SNOMEDCT/272125009>,
        schema:Text ;
    rdfs:comment "specifying the code of the medication dispensation activity" .

schema:medicalReport a rdf:Property ;
    rdfs:label "medicalReport" ;
    schema:domainIncludes schema:MedicalProcedure,
        schema:Patient ;
    schema:rangeIncludes schema:MedicalRecord,
        schema:MedicalReport ;
    rdfs:comment "Specifying any medical report" ;
    rdfs:subPropertyOf schema:clinicalDocument .

schema:medicalRequest a rdf:Property ;
    rdfs:label "medicalRequest" ;
    schema:domainIncludes schema:MedicalIntervention,
        schema:MedicalProcedure,
        schema:Patient ;
    schema:rangeIncludes schema:MedicalRequest ;
    rdfs:comment "Specifying any medical request" .

schema:medicalRequestID a rdf:Property ;
    rdfs:label "medicalRequestID" ;
    schema:domainIncludes schema:MedicalRequest ;
    schema:rangeIncludes schema:Text ;
    rdfs:comment "Specifying a medical request identifier" .

schema:medicalRoom a rdf:Property ;
    rdfs:label "medicalRoom" ;
    schema:domainIncludes <http://purl.bioontology.org/ontology/SNOMEDCT/404684003>,
        schema:ClinicalFinding,
        schema:LifeEvent,
        schema:MedicalIntervention,
        schema:MedicalProcedure,
        schema:Patient ;
    schema:rangeIncludes schema:MedicalRoom ;
    rdfs:comment "Specifying the medical room where a procedure or a care event is taking place or attended by a patient." ;
    rdfs:subPropertyOf schema:healthFacility .

schema:medicalSubSpecialty a rdf:Property ;
    rdfs:label "medicalSubSpecialty" ;
    schema:domainIncludes <http://purl.bioontology.org/ontology/SNOMEDCT/223366009>,
        schema:HealthFacility,
        schema:HealthcareProfessional,
        schema:Person ;
    schema:rangeIncludes schema:MedicalSubSpeciality ;
    rdfs:comment "Specifying the medical sub-specialty of a healthcare provider" ;
    rdfs:subPropertyOf schema:medicalSpecialty .

schema:medicalTransfer a rdf:Property ;
    rdfs:label "medicalTransfer" ;
    schema:domainIncludes schema:MedicalEncounter,
        schema:Person ;
    schema:rangeIncludes schema:MedicalTransfer ;
    rdfs:comment "Specifying a medical transfer event of patient from one place in a health care environment to another" ;
    rdfs:subPropertyOf schema:medicalEncounter .

schema:medicalUnit a rdf:Property ;
    rdfs:label "medicalUnit" ;
    schema:domainIncludes <http://purl.bioontology.org/ontology/SNOMEDCT/404684003>,
        schema:ClinicalFinding,
        schema:LifeEvent,
        schema:MedicalIntervention,
        schema:MedicalProcedure,
        schema:Patient ;
    schema:rangeIncludes schema:MedicalUnit ;
    rdfs:comment "Specifying the medical department unit where a procedure or a care event is taking place or attended by a patient." ;
    rdfs:subPropertyOf schema:healthFacility .

schema:medicalWard a rdf:Property ;
    rdfs:label "medicalWard" ;
    schema:domainIncludes <http://purl.bioontology.org/ontology/SNOMEDCT/404684003>,
        schema:ClinicalFinding,
        schema:LifeEvent,
        schema:MedicalIntervention,
        schema:MedicalProcedure,
        schema:Patient ;
    schema:rangeIncludes schema:MedicalWard ;
    rdfs:comment "Specifying the medical ward (a set of rooms) where a procedure or a care event is taking place or attended by a patient." ;
    rdfs:subPropertyOf schema:healthFacility .

schema:medicationProcedure a rdf:Property ;
    rdfs:label "medicationProcedure" ;
    schema:domainIncludes schema:Patient ;
    schema:rangeIncludes schema:MedicalTherapy ;
    rdfs:comment "Specifying a medication procedure resource for a patient or a person" ;
    rdfs:subPropertyOf schema:therapeuticProcedure .

schema:medicationTime a rdf:Property ;
    rdfs:label "medicationTime" ;
    schema:domainIncludes schema:Drug ;
    schema:rangeIncludes schema:DateTime ;
    rdfs:comment "specifying the medication time i.e when the drug has or was administrated" .

schema:medicineSystem a rdf:Property ;
    rdfs:label "medicineSystem" ;
    schema:domainIncludes schema:MedicalEntity ;
    schema:rangeIncludes schema:MedicineSystem ;
    rdfs:comment "The system of medicine that includes this MedicalEntity, for example 'evidence-based', 'homeopathic', 'chiropractic', etc." .

schema:menopause a rdf:Property ;
    rdfs:label "menopause" ;
    schema:domainIncludes schema:Person ;
    schema:rangeIncludes <http://purl.bioontology.org/ontology/SNOMEDCT/276477006>,
        schema:Menopause ;
    rdfs:comment "Specifying the menopause event of a women " ;
    rdfs:subPropertyOf schema:gynObsHistory .

schema:menstruation a rdf:Property ;
    rdfs:label "menstruation" ;
    schema:domainIncludes <http://purl.bioontology.org/ontology/SNOMEDCT/224526002> ;
    schema:rangeIncludes schema:Menstruation ;
    rdfs:comment "Specifying the menstruation event of a women " ;
    rdfs:subPropertyOf schema:gynObsHistory .

schema:menstruationPeriod a rdf:Property ;
    rdfs:label "menstruationPeriod" ;
    schema:domainIncludes <http://purl.bioontology.org/ontology/SNOMEDCT/224526002> ;
    schema:rangeIncludes schema:QuantitativeValue ;
    rdfs:comment "Specifying the menstruation period description event of a women " ;
    rdfs:subPropertyOf schema:interval .

schema:mentalHealthHistory a rdf:Property ;
    rdfs:label "mentalHealthHistory" ;
    schema:domainIncludes schema:Person ;
    schema:rangeIncludes schema:MentalHealthHistory ;
    rdfs:comment "Specifying the mental health history for a patient" ;
    rdfs:subPropertyOf schema:personalHistory .

schema:mother a rdf:Property ;
    rdfs:label "mother" ;
    schema:domainIncludes schema:Person ;
    schema:rangeIncludes schema:Person ;
    rdfs:comment "Specifying a mother (parent) of this person when no other specifications are given." ;
    rdfs:subPropertyOf schema:parent .

schema:muscleAction a rdf:Property ;
    rdfs:label "muscleAction" ;
    schema:domainIncludes schema:Muscle ;
    schema:rangeIncludes schema:Text ;
    rdfs:comment "The movement the muscle generates." .

schema:naturalProgression a rdf:Property ;
    rdfs:label "naturalProgression" ;
    schema:domainIncludes schema:MedicalCondition ;
    schema:rangeIncludes schema:Text ;
    rdfs:comment "The expected progression of the condition if it is not treated and allowed to progress naturally." .

schema:nerve a rdf:Property ;
    rdfs:label "nerve" ;
    schema:domainIncludes schema:Muscle ;
    schema:rangeIncludes schema:Nerve ;
    rdfs:comment "The underlying innervation associated with the muscle." .

schema:nerveMotor a rdf:Property ;
    rdfs:label "nerveMotor" ;
    schema:domainIncludes schema:Nerve ;
    schema:rangeIncludes schema:Muscle ;
    rdfs:comment "The neurological pathway extension that involves muscle control." .

schema:newborn a rdf:Property ;
    rdfs:label "newborn" ;
    schema:domainIncludes <http://purl.bioontology.org/ontology/SNOMEDCT/360149000>,
        schema:LifeEvent,
        schema:MedicalIntervention,
        schema:MedicalProcedure,
        schema:Person ;
    schema:rangeIncludes <http://purl.bioontology.org/ontology/SNOMEDCT/133933007> ;
    rdfs:comment "Specifying the newborn person " .

schema:nonProprietaryName a rdf:Property ;
    rdfs:label "nonProprietaryName" ;
    schema:domainIncludes schema:DietarySupplement,
        schema:Drug ;
    schema:rangeIncludes schema:Text ;
    rdfs:comment "The generic name of this drug or supplement." .

schema:normalRange a rdf:Property ;
    rdfs:label "normalRange" ;
    schema:domainIncludes schema:MedicalTest ;
    schema:rangeIncludes schema:Text ;
    rdfs:comment "Range of acceptable values for a typical patient, when applicable." .

schema:nutrition a rdf:Property ;
    rdfs:label "nutrition" ;
    schema:domainIncludes schema:Recipe ;
    schema:rangeIncludes schema:NutritionInformation ;
    rdfs:comment "Nutrition information about the recipe." .

schema:observable a rdf:Property ;
    rdfs:label "observable" ;
    schema:domainIncludes schema:Patient ;
    schema:rangeIncludes <http://purl.bioontology.org/ontology/SNOMEDCT/363787002> ;
    rdfs:comment "Specifying a clinical observable of a patient not necessarily through a clinical examination. example: a swelling, etc" .

schema:occupationalHistory a rdf:Property ;
    rdfs:label "occupationalHistory" ;
    schema:domainIncludes schema:Person ;
    schema:rangeIncludes schema:OccupationalHistory ;
    rdfs:comment "Specifying the occupational history resource of the patient or person." ;
    rdfs:subPropertyOf schema:socialHistory .

schema:onsetMode a rdf:Property ;
    rdfs:label "onsetMode" ;
    schema:domainIncludes schema:MedicalCondition ;
    schema:rangeIncludes schema:OnsetMode ;
    rdfs:comment "Specifying a way a process, an illness, or an event comes into existence" .

schema:origin a rdf:Property ;
    rdfs:label "origin" ;
    schema:domainIncludes schema:Muscle ;
    schema:rangeIncludes schema:AnatomicalStructure ;
    rdfs:comment "The place or point where a muscle arises." .

schema:originatesFrom a rdf:Property ;
    rdfs:label "originatesFrom" ;
    schema:domainIncludes schema:LymphaticVessel ;
    schema:rangeIncludes schema:Vessel ;
    rdfs:comment "The vasculature the lymphatic structure originates, or afferents, from." .

schema:outcome a rdf:Property ;
    rdfs:label "outcome" ;
    schema:domainIncludes schema:MedicalStudy ;
    schema:rangeIncludes schema:Text ;
    rdfs:comment "Expected or actual outcomes of the study." .

schema:overdosage a rdf:Property ;
    rdfs:label "overdosage" ;
    schema:domainIncludes schema:Drug ;
    schema:rangeIncludes schema:Text ;
    rdfs:comment "Any information related to overdose on a drug, including signs or symptoms, treatments, contact information for emergency response." .

schema:palliativeProcedure a rdf:Property ;
    rdfs:label "palliativeProcedure" ;
    schema:domainIncludes schema:Patient ;
    schema:rangeIncludes schema:PalliativeProcedure ;
    rdfs:comment "Specifying a palliative procedure resource for a patient or a person" ;
    rdfs:subPropertyOf schema:therapeuticProcedure .

schema:parity a rdf:Property ;
    rdfs:label "parity" ;
    schema:domainIncludes <http://purl.bioontology.org/ontology/SNOMEDCT/224526002>,
        schema:Person ;
    schema:rangeIncludes schema:Number ;
    rdfs:comment "Parity is defined as the number of times that she has given birth to a fetus with a gestational age of 24 weeks or more, regardless of whether the child was born alive or was stillborn." .

schema:partOfSystem a rdf:Property ;
    rdfs:label "partOfSystem" ;
    schema:domainIncludes schema:AnatomicalStructure ;
    schema:rangeIncludes schema:AnatomicalSystem ;
    rdfs:comment "The anatomical or organ system that this structure is part of." ;
    rdfs:subPropertyOf schema:isPartOf .

schema:pastMedicalHistory a rdf:Property ;
    rdfs:label "pastMedicalHistory" ;
    schema:domainIncludes schema:Person ;
    schema:rangeIncludes schema:PastMedicalHistory ;
    rdfs:comment "Specifying the past medical history of a patient" ;
    rdfs:subPropertyOf schema:personalHistory .

schema:paternalRelative a rdf:Property ;
    rdfs:label "paternalRelative" ;
    schema:domainIncludes schema:Person ;
    schema:rangeIncludes schema:Person ;
    rdfs:comment "Specifying the a paternal relative person of this person" ;
    rdfs:subPropertyOf schema:familyMember .

schema:pathophysiology a rdf:Property ;
    rdfs:label "pathophysiology" ;
    schema:domainIncludes schema:MedicalCondition,
        schema:PhysicalActivity ;
    schema:rangeIncludes schema:Text ;
    rdfs:comment "Changes in the normal mechanical, physical, and biochemical functions that are associated with this activity or condition." .

schema:patientCode a rdf:Property ;
    rdfs:label "patientCode" ;
    schema:domainIncludes <http://purl.bioontology.org/ontology/SNOMEDCT/404684003>,
        schema:Patient ;
    schema:rangeIncludes schema:Text ;
    rdfs:comment "Specifying a patient code. Used in general cross-hospitals" .

schema:patientID a rdf:Property ;
    rdfs:label "patientID" ;
    schema:domainIncludes <http://purl.bioontology.org/ontology/SNOMEDCT/404684003>,
        schema:Patient ;
    schema:rangeIncludes schema:Text ;
    rdfs:comment "Specifying a digit ID for the patient within a healthcare facility. Therefore a patient can have multiple ID specific to each hospitals" .

schema:phase a rdf:Property ;
    rdfs:label "phase" ;
    schema:domainIncludes schema:MedicalTrial ;
    schema:rangeIncludes schema:Text ;
    rdfs:comment "The phase of the trial." .

schema:physicalActivity a rdf:Property ;
    rdfs:label "physicalActivity" ;
    schema:domainIncludes schema:Person ;
    schema:rangeIncludes schema:PhysicalActivity,
        schema:RecreationalHistory ;
    rdfs:comment "Specifying the physical activity  resource of the patient or person." .

schema:physicalExamination a rdf:Property ;
    rdfs:label "physicalExamination" ;
    schema:domainIncludes <http://purl.bioontology.org/ontology/SNOMEDCT/404684003>,
        schema:ClinicalFinding,
        schema:LifeEvent,
        schema:MedicalIntervention,
        schema:MedicalProcedure,
        schema:Patient ;
    schema:rangeIncludes schema:PhysicalExam ;
    rdfs:comment "Specifying a physical examination procedure resource for a patient or a person" ;
    rdfs:subPropertyOf schema:diagnosticProcedure .

schema:physiologicalBenefits a rdf:Property ;
    rdfs:label "physiologicalBenefits" ;
    schema:domainIncludes schema:Diet ;
    schema:rangeIncludes schema:Text ;
    rdfs:comment "Specific physiologic benefits associated to the plan." .

schema:physiologicalRole a rdf:Property ;
    rdfs:label "physiologicalRole" ;
    schema:domainIncludes schema:MedicalEntity ;
    schema:rangeIncludes schema:PhysiologicalEntity ;
    rdfs:comment "Specifying any physiological role of something" .

schema:playsRole a rdf:Property ;
    rdfs:label "playsRole" ;
    schema:domainIncludes schema:MedicalEntity ;
    schema:rangeIncludes schema:MedicalEntity ;
    rdfs:comment "Specifying the role played by an agent " .

schema:population a rdf:Property ;
    rdfs:label "population" ;
    schema:domainIncludes schema:MedicalStudy ;
    schema:rangeIncludes schema:Text ;
    rdfs:comment "Any characteristics of the population used in the study, e.g. 'males under 65'." .

schema:possibleCause a rdf:Property ;
    rdfs:label "possibleCause" ;
    schema:domainIncludes schema:MedicalEntity ;
    schema:rangeIncludes schema:MedicalEntity ;
    rdfs:comment "Specifying a possible cause of something" ;
    rdfs:subPropertyOf schema:cause .

schema:possibleComplication a rdf:Property ;
    rdfs:label "possibleComplication" ;
    schema:domainIncludes schema:MedicalCondition ;
    schema:rangeIncludes schema:Text ;
    rdfs:comment "A possible unexpected and unfavorable evolution of a medical condition. Complications may include worsening of the signs or symptoms of the disease, extension of the condition to other organ systems, etc." .

schema:possibleTreatment a rdf:Property ;
    rdfs:label "possibleTreatment" ;
    schema:domainIncludes schema:MedicalCondition,
        schema:MedicalSignOrSymptom ;
    schema:rangeIncludes schema:MedicalTherapy ;
    rdfs:comment "A possible treatment to address this condition, sign or symptom." ;
    rdfs:subPropertyOf schema:treatment .

schema:postOp a rdf:Property ;
    rdfs:label "postOp" ;
    schema:domainIncludes schema:MedicalDevice ;
    schema:rangeIncludes schema:Text ;
    rdfs:comment "A description of the postoperative procedures, care, and/or followups for this device." .

schema:preOp a rdf:Property ;
    rdfs:label "preOp" ;
    schema:domainIncludes schema:MedicalDevice ;
    schema:rangeIncludes schema:Text ;
    rdfs:comment "A description of the workup, testing, and other preparations required before implanting this device." .

schema:pregnancy a rdf:Property ;
    rdfs:label "pregnancy" ;
    schema:domainIncludes schema:Person ;
    schema:rangeIncludes schema:Gravidity ;
    rdfs:comment "Specifying the resource as the pregnancy event or period related to the patient not differentiating if the pregnancy gave a birth or not. Should be noted that gravidity property is a data property instead. " .

schema:pregnancyCategory a rdf:Property ;
    rdfs:label "pregnancyCategory" ;
    schema:domainIncludes schema:Drug ;
    schema:rangeIncludes schema:DrugPregnancyCategory ;
    rdfs:comment "Pregnancy category of this drug." .

schema:pregnancyWarning a rdf:Property ;
    rdfs:label "pregnancyWarning" ;
    schema:domainIncludes schema:Drug ;
    schema:rangeIncludes schema:Text ;
    rdfs:comment "Any precaution, guidance, contraindication, etc. related to this drug's use during pregnancy." .

schema:prepTime a rdf:Property ;
    rdfs:label "prepTime" ;
    schema:domainIncludes schema:Recipe ;
    schema:rangeIncludes schema:Duration ;
    rdfs:comment "The length of time it takes to prepare the recipe, in ISO 8601 duration format." .

schema:preparation a rdf:Property ;
    rdfs:label "preparation" ;
    schema:domainIncludes schema:MedicalProcedure ;
    schema:rangeIncludes schema:Text ;
    rdfs:comment "Typical preparation that a patient must undergo before having the procedure performed." .

schema:prescribingInfo a rdf:Property ;
    rdfs:label "prescribingInfo" ;
    schema:domainIncludes schema:Drug ;
    schema:rangeIncludes schema:URL ;
    rdfs:comment "Link to prescribing information for the drug." .

schema:prescribingProcedure a rdf:Property ;
    rdfs:label "prescribingProcedure" ;
    schema:domainIncludes <http://purl.bioontology.org/ontology/SNOMEDCT/223366009>,
        schema:HealthcareProfessional,
        schema:Patient ;
    schema:rangeIncludes schema:PrescribingProcedure ;
    rdfs:comment "Specifying a prescribing procedure resource for a patient or a person. This property is linking a patient or a provider to the procedure. The procedure has as an output a prescription." ;
    rdfs:subPropertyOf schema:therapeuticProcedure .

schema:prescriptionStatus a rdf:Property ;
    rdfs:label "prescriptionStatus" ;
    schema:domainIncludes schema:Drug ;
    schema:rangeIncludes schema:DrugPrescriptionStatus ;
    rdfs:comment "Indicates whether this drug is available by prescription or over-the-counter." .

schema:procedureActivity a rdf:Property ;
    rdfs:label "procedureActivity" ;
    schema:domainIncludes schema:MedicalProcedure ;
    schema:rangeIncludes schema:MedicalProcedureActivity ;
    rdfs:comment "Specifying the medical procedure activity. This can be another medical procedure" ;
    rdfs:subPropertyOf schema:medicalProcedure .

schema:procedurePhase a rdf:Property ;
    rdfs:label "procedurePhase" ;
    schema:domainIncludes schema:MedicalProcedure ;
    schema:rangeIncludes schema:MedicalProcedurePhase ;
    rdfs:comment "Specifying the medical procedure phase, specially when a procedure is performed in multiple phases." ;
    rdfs:subPropertyOf schema:medicalProcedure .

schema:procedureType a rdf:Property ;
    rdfs:label "procedureType" ;
    schema:domainIncludes schema:MedicalProcedure ;
    schema:rangeIncludes schema:MedicalProcedureType ;
    rdfs:comment "The type of procedure, for example Surgical, Noninvasive, or Percutaneous." .

schema:publicationType a rdf:Property ;
    rdfs:label "publicationType" ;
    schema:domainIncludes schema:MedicalScholarlyArticle ;
    schema:rangeIncludes schema:Text ;
    rdfs:comment "The type of the medical article, taken from the US NLM MeSH publication type catalog. See: http://www.nlm.nih.gov/mesh/pubtypes.html" .

schema:purpose a rdf:Property ;
    rdfs:label "purpose" ;
    schema:domainIncludes schema:AllocateAction,
        schema:MedicalDevice,
        schema:PayAction ;
    schema:rangeIncludes schema:MedicalDevicePurpose,
        schema:Thing ;
    rdfs:comment "A goal towards an action is taken. Can be concrete or abstract." .

schema:race a rdf:Property ;
    rdfs:label "race" ;
    schema:domainIncludes schema:Person ;
    schema:rangeIncludes schema:Race ;
    rdfs:comment "Specifying a race group or anthropological family as origin of the person. Race and Ethnicity as well as religious beliefs are in most cases not given in EHR, and collecting this info is often seen as illegal. Please check local regulations before using this property " .

schema:rankOrder a rdf:Property ;
    rdfs:label "rankOrder" ;
    schema:domainIncludes schema:MedicalEntity ;
    schema:rangeIncludes schema:Number ;
    rdfs:comment "The rank order number of something. Typically used together with schema:numerator and schema:denominator. eg. refill number 4 out of 10." .

schema:recipe a rdf:Property ;
    rdfs:label "recipe" ;
    schema:domainIncludes schema:CookAction ;
    schema:rangeIncludes schema:Recipe ;
    rdfs:comment "A sub property of instrument. The recipe/instructions used to perform the action." ;
    rdfs:subPropertyOf schema:instrument .

schema:recipeCategory a rdf:Property ;
    rdfs:label "recipeCategory" ;
    schema:domainIncludes schema:Recipe ;
    schema:rangeIncludes schema:Text ;
    rdfs:comment "The category of the recipe—for example, appetizer, entree, etc." .

schema:recipeCuisine a rdf:Property ;
    rdfs:label "recipeCuisine" ;
    schema:domainIncludes schema:Recipe ;
    schema:rangeIncludes schema:Text ;
    rdfs:comment "The cuisine of the recipe (for example, French or Ethiopian)." .

schema:recipeIngredient a rdf:Property ;
    rdfs:label "recipeIngredient" ;
    schema:domainIncludes schema:Recipe ;
    schema:rangeIncludes schema:Text ;
    rdfs:comment "A single ingredient used in the recipe, e.g. sugar, flour or garlic." .

schema:recipeInstructions a rdf:Property ;
    rdfs:label "recipeInstructions" ;
    schema:domainIncludes schema:Recipe ;
    schema:rangeIncludes schema:ItemList,
        schema:Text ;
    rdfs:comment "A step or instruction involved in making the recipe." .

schema:recipeYield a rdf:Property ;
    rdfs:label "recipeYield" ;
    schema:domainIncludes schema:Recipe ;
    schema:rangeIncludes schema:Text ;
    rdfs:comment "The quantity produced by the recipe (for example, number of people served, number of servings, etc)." .

schema:recognizingAuthority a rdf:Property ;
    rdfs:label "recognizingAuthority" ;
    schema:domainIncludes schema:MedicalEntity ;
    schema:rangeIncludes schema:Organization ;
    rdfs:comment "If applicable, the organization that officially recognizes this entity as part of its endorsed system of medicine." .

schema:recommendationStrength a rdf:Property ;
    rdfs:label "recommendationStrength" ;
    schema:domainIncludes schema:MedicalGuidelineRecommendation ;
    schema:rangeIncludes schema:Text ;
    rdfs:comment "Strength of the guideline's recommendation (e.g. 'class I')." .

schema:recommendedIntake a rdf:Property ;
    rdfs:label "recommendedIntake" ;
    schema:domainIncludes schema:DietarySupplement ;
    schema:rangeIncludes schema:RecommendedDoseSchedule ;
    rdfs:comment "Recommended intake of this supplement for a given population as defined by a specific recommending authority." .

schema:recommendedTreatment a rdf:Property ;
    rdfs:label "recommendedTreatment" ;
    schema:domainIncludes schema:MedicalCondition,
        schema:Patient ;
    schema:rangeIncludes schema:Drug,
        schema:TherapeuticProcedure ;
    rdfs:comment "Specifying a recommended treatment of a given patient (like pediatric person) or a medical condition." ;
    rdfs:subPropertyOf schema:treatment .

schema:referredBy a rdf:Property ;
    rdfs:label "referredBy" ;
    schema:domainIncludes <http://purl.bioontology.org/ontology/SNOMEDCT/116154003>,
        schema:Person ;
    schema:rangeIncludes schema:HealthFacility,
        schema:Person ;
    rdfs:comment "Specifying a referrer for a patient in general, but can be applied to other medical entities" .

schema:referringPhysician a rdf:Property ;
    rdfs:label "referringPhysician" ;
    schema:domainIncludes schema:Patient ;
    schema:rangeIncludes schema:HealthcareProfessional ;
    rdfs:comment "A healthcare provider referring a patient to another healthcare provider." ;
    rdfs:subPropertyOf schema:careProvider .

schema:refill a rdf:Property ;
    rdfs:label "refill" ;
    schema:domainIncludes schema:Patient ;
    schema:rangeIncludes schema:Refill ;
    rdfs:comment "Specifying the history or plan of refills that can be done before a new prescription is needed, related to a given prescription." .

schema:regionDrained a rdf:Property ;
    rdfs:label "regionDrained" ;
    schema:domainIncludes schema:LymphaticVessel,
        schema:Vein ;
    schema:rangeIncludes schema:AnatomicalStructure,
        schema:AnatomicalSystem ;
    rdfs:comment "The anatomical or organ system drained by this vessel; generally refers to a specific part of an organ." .

schema:regionsAllowed a rdf:Property ;
    rdfs:label "regionsAllowed" ;
    schema:domainIncludes schema:MediaObject ;
    schema:rangeIncludes schema:Place ;
    rdfs:comment "The regions where the media is allowed. If not specified, then it's assumed to be allowed everywhere. Specify the countries in ISO 3166 format." .

schema:relatedAnatomy a rdf:Property ;
    rdfs:label "relatedAnatomy" ;
    schema:domainIncludes schema:SuperficialAnatomy ;
    schema:rangeIncludes schema:AnatomicalStructure,
        schema:AnatomicalSystem ;
    rdfs:comment "Anatomical systems or structures that relate to the superficial anatomy." .

schema:relatedCondition a rdf:Property ;
    rdfs:label "relatedCondition" ;
    schema:domainIncludes schema:AnatomicalStructure,
        schema:AnatomicalSystem,
        schema:SuperficialAnatomy ;
    schema:rangeIncludes schema:MedicalCondition ;
    rdfs:comment "A medical condition associated with this anatomy." .

schema:relatedDrug a rdf:Property ;
    rdfs:label "relatedDrug" ;
    schema:domainIncludes schema:Drug ;
    schema:rangeIncludes schema:Drug ;
    rdfs:comment "Any other drug related to this one, for example commonly-prescribed alternatives." .

schema:relatedEncounter a rdf:Property ;
    rdfs:label "relatedEncounter" ;
    schema:domainIncludes schema:ClinicalDocument,
        schema:LifeEvent,
        schema:MedicalProcedure,
        schema:MedicalRecord,
        schema:MedicalScore ;
    schema:rangeIncludes schema:MedicalEncounter ;
    rdfs:comment "Specifying a medical encounter procedure resource related to other procedure" .

schema:relatedStructure a rdf:Property ;
    rdfs:label "relatedStructure" ;
    schema:domainIncludes schema:AnatomicalSystem ;
    schema:rangeIncludes schema:AnatomicalStructure ;
    rdfs:comment "Related anatomical structure(s) that are not part of the system but relate or connect to it, such as vascular bundles associated with an organ system." .

schema:relatedTherapy a rdf:Property ;
    rdfs:label "relatedTherapy" ;
    schema:domainIncludes schema:AnatomicalStructure,
        schema:AnatomicalSystem,
        schema:SuperficialAnatomy ;
    schema:rangeIncludes schema:MedicalTherapy ;
    rdfs:comment "A medical therapy related to this anatomy." .

schema:relevantSpecialty a rdf:Property ;
    rdfs:label "relevantSpecialty" ;
    schema:domainIncludes schema:MedicalEntity ;
    schema:rangeIncludes schema:MedicalSpecialty ;
    rdfs:comment "If applicable, a medical specialty in which this entity is relevant." .

schema:religiousBelief a rdf:Property ;
    rdfs:label "religiousBelief" ;
    schema:domainIncludes schema:Person ;
    schema:rangeIncludes schema:ReligiousBelief ;
    rdfs:comment "Specifying the religion beliefs of a person. Someone can have multiple religion beliefs." ;
    rdfs:subPropertyOf schema:religionGroup .

schema:residenceHistory a rdf:Property ;
    rdfs:label "residenceHistory" ;
    schema:domainIncludes schema:Person ;
    schema:rangeIncludes schema:ResidenceHistory ;
    rdfs:comment "Specifying the residence history resource of the patient or person." ;
    rdfs:subPropertyOf schema:socialHistory .

schema:residentialStatus a rdf:Property ;
    rdfs:label "residentialStatus" ;
    schema:domainIncludes schema:Person ;
    schema:rangeIncludes schema:Thing ;
    rdfs:comment "Specifying the act of dwelling in a place. This status is linked to an address and period of the time" .

schema:resistantTo a rdf:Property ;
    rdfs:label "resistantTo" ;
    schema:domainIncludes <http://purl.bioontology.org/ontology/SNOMEDCT/264395009> ;
    schema:rangeIncludes schema:PharmaceuticalSubstance ;
    rdfs:comment "Specifying pharmacological substance a micro-organism is resistant to." .

schema:riskFactor a rdf:Property ;
    rdfs:label "riskFactor" ;
    schema:domainIncludes schema:MedicalCondition ;
    schema:rangeIncludes schema:MedicalRiskFactor ;
    rdfs:comment "A modifiable or non-modifiable factor that increases the risk of a patient contracting this condition, e.g. age,  coexisting condition." .

schema:risks a rdf:Property ;
    rdfs:label "risks" ;
    schema:domainIncludes schema:Diet ;
    schema:rangeIncludes schema:Text ;
    rdfs:comment "Specific physiologic risks associated to the plan." .

schema:runsTo a rdf:Property ;
    rdfs:label "runsTo" ;
    schema:domainIncludes schema:LymphaticVessel ;
    schema:rangeIncludes schema:Vessel ;
    rdfs:comment "The vasculature the lymphatic structure runs, or efferents, to." .

schema:safetyConsideration a rdf:Property ;
    rdfs:label "safetyConsideration" ;
    schema:domainIncludes schema:DietarySupplement ;
    schema:rangeIncludes schema:Text ;
    rdfs:comment "Any potential safety concern associated with the supplement. May include interactions with other drugs and foods, pregnancy, breastfeeding, known adverse reactions, and documented efficacy of the supplement." .

schema:secondaryPrevention a rdf:Property ;
    rdfs:label "secondaryPrevention" ;
    schema:domainIncludes schema:MedicalCondition ;
    schema:rangeIncludes schema:MedicalTherapy ;
    rdfs:comment "A preventative therapy used to prevent reoccurrence of the medical condition after an initial episode of the condition." .

schema:sensoryUnit a rdf:Property ;
    rdfs:label "sensoryUnit" ;
    schema:domainIncludes schema:Nerve ;
    schema:rangeIncludes schema:AnatomicalStructure,
        schema:SuperficialAnatomy ;
    rdfs:comment "The neurological pathway extension that inputs and sends information to the brain or spinal cord." .

schema:seriousAdverseOutcome a rdf:Property ;
    rdfs:label "seriousAdverseOutcome" ;
    schema:domainIncludes schema:MedicalDevice,
        schema:MedicalTherapy ;
    schema:rangeIncludes schema:MedicalEntity ;
    rdfs:comment "A possible serious complication and/or serious side effect of this therapy. Serious adverse outcomes include those that are life-threatening; result in death, disability, or permanent damage; require hospitalization or prolong existing hospitalization; cause congenital anomalies or birth defects; or jeopardize the patient and may require medical or surgical intervention to prevent one of the outcomes in this definition." .

schema:severity a rdf:Property ;
    rdfs:label "severity" ;
    schema:domainIncludes schema:MedicalEntity ;
    schema:rangeIncludes schema:Severity ;
    rdfs:comment "Specifying a severity evaluation of a disease: typically by classification resource or ranking scale: mild, moderate, severe, life threatening or fatal" .

schema:sexualBehaviour a rdf:Property ;
    rdfs:label "sexualBehaviour" ;
    schema:domainIncludes schema:Person ;
    schema:rangeIncludes schema:SexualBehaviour ;
    rdfs:comment "Specifying the sexual behaviour resource of  a patient" ;
    rdfs:subPropertyOf schema:lifestyleOrHabit .

schema:signDetected a rdf:Property ;
    rdfs:label "signDetected" ;
    schema:domainIncludes schema:MedicalTest ;
    schema:rangeIncludes schema:MedicalSign ;
    rdfs:comment "A sign detected by the test." .

schema:significance a rdf:Property ;
    rdfs:label "significance" ;
    schema:domainIncludes schema:SuperficialAnatomy ;
    schema:rangeIncludes schema:Text ;
    rdfs:comment "The significance associated with the superficial anatomy; as an example, how characteristics of the superficial anatomy can suggest underlying medical conditions or courses of treatment." .

schema:smoking a rdf:Property ;
    rdfs:label "smoking" ;
    schema:domainIncludes schema:Person ;
    schema:rangeIncludes schema:Smoking ;
    rdfs:comment "Describing the smoking habit resource for the patient" ;
    rdfs:subPropertyOf schema:lifestyleOrHabit .

schema:source a rdf:Property ;
    rdfs:label "source" ;
    schema:domainIncludes schema:Artery ;
    schema:rangeIncludes schema:AnatomicalStructure ;
    rdfs:comment "The anatomical or organ system that the artery originates from." .

schema:sponsor a rdf:Property ;
    rdfs:label "sponsor" ;
    schema:domainIncludes schema:MedicalStudy ;
    schema:rangeIncludes schema:Organization ;
    rdfs:comment "Sponsor of the study." .

schema:stage a rdf:Property ;
    rdfs:label "stage" ;
    schema:domainIncludes schema:MedicalCondition ;
    schema:rangeIncludes schema:MedicalConditionStage ;
    rdfs:comment "The stage of the condition, if applicable." .

schema:stageAsNumber a rdf:Property ;
    rdfs:label "stageAsNumber" ;
    schema:domainIncludes schema:MedicalConditionStage ;
    schema:rangeIncludes schema:Number ;
    rdfs:comment "The stage represented as a number, e.g. 3." .

schema:strengthUnit a rdf:Property ;
    rdfs:label "strengthUnit" ;
    schema:domainIncludes schema:DrugStrength ;
    schema:rangeIncludes schema:Text ;
    rdfs:comment "The units of an active ingredient's strength, e.g. mg." .

schema:strengthValue a rdf:Property ;
    rdfs:label "strengthValue" ;
    schema:domainIncludes schema:DrugStrength ;
    schema:rangeIncludes schema:Number ;
    rdfs:comment "The value of an active ingredient's strength, e.g. 325." .

schema:structuralClass a rdf:Property ;
    rdfs:label "structuralClass" ;
    schema:domainIncludes schema:Joint ;
    schema:rangeIncludes schema:Text ;
    rdfs:comment "The name given to how bone physically connects to each other." .

schema:study a rdf:Property ;
    rdfs:label "study" ;
    schema:domainIncludes schema:MedicalEntity ;
    schema:rangeIncludes schema:MedicalStudy ;
    rdfs:comment "A medical study or trial related to this entity." .

schema:studyDesign a rdf:Property ;
    rdfs:label "studyDesign" ;
    schema:domainIncludes schema:MedicalObservationalStudy ;
    schema:rangeIncludes schema:MedicalObservationalStudyDesign ;
    rdfs:comment "Specifics about the observational study design (enumerated)." .

schema:studyLocation a rdf:Property ;
    rdfs:label "studyLocation" ;
    schema:domainIncludes schema:MedicalStudy ;
    schema:rangeIncludes schema:AdministrativeArea ;
    rdfs:comment "The location in which the study is taking/took place." .

schema:studySubject a rdf:Property ;
    rdfs:label "studySubject" ;
    schema:domainIncludes schema:MedicalStudy ;
    schema:rangeIncludes schema:MedicalEntity ;
    rdfs:comment "A subject of the study, i.e. one of the medical conditions, therapies, devices, drugs, etc. investigated by the study." .

schema:subStageSuffix a rdf:Property ;
    rdfs:label "subStageSuffix" ;
    schema:domainIncludes schema:MedicalConditionStage ;
    schema:rangeIncludes schema:Text ;
    rdfs:comment "The substage, e.g. 'a' for Stage IIIa." .

schema:subStructure a rdf:Property ;
    rdfs:label "subStructure" ;
    schema:domainIncludes schema:AnatomicalStructure ;
    schema:rangeIncludes schema:AnatomicalStructure ;
    rdfs:comment "Component (sub-)structure(s) that comprise this anatomical structure." .

schema:subTest a rdf:Property ;
    rdfs:label "subTest" ;
    schema:domainIncludes schema:MedicalTestPanel ;
    schema:rangeIncludes schema:MedicalTest ;
    rdfs:comment "A component test of the panel." .

schema:substanceUseOrAbuse a rdf:Property ;
    rdfs:label "substanceUseOrAbuse" ;
    schema:domainIncludes schema:Person ;
    schema:rangeIncludes schema:SubstanceUseOrAbuse ;
    rdfs:comment "Describing the substance use or abuse resource of the person" ;
    rdfs:subPropertyOf schema:lifestyleOrHabit .

schema:subtype a rdf:Property ;
    rdfs:label "subtype" ;
    schema:domainIncludes schema:MedicalCondition ;
    schema:rangeIncludes schema:Text ;
    rdfs:comment "A more specific type of the condition, where applicable, for example 'Type 1 Diabetes', 'Type 2 Diabetes', or 'Gestational Diabetes' for Diabetes." .

schema:supplyTo a rdf:Property ;
    rdfs:label "supplyTo" ;
    schema:domainIncludes schema:Artery ;
    schema:rangeIncludes schema:AnatomicalStructure ;
    rdfs:comment "The area to which the artery supplies blood." .

schema:surgicalProcedure a rdf:Property ;
    rdfs:label "surgicalProcedure" ;
    schema:domainIncludes schema:Patient ;
    schema:rangeIncludes schema:SurgicalProcedure ;
    rdfs:comment "Specifying a surgical procedure resource for a patient or a person" ;
    rdfs:subPropertyOf schema:medicalProcedure .

schema:susceptibleTo a rdf:Property ;
    rdfs:label "susceptibleTo" ;
    schema:domainIncludes <http://purl.bioontology.org/ontology/SNOMEDCT/264395009> ;
    schema:rangeIncludes schema:PharmaceuticalSubstance ;
    rdfs:comment "Specifying a pharmacological substance a microorganism is susceptible to." .

schema:systemicReview a rdf:Property ;
    rdfs:label "systemicReview" ;
    schema:domainIncludes schema:AnamnesisProcedure,
        schema:ClinicalDocument,
        schema:MedicalRecord,
        schema:Patient ;
    schema:rangeIncludes schema:SystemicReview ;
    rdfs:comment "Specifying a systemic review resource as a part of  anamnesis" .

schema:systolicBloodPressure a rdf:Property ;
    rdfs:label "systolicBloodPressure" ;
    schema:domainIncludes schema:Person ;
    schema:rangeIncludes <http://purl.bioontology.org/ontology/SNOMEDCT/271649006> ;
    rdfs:comment "Specifying  systolic arterial blood pressure of a patient." ;
    rdfs:subPropertyOf schema:bloodPressure .

schema:totalTime a rdf:Property ;
    rdfs:label "totalTime" ;
    schema:domainIncludes schema:MedicalProcedure,
        schema:Recipe ;
    schema:rangeIncludes schema:Duration ;
    rdfs:comment "The total time it takes to prepare and cook the recipe, in ISO 8601 duration format." .

schema:totalValue a rdf:Property ;
    rdfs:label "totalValue" ;
    schema:domainIncludes schema:MedicalEntity ;
    schema:rangeIncludes schema:Number ;
    rdfs:comment "Total number of something." .

schema:transFatContent a rdf:Property ;
    rdfs:label "transFatContent" ;
    schema:domainIncludes schema:NutritionInformation ;
    schema:rangeIncludes schema:Mass ;
    rdfs:comment "The number of grams of trans fat." .

schema:transferDate a rdf:Property ;
    rdfs:label "transferDate" ;
    schema:domainIncludes schema:MedicalTransfer,
        schema:Person ;
    schema:rangeIncludes schema:DateTime ;
    rdfs:comment "Specifying the medical transfer date for a patient" ;
    rdfs:subPropertyOf schema:dateTime .

schema:transmissionMethod a rdf:Property ;
    rdfs:label "transmissionMethod" ;
    schema:domainIncludes schema:InfectiousDisease ;
    schema:rangeIncludes schema:Text ;
    rdfs:comment "How the disease spreads, either as a route or vector, for example 'direct contact', 'Aedes aegypti', etc." .

schema:treatingPhysician a rdf:Property ;
    rdfs:label "treatingPhysician" ;
    schema:domainIncludes schema:CaringEvent,
        schema:Patient ;
    schema:rangeIncludes <http://purl.bioontology.org/ontology/SNOMEDCT/223366009>,
        schema:HealthcareProfessional ;
    rdfs:comment "Specifying a specific physician assigned to the patient as specific or individual healthcare provider." ;
    rdfs:subPropertyOf schema:careProvider .

schema:triageProcedure a rdf:Property ;
    rdfs:label "triageProcedure" ;
    schema:domainIncludes schema:CaringEvent,
        schema:Patient ;
    schema:rangeIncludes schema:MedicalTriage ;
    rdfs:comment "Specifying a triage procedure resource" .

schema:triageScore a rdf:Property ;
    rdfs:label "triageScore" ;
    schema:domainIncludes schema:Patient,
        schema:TriageScore ;
    schema:rangeIncludes schema:Number ;
    rdfs:comment "Specifying the value of a triage score" .

schema:trialDesign a rdf:Property ;
    rdfs:label "trialDesign" ;
    schema:domainIncludes schema:MedicalTrial ;
    schema:rangeIncludes schema:MedicalTrialDesign ;
    rdfs:comment "Specifics about the trial design (enumerated)." .

schema:tributary a rdf:Property ;
    rdfs:label "tributary" ;
    schema:domainIncludes schema:Vein ;
    schema:rangeIncludes schema:AnatomicalStructure ;
    rdfs:comment "The anatomical or organ system that the vein flows into; a larger structure that the vein connects to." .

schema:typicalTest a rdf:Property ;
    rdfs:label "typicalTest" ;
    schema:domainIncludes schema:MedicalCondition ;
    schema:rangeIncludes schema:MedicalTest ;
    rdfs:comment "A medical test typically performed given this condition." .

schema:unsaturatedFatContent a rdf:Property ;
    rdfs:label "unsaturatedFatContent" ;
    schema:domainIncludes schema:NutritionInformation ;
    schema:rangeIncludes schema:Mass ;
    rdfs:comment "The number of grams of unsaturated fat." .

schema:usedToDiagnose a rdf:Property ;
    rdfs:label "usedToDiagnose" ;
    schema:domainIncludes schema:MedicalTest ;
    schema:rangeIncludes schema:MedicalCondition ;
    rdfs:comment "A condition the test is used to diagnose." .

schema:usesDevice a rdf:Property ;
    rdfs:label "usesDevice" ;
    schema:domainIncludes schema:MedicalTest ;
    schema:rangeIncludes schema:MedicalDevice ;
    rdfs:comment "Device used to perform the test." .

schema:vaccination a rdf:Property ;
    rdfs:label "vaccination" ;
    schema:domainIncludes schema:Person ;
    schema:rangeIncludes schema:Vaccination ;
    rdfs:comment "Specifying a vaccination procedure resource" ;
    rdfs:subPropertyOf schema:primaryPrevention .

schema:vitalSign a rdf:Property ;
    rdfs:label "vitalSign" ;
    schema:domainIncludes schema:Patient ;
    schema:rangeIncludes schema:VitalSign ;
    rdfs:comment "Specifying the vital sign of a person" ;
    rdfs:subPropertyOf schema:medicalSign .

schema:waistCircumference a rdf:Property ;
    rdfs:label "waistCircumference" ;
    schema:domainIncludes schema:Person,
        schema:WaistCircumference ;
    schema:rangeIncludes schema:Number ;
    rdfs:comment "The waist circumference measurement of someone" .

schema:waistHipRatio a rdf:Property ;
    rdfs:label "waistHipRatio" ;
    schema:domainIncludes schema:Person,
        schema:WaistHipRatio ;
    schema:rangeIncludes schema:Number ;
    rdfs:comment "The waist hip ratio measurement of someone" .

schema:warning a rdf:Property ;
    rdfs:label "warning" ;
    schema:domainIncludes schema:Drug ;
    schema:rangeIncludes schema:Text,
        schema:URL ;
    rdfs:comment "Any FDA or other warnings about the drug (text or URL)." .

schema:adverseEvent a rdf:Property ;
    rdfs:label "adverseEvent" ;
    schema:domainIncludes <http://purl.bioontology.org/ontology/SNOMEDCT/105590001>,
        <http://purl.bioontology.org/ontology/SNOMEDCT/277132007>,
        schema:MedicalProcedure,
        schema:MedicalTherapy,
        schema:Patient,
        schema:TherapeuticProcedure ;
    schema:rangeIncludes <http://purl.bioontology.org/ontology/SNOMEDCT/281647001>,
        schema:AdverseEvent ;
    rdfs:comment "Any unfavorable and unintended sign including an abnormal laboratory finding, symptom or disease associated with the use of a medical treatment or procedure, regardless of whether it is considered related to the medical treatment or procedure, that occurs during the course of the study (Stony Brook Medicine, NIH)." ;
    rdfs:subPropertyOf schema:adverseOutcome .

schema:cause a rdf:Property ;
    rdfs:label "cause" ;
    schema:domainIncludes schema:MedicalCondition,
        schema:MedicalSignOrSymptom ;
    schema:rangeIncludes schema:MedicalCause ;
    rdfs:comment "Specifying a cause of something in general. e.g in medicine , one of the causative agent(s) that are most directly responsible for the pathophysiologic process that eventually results in the occurrence." .

schema:electiveProcedure a rdf:Property ;
    rdfs:label "electiveProcedure" ;
    schema:domainIncludes schema:Person ;
    schema:rangeIncludes schema:ElectiveProcedure ;
    rdfs:comment "Specifying the elective procedure resource for a patient or a person." ;
    rdfs:subPropertyOf schema:medicalProcedure .

schema:lifeEvent a rdf:Property ;
    rdfs:label "lifeEvent" ;
    schema:domainIncludes schema:Patient ;
    schema:rangeIncludes schema:LifeEvent ;
    rdfs:comment "Specifying an event in person's life time line" .

schema:medicalRecord a rdf:Property ;
    rdfs:label "medicalRecord" ;
    schema:domainIncludes schema:Patient ;
    schema:rangeIncludes schema:MedicalRecord ;
    rdfs:comment "Specifying a medical record for a given medical entity or patient." .

schema:medicalSpecialty a rdf:Property ;
    rdfs:label "medicalSpecialty" ;
    schema:domainIncludes schema:Hospital,
        schema:MedicalClinic,
        schema:Physician ;
    schema:rangeIncludes schema:MedicalSpecialty ;
    rdfs:comment "A medical specialty of the provider." .

schema:medicalSymptom a rdf:Property ;
    rdfs:label "medicalSymptom" ;
    schema:domainIncludes schema:Patient ;
    schema:rangeIncludes schema:MedicalSymptom ;
    rdfs:comment "Specifying a symptom resource" ;
    rdfs:subPropertyOf schema:signOrSymptom .

schema:preventiveProcedure a rdf:Property ;
    rdfs:label "preventiveProcedure" ;
    schema:domainIncludes schema:Patient ;
    schema:rangeIncludes schema:PreventiveProcedure ;
    rdfs:comment "Specifying any preventive procedure resource for a person" ;
    rdfs:subPropertyOf schema:therapeuticProcedure .

schema:primaryPrevention a rdf:Property ;
    rdfs:label "primaryPrevention" ;
    schema:domainIncludes schema:MedicalCondition ;
    schema:rangeIncludes schema:MedicalTherapy ;
    rdfs:comment "A preventative therapy used to prevent an initial occurrence of the medical condition, such as vaccination." ;
    rdfs:subPropertyOf schema:preventiveProcedure .

schema:procedure a rdf:Property ;
    rdfs:label "procedure" ;
    schema:domainIncludes schema:MedicalDevice ;
    schema:rangeIncludes schema:Text ;
    rdfs:comment "A description of the procedure involved in setting up, using, and/or installing the device." .

schema:religionGroup a rdf:Property ;
    rdfs:label "religionGroup" ;
    schema:domainIncludes schema:Person ;
    schema:rangeIncludes schema:ReligionGroup ;
    rdfs:comment "Specifying a religion group of person." .

schema:Enzyme a rdf:Property ;
    rdfs:label "Enzyme" ;
    schema:domainIncludes schema:PhysiologicalEntity ;
    schema:rangeIncludes schema:Enzyme ;
    rdfs:comment "Biological molecules (proteins) that act as catalysts and help biochemical reactions into the body" .

schema:adverseOutcome a rdf:Property ;
    rdfs:label "adverseOutcome" ;
    schema:domainIncludes schema:MedicalDevice,
        schema:TherapeuticProcedure ;
    schema:rangeIncludes schema:MedicalEntity ;
    rdfs:comment "A possible complication and/or side effect of this therapy. If it is known that an adverse outcome is serious (resulting in death, disability, or permanent damage; requiring hospitalization; or is otherwise life-threatening or requires immediate medical attention), tag it as a seriouseAdverseOutcome instead." .

schema:bloodPressure a rdf:Property ;
    rdfs:label "bloodPressure" ;
    schema:domainIncludes schema:Person ;
    schema:rangeIncludes <http://purl.bioontology.org/ontology/SNOMEDCT/75367002>,
        schema:BloodPressure ;
    rdfs:comment "Specifying the blood pressure resource of a patient" .

schema:careProvider a rdf:Property ;
    rdfs:label "careProvider" ;
    schema:domainIncludes schema:CaringEvent,
        schema:MedicalProcedure,
        schema:Patient ;
    schema:rangeIncludes <http://purl.bioontology.org/ontology/SNOMEDCT/223366009>,
        schema:HealthcareProfessional,
        schema:Person,
        schema:Place ;
    rdfs:comment "Specifying a person, medical organization, or unit care-provider for any health care services" ;
    rdfs:subPropertyOf schema:provider .

schema:diagnosticProcedure a rdf:Property ;
    rdfs:label "diagnosticProcedure" ;
    schema:domainIncludes schema:Patient ;
    schema:rangeIncludes schema:DiagnosticProcedure ;
    rdfs:comment "Specifying the diagnostic procedure resource for a patient or a person." ;
    rdfs:subPropertyOf schema:medicalProcedure .

schema:familyMember a rdf:Property ;
    rdfs:label "familyMember" ;
    schema:domainIncludes schema:Person ;
    schema:rangeIncludes schema:Person ;
    rdfs:comment "Specifying a family member for this person" .

schema:gynObsHistory a rdf:Property ;
    rdfs:label "gynObsHistory" ;
    schema:domainIncludes schema:Person ;
    schema:rangeIncludes schema:GynObsHistory ;
    rdfs:comment "Specifying the gynaecology-obstetric history of a patient" ;
    rdfs:subPropertyOf schema:personalHistory .

schema:indication a rdf:Property ;
    rdfs:label "indication" ;
    schema:domainIncludes <http://purl.bioontology.org/ontology/SNOMEDCT/71388002>,
        schema:CaringEvent,
        schema:MedicalDevice,
        schema:MedicalIndication,
        schema:MedicalIntervention,
        schema:MedicalProcedure,
        schema:TherapeuticProcedure ;
    schema:rangeIncludes schema:MedicalIndication ;
    rdfs:comment "A factor that indicates use of this therapy for treatment and/or prevention of a condition, symptom, etc. For therapies such as drugs, indications can include both officially-approved indications as well as off-label uses. These can be distinguished by using the ApprovedIndication subtype of MedicalIndication." .

schema:interval a rdf:Property ;
    rdfs:label "interval" ;
    schema:domainIncludes schema:MedicalEntity ;
    schema:rangeIncludes schema:QuantitativeValue ;
    rdfs:comment "Typically derived from W3C Time Ontology this describes a time interval when an event or action occurs." .

schema:medicalHistory a rdf:Property ;
    rdfs:label "medicalHistory" ;
    schema:domainIncludes schema:Person ;
    schema:rangeIncludes schema:MedicalHistory ;
    rdfs:comment "Specifying a full medical history provided by the patient during an anamnesis procedure ." .

schema:medicalSign a rdf:Property ;
    rdfs:label "medicalSign" ;
    schema:domainIncludes schema:MedicalCondition,
        schema:MedicalScore,
        schema:Patient ;
    rdfs:comment "Specifying a sign resource" ;
    rdfs:subPropertyOf schema:signOrSymptom .

schema:signOrSymptom a rdf:Property ;
    rdfs:label "signOrSymptom" ;
    schema:domainIncludes schema:MedicalCondition ;
    schema:rangeIncludes schema:MedicalSignOrSymptom ;
    rdfs:comment "A sign or symptom of this condition. Signs are objective or physically observable manifestations of the medical condition while symptoms are the subjective experience of the medical condition." .

schema:treatment a rdf:Property ;
    rdfs:label "treatment" ;
    schema:domainIncludes <http://purl.bioontology.org/ontology/SNOMEDCT/64572001>,
        schema:MedicalCondition,
        schema:Patient ;
    schema:rangeIncludes <http://purl.bioontology.org/ontology/SNOMEDCT/277132007>,
        schema:Drug,
        schema:TherapeuticProcedure ;
    rdfs:comment "Specifying a treatment or management or therapeutic procedures for a disorder or a patient" .

schema:medicalEncounter a rdf:Property ;
    rdfs:label "medicalEncounter" ;
    schema:domainIncludes schema:Person ;
    schema:rangeIncludes <http://purl.bioontology.org/ontology/SNOMEDCT/308335008>,
        schema:MedicalEncounter ;
    rdfs:comment "Specifying a medical encounter between the patient and a healthcare provider." .

schema:status a rdf:Property ;
    rdfs:label "status" ;
    schema:domainIncludes schema:MedicalStudy ;
    schema:rangeIncludes schema:MedicalStudyStatus ;
    rdfs:comment "The status of the study (enumerated)." .

schema:lifestyleOrHabit a rdf:Property ;
    rdfs:label "lifestyleOrHabit" ;
    schema:domainIncludes schema:Person ;
    schema:rangeIncludes schema:LifestyleOrHabits ;
    rdfs:comment "describing the lifestyles or habits of the person" ;
    rdfs:subPropertyOf schema:personalHistory .

schema:therapeuticProcedure a rdf:Property ;
    rdfs:label "therapeuticProcedure" ;
    schema:domainIncludes schema:Person ;
    schema:rangeIncludes schema:TherapeuticProcedure ;
    rdfs:comment "Specifying the therapeutic procedure resource for a patient or a person." ;
    rdfs:subPropertyOf schema:medicalProcedure .

schema:clinicalDocument a rdf:Property ;
    rdfs:label "clinicalDocument" ;
    schema:domainIncludes schema:Patient ;
    schema:rangeIncludes schema:ClinicalDocument ;
    rdfs:comment "Specifying any clinical document" .

schema:socialHistory a rdf:Property ;
    rdfs:label "socialHistory" ;
    schema:domainIncludes schema:Person ;
    schema:rangeIncludes schema:SocialHistory ;
    rdfs:comment "Specifying the social history resource of the patient or person." ;
    rdfs:subPropertyOf schema:personalHistory .

schema:dateTime a rdf:Property ;
    rdfs:label "dateTime" ;
    schema:domainIncludes schema:MedicalEntity ;
    schema:rangeIncludes schema:DateTime ;
    rdfs:comment "Specifying an instant of something. Typically derived from W3C Time Ontology this describes a point in time when an event or action occurs." .

schema:healthFacility a rdf:Property ;
    rdfs:label "healthFacility" ;
    schema:domainIncludes <http://purl.bioontology.org/ontology/SNOMEDCT/404684003>,
        schema:ClinicalFinding,
        schema:LifeEvent,
        schema:MedicalIntervention,
        schema:MedicalProcedure,
        schema:Patient ;
    schema:rangeIncludes schema:HealthFacility ;
    rdfs:comment "Specifying a health facility where care is being given." .

schema:personalHistory a rdf:Property ;
    rdfs:label "personalHistory" ;
    schema:domainIncludes schema:Person ;
    schema:rangeIncludes <http://purl.bioontology.org/ontology/SNOMEDCT/160476009>,
        schema:PersonalHistory ;
    rdfs:comment " specifying a personal history provided by the patient during an anamnesis procedure ." ;
    rdfs:subPropertyOf schema:medicalHistory .

schema:medicalProcedure a rdf:Property ;
    rdfs:label "medicalProcedure" ;
    schema:domainIncludes schema:Patient ;
    schema:rangeIncludes schema:MedicalProcedure ;
    rdfs:comment "Specifying the medical procedure resource of the patient or person." ;
    rdfs:subPropertyOf schema:procedure .
